<?xml version="1.0"?>
<rdf:RDF xmlns="http://www.semanticweb.org/ontologies/2022/6/geological_taxonomy#"
     xml:base="http://www.semanticweb.org/ontologies/2022/6/geological_taxonomy"
     xmlns:owl="http://www.w3.org/2002/07/owl#"
     xmlns:rdf="http://www.w3.org/1999/02/22-rdf-syntax-ns#"
     xmlns:xml="http://www.w3.org/XML/1998/namespace"
     xmlns:xsd="http://www.w3.org/2001/XMLSchema#"
     xmlns:rdfs="http://www.w3.org/2000/01/rdf-schema#">
    <owl:Ontology/>
    


    <!-- 
    ///////////////////////////////////////////////////////////////////////////////////////
    //
    // Classes
    //
    ///////////////////////////////////////////////////////////////////////////////////////
     -->

    


    <!-- http://www.semanticweb.org/ontologies/2022/6/geological_taxonomy#Abnormally_Dry -->

    <owl:Class rdf:about="http://www.semanticweb.org/ontologies/2022/6/geological_taxonomy#Abnormally_Dry">
        <rdfs:subClassOf rdf:resource="http://www.semanticweb.org/ontologies/2022/6/geological_taxonomy#Drought"/>
        <rdfs:comment>It is the D0 category that refers short-term dryness slowing planting, growth of crops or pastures.

Resource: https://droughtmonitor.unl.edu/About/WhatistheUSDM.aspx</rdfs:comment>
    </owl:Class>
    


    <!-- http://www.semanticweb.org/ontologies/2022/6/geological_taxonomy#Adakite -->

    <owl:Class rdf:about="http://www.semanticweb.org/ontologies/2022/6/geological_taxonomy#Adakite">
        <rdfs:subClassOf rdf:resource="http://www.semanticweb.org/ontologies/2022/6/geological_taxonomy#Basalt"/>
        <rdfs:comment>A class of basaltic rocks containing low yttrium and ytterbium

Resource: https://geology.fandom.com/wiki/List_of_rock_types</rdfs:comment>
    </owl:Class>
    


    <!-- http://www.semanticweb.org/ontologies/2022/6/geological_taxonomy#Albolls -->

    <owl:Class rdf:about="http://www.semanticweb.org/ontologies/2022/6/geological_taxonomy#Albolls">
        <rdfs:subClassOf rdf:resource="http://www.semanticweb.org/ontologies/2022/6/geological_taxonomy#Mollisols"/>
        <rdfs:comment>Albolls have a bleached subsurface horizon called the albic horizon and are usually wet

Resource: https://www.sciencedirect.com/topics/agricultural-and-biological-sciences/mollisol</rdfs:comment>
    </owl:Class>
    


    <!-- http://www.semanticweb.org/ontologies/2022/6/geological_taxonomy#Alfisols -->

    <owl:Class rdf:about="http://www.semanticweb.org/ontologies/2022/6/geological_taxonomy#Alfisols">
        <rdfs:subClassOf rdf:resource="http://www.semanticweb.org/ontologies/2022/6/geological_taxonomy#Soil"/>
        <rdfs:comment>The central concept of Alfisols is that of soils that have an argillic, a kandic, or a natric horizon and a base saturation of 35% or greater.

Resource: https://www.nrcs.usda.gov/wps/portal/nrcs/detail/soils/survey/class/maps/?cid=nrcs142p2_053590

Justification: Depending upon soil Moisture regimes</rdfs:comment>
    </owl:Class>
    


    <!-- http://www.semanticweb.org/ontologies/2022/6/geological_taxonomy#Alkali_feldspar_granite -->

    <owl:Class rdf:about="http://www.semanticweb.org/ontologies/2022/6/geological_taxonomy#Alkali_feldspar_granite">
        <rdfs:subClassOf rdf:resource="http://www.semanticweb.org/ontologies/2022/6/geological_taxonomy#Igneous_rocks"/>
        <rdfs:comment>Alkali feldspar granite, some varieties of which are called &apos;red granite&apos;, is a felsic igneous rock and a type of granite rich in the mineral potassium feldspar (K-spar).

Resource: https://en.wikipedia.org/wiki/Alkali_feldspar_granite</rdfs:comment>
    </owl:Class>
    


    <!-- http://www.semanticweb.org/ontologies/2022/6/geological_taxonomy#Amphibolite -->

    <owl:Class rdf:about="http://www.semanticweb.org/ontologies/2022/6/geological_taxonomy#Amphibolite">
        <rdfs:subClassOf rdf:resource="http://www.semanticweb.org/ontologies/2022/6/geological_taxonomy#Metamorphic_rocks"/>
        <rdfs:comment>A metamorphic rock containing mainly amphibole and plagioclase

Resource: https://en.wikipedia.org/wiki/List_of_rock_types</rdfs:comment>
    </owl:Class>
    


    <!-- http://www.semanticweb.org/ontologies/2022/6/geological_taxonomy#Andesite -->

    <owl:Class rdf:about="http://www.semanticweb.org/ontologies/2022/6/geological_taxonomy#Andesite">
        <rdfs:subClassOf rdf:resource="http://www.semanticweb.org/ontologies/2022/6/geological_taxonomy#Igneous_rocks"/>
        <rdfs:comment>Andesite is a volcanic rock of intermediate composition.

Resource: https://en.wikipedia.org/wiki/Andesite</rdfs:comment>
    </owl:Class>
    


    <!-- http://www.semanticweb.org/ontologies/2022/6/geological_taxonomy#Andisols -->

    <owl:Class rdf:about="http://www.semanticweb.org/ontologies/2022/6/geological_taxonomy#Andisols">
        <rdfs:subClassOf rdf:resource="http://www.semanticweb.org/ontologies/2022/6/geological_taxonomy#Soil"/>
        <rdfs:comment>The central concept of Andisols is that of soils dominated by short-range-order minerals. They include weakly weathered soils with much volcanic glass as well as more strongly weathered soils.

Resource: https://www.nrcs.usda.gov/wps/portal/nrcs/detail/soils/survey/class/maps/?cid=nrcs142p2_053592

Justification: These suborders are defined based on soil temperature and soil moisture regimes.
https://www.nasa.gov/centers/johnson/pdf/486016main_Takahashi.pdf</rdfs:comment>
    </owl:Class>
    


    <!-- http://www.semanticweb.org/ontologies/2022/6/geological_taxonomy#Anorthosite -->

    <owl:Class rdf:about="http://www.semanticweb.org/ontologies/2022/6/geological_taxonomy#Anorthosite">
        <rdfs:subClassOf rdf:resource="http://www.semanticweb.org/ontologies/2022/6/geological_taxonomy#Igneous_rocks"/>
        <rdfs:comment>An intrusive igneous felsic rock composed predominantly of plagioclase

Resource: https://geology.fandom.com/wiki/Anorthosite</rdfs:comment>
    </owl:Class>
    


    <!-- http://www.semanticweb.org/ontologies/2022/6/geological_taxonomy#Anthracite -->

    <owl:Class rdf:about="http://www.semanticweb.org/ontologies/2022/6/geological_taxonomy#Anthracite">
        <rdfs:subClassOf rdf:resource="http://www.semanticweb.org/ontologies/2022/6/geological_taxonomy#Metamorphic_rocks"/>
        <rdfs:comment>Anthracite is a type of coal with a highest rank. Coal rank measures the carbon content which is in correlation with calorific value and metamorphic grade.

Resource: https://www.sandatlas.org/rock-types/#Anthracite</rdfs:comment>
    </owl:Class>
    


    <!-- http://www.semanticweb.org/ontologies/2022/6/geological_taxonomy#Anthrepts -->

    <owl:Class rdf:about="http://www.semanticweb.org/ontologies/2022/6/geological_taxonomy#Anthrepts">
        <rdfs:subClassOf rdf:resource="http://www.semanticweb.org/ontologies/2022/6/geological_taxonomy#Inceptisols"/>
        <rdfs:comment>Inceptisols that have a plaggen or anthropic epipedon

Resource: https://sites.google.com/site/dinpuithai/Home/key10/key10k</rdfs:comment>
    </owl:Class>
    


    <!-- http://www.semanticweb.org/ontologies/2022/6/geological_taxonomy#Aplite -->

    <owl:Class rdf:about="http://www.semanticweb.org/ontologies/2022/6/geological_taxonomy#Aplite">
        <rdfs:subClassOf rdf:resource="http://www.semanticweb.org/ontologies/2022/6/geological_taxonomy#Igneous_rocks"/>
        <rdfs:comment>Aplite is an intrusive igneous rock in which the mineral composition is the same as granite, but in which the grains are much finer, under 1 mm across.

Resource: https://en.wikipedia.org/wiki/Aplite</rdfs:comment>
    </owl:Class>
    


    <!-- http://www.semanticweb.org/ontologies/2022/6/geological_taxonomy#Aqualfs -->

    <owl:Class rdf:about="http://www.semanticweb.org/ontologies/2022/6/geological_taxonomy#Aqualfs">
        <rdfs:subClassOf rdf:resource="http://www.semanticweb.org/ontologies/2022/6/geological_taxonomy#Alfisols"/>
        <rdfs:comment>In the horizons that have aquic conditions, enough active ferrous iron to give a positive reaction to alpha,alphadipyridyl at a time when the soil is not being irrigated.

Resource: https://sites.google.com/site/dinpuithai/Home/taxonomy/j-alfisols</rdfs:comment>
    </owl:Class>
    


    <!-- http://www.semanticweb.org/ontologies/2022/6/geological_taxonomy#Aquands -->

    <owl:Class rdf:about="http://www.semanticweb.org/ontologies/2022/6/geological_taxonomy#Aquands">
        <rdfs:subClassOf rdf:resource="http://www.semanticweb.org/ontologies/2022/6/geological_taxonomy#Andisols"/>
        <rdfs:comment>Andisols with a water table at or near the surface for much of the year.

Resource: https://en.wikipedia.org/wiki/Andisol</rdfs:comment>
    </owl:Class>
    


    <!-- http://www.semanticweb.org/ontologies/2022/6/geological_taxonomy#Aquents -->

    <owl:Class rdf:about="http://www.semanticweb.org/ontologies/2022/6/geological_taxonomy#Aquents">
        <rdfs:subClassOf rdf:resource="http://www.semanticweb.org/ontologies/2022/6/geological_taxonomy#Entisols"/>
        <rdfs:comment>Wet Entisols (aquic conditions in the upper part)

Resource: &quot;Illustrated Guide to Soil Taxonomy&quot; book by Unites States Department of Agriculture</rdfs:comment>
    </owl:Class>
    


    <!-- http://www.semanticweb.org/ontologies/2022/6/geological_taxonomy#Aquepts -->

    <owl:Class rdf:about="http://www.semanticweb.org/ontologies/2022/6/geological_taxonomy#Aquepts">
        <rdfs:subClassOf rdf:resource="http://www.semanticweb.org/ontologies/2022/6/geological_taxonomy#Inceptisols"/>
        <rdfs:comment>They show redoximorphic features and are saturated with water at some period in the year. Aquepts usually have cambic horizons and commonly in the US, they have fragipans

Resource: https://web.archive.org/web/20040918225129/http://grunwald.ifas.ufl.edu/Nat_resources/soil_orders/inceptisols.htm</rdfs:comment>
    </owl:Class>
    


    <!-- http://www.semanticweb.org/ontologies/2022/6/geological_taxonomy#Aquerts -->

    <owl:Class rdf:about="http://www.semanticweb.org/ontologies/2022/6/geological_taxonomy#Aquerts">
        <rdfs:subClassOf rdf:resource="http://www.semanticweb.org/ontologies/2022/6/geological_taxonomy#Vertisols"/>
        <rdfs:comment>Vertisols that have, in one or more horizons within 50 cm of the mineral soil surface, aquic conditions for some time in normal years (or artificial drainage)

Resource: https://sites.google.com/site/dinpuithai/Home/key10/key10f</rdfs:comment>
    </owl:Class>
    


    <!-- http://www.semanticweb.org/ontologies/2022/6/geological_taxonomy#Aquods -->

    <owl:Class rdf:about="http://www.semanticweb.org/ontologies/2022/6/geological_taxonomy#Aquods">
        <rdfs:subClassOf rdf:resource="http://www.semanticweb.org/ontologies/2022/6/geological_taxonomy#Spodosols"/>
        <rdfs:comment>Wet Spodosols (aquic conditions in the upper part)

Resource: &quot;Illustrated Guide to Soil Taxonomy&quot; book by Unites States Department of Agriculture</rdfs:comment>
    </owl:Class>
    


    <!-- http://www.semanticweb.org/ontologies/2022/6/geological_taxonomy#Aquolls -->

    <owl:Class rdf:about="http://www.semanticweb.org/ontologies/2022/6/geological_taxonomy#Aquolls">
        <rdfs:subClassOf rdf:resource="http://www.semanticweb.org/ontologies/2022/6/geological_taxonomy#Mollisols"/>
        <rdfs:comment>Aquolls are wet Mollisols and may have a histic epipedon

Resource: https://www.sciencedirect.com/topics/agricultural-and-biological-sciences/mollisol</rdfs:comment>
    </owl:Class>
    


    <!-- http://www.semanticweb.org/ontologies/2022/6/geological_taxonomy#Aquox -->

    <owl:Class rdf:about="http://www.semanticweb.org/ontologies/2022/6/geological_taxonomy#Aquox">
        <rdfs:subClassOf rdf:resource="http://www.semanticweb.org/ontologies/2022/6/geological_taxonomy#Oxisols"/>
        <rdfs:comment>Oxisols that have aquic conditions for some time in normal years (or artificial drainage) in one or more horizons within 50 cm of the mineral soil surface

Resource: https://sites.google.com/site/dinpuithai/Home/key10/key10e</rdfs:comment>
    </owl:Class>
    


    <!-- http://www.semanticweb.org/ontologies/2022/6/geological_taxonomy#Aquults -->

    <owl:Class rdf:about="http://www.semanticweb.org/ontologies/2022/6/geological_taxonomy#Aquults">
        <rdfs:subClassOf rdf:resource="http://www.semanticweb.org/ontologies/2022/6/geological_taxonomy#Ultisols"/>
        <rdfs:comment>Ultisols that have aquic conditions for some time in normal years (or artificial drainage) in one or more horizons within 50 cm of the mineral soil surface

Resource: https://sites.google.com/site/dinpuithai/Home/key10/key10h</rdfs:comment>
    </owl:Class>
    


    <!-- http://www.semanticweb.org/ontologies/2022/6/geological_taxonomy#Areal -->

    <owl:Class rdf:about="http://www.semanticweb.org/ontologies/2022/6/geological_taxonomy#Areal">
        <rdfs:subClassOf rdf:resource="http://www.semanticweb.org/ontologies/2022/6/geological_taxonomy#Flood"/>
        <rdfs:comment>Areal floods are caused when excessive snowmelt or high rainfall accumulates on land, sometimes to hazardous depths	

Resource: https://www.worldatlas.com/articles/how-many-types-of-floods-are-there.html</rdfs:comment>
    </owl:Class>
    


    <!-- http://www.semanticweb.org/ontologies/2022/6/geological_taxonomy#Arents -->

    <owl:Class rdf:about="http://www.semanticweb.org/ontologies/2022/6/geological_taxonomy#Arents">
        <rdfs:subClassOf rdf:resource="http://www.semanticweb.org/ontologies/2022/6/geological_taxonomy#Entisols"/>
        <rdfs:comment>Entisols that have, in one or more layers at a depth between 25 and 100 cm below the mineral soil surface, 3 percent or more (by volume) fragments of diagnostic horizons that are not arranged in any discernible order.

Resource: https://sites.google.com/site/dinpuithai/Home/key10/key10l</rdfs:comment>
    </owl:Class>
    


    <!-- http://www.semanticweb.org/ontologies/2022/6/geological_taxonomy#Argids -->

    <owl:Class rdf:about="http://www.semanticweb.org/ontologies/2022/6/geological_taxonomy#Argids">
        <rdfs:subClassOf rdf:resource="http://www.semanticweb.org/ontologies/2022/6/geological_taxonomy#Aridisols"/>
        <rdfs:comment>Characterized by an accumulation of clay by translocation, the Argids are present in areas adjoining soils with an ustic SMR.

Resource: https://www.sciencedirect.com/topics/agricultural-and-biological-sciences/aridisol</rdfs:comment>
    </owl:Class>
    


    <!-- http://www.semanticweb.org/ontologies/2022/6/geological_taxonomy#Argillite -->

    <owl:Class rdf:about="http://www.semanticweb.org/ontologies/2022/6/geological_taxonomy#Argillite">
        <rdfs:subClassOf rdf:resource="http://www.semanticweb.org/ontologies/2022/6/geological_taxonomy#Sedimentary_rocks"/>
        <rdfs:comment>Sedimentary rock, mostly of indurated clay particles

Resource: https://en.wikipedia.org/wiki/List_of_rock_types</rdfs:comment>
    </owl:Class>
    


    <!-- http://www.semanticweb.org/ontologies/2022/6/geological_taxonomy#Aridisols -->

    <owl:Class rdf:about="http://www.semanticweb.org/ontologies/2022/6/geological_taxonomy#Aridisols">
        <rdfs:subClassOf rdf:resource="http://www.semanticweb.org/ontologies/2022/6/geological_taxonomy#Soil"/>
        <rdfs:comment>The central concept of Aridisols is that of soils that are too dry for mesophytic plants to grow.

Resource: https://www.nrcs.usda.gov/wps/portal/nrcs/detail/soils/survey/class/maps/?cid=nrcs142p2_053594

Justification: Depending upon the composition and accumulation of the soluble fraction and results of dominant soil-forming processes.
https://www.sciencedirect.com/topics/agricultural-and-biological-sciences/aridisol</rdfs:comment>
    </owl:Class>
    


    <!-- http://www.semanticweb.org/ontologies/2022/6/geological_taxonomy#Arkose -->

    <owl:Class rdf:about="http://www.semanticweb.org/ontologies/2022/6/geological_taxonomy#Arkose">
        <rdfs:subClassOf rdf:resource="http://www.semanticweb.org/ontologies/2022/6/geological_taxonomy#Sedimentary_rocks"/>
        <rdfs:comment>A sedimentary rock similar to sandstone

Resource: https://geology.fandom.com/wiki/List_of_rock_types</rdfs:comment>
    </owl:Class>
    


    <!-- http://www.semanticweb.org/ontologies/2022/6/geological_taxonomy#Asthenosphere -->

    <owl:Class rdf:about="http://www.semanticweb.org/ontologies/2022/6/geological_taxonomy#Asthenosphere">
        <rdfs:subClassOf rdf:resource="http://www.semanticweb.org/ontologies/2022/6/geological_taxonomy#Upper_mantle"/>
        <rdfs:comment>layer in Earth&apos;s mantle between the lithosphere (above) and the upper mantle (below). It is the weak and easily deformed layer of the Earth that acts as a “lubricant” for the tectonic plates to slide over.

Resource: https://education.nationalgeographic.org/resource/mantle
http://ser.sese.asu.edu/GEO110/GEO110_S03/Dis2b.pdf</rdfs:comment>
    </owl:Class>
    


    <!-- http://www.semanticweb.org/ontologies/2022/6/geological_taxonomy#Banded_iron_formation -->

    <owl:Class rdf:about="http://www.semanticweb.org/ontologies/2022/6/geological_taxonomy#Banded_iron_formation">
        <rdfs:subClassOf rdf:resource="http://www.semanticweb.org/ontologies/2022/6/geological_taxonomy#Sedimentary_rocks"/>
        <rdfs:comment>A fine grained chemical sedimentary rock composed of iron oxide minerals

Resource: https://geology.fandom.com/wiki/List_of_rock_types</rdfs:comment>
    </owl:Class>
    


    <!-- http://www.semanticweb.org/ontologies/2022/6/geological_taxonomy#Basalt -->

    <owl:Class rdf:about="http://www.semanticweb.org/ontologies/2022/6/geological_taxonomy#Basalt">
        <rdfs:subClassOf rdf:resource="http://www.semanticweb.org/ontologies/2022/6/geological_taxonomy#Igneous_rocks"/>
        <rdfs:comment>Basalt is an aphanitic (fine-grained) extrusive igneous rock formed from the rapid cooling of low-viscosity lava rich in magnesium and iron exposed at or very near the surface of a rocky planet or moon.

Resource: https://en.wikipedia.org/wiki/Basalt

Justification: Depending upon the type of the flow of Basaltic lava and different formation process from basalt</rdfs:comment>
    </owl:Class>
    


    <!-- http://www.semanticweb.org/ontologies/2022/6/geological_taxonomy#Basaltic_trachyandesite -->

    <owl:Class rdf:about="http://www.semanticweb.org/ontologies/2022/6/geological_taxonomy#Basaltic_trachyandesite">
        <rdfs:subClassOf rdf:resource="http://www.semanticweb.org/ontologies/2022/6/geological_taxonomy#Trachyandesite"/>
        <rdfs:comment>A alkaline/basic rocktype intermediate between andesite and phonolite, difficult to define without the TAS diagram.

Resource: https://www.mindat.org/min-48461.html</rdfs:comment>
    </owl:Class>
    


    <!-- http://www.semanticweb.org/ontologies/2022/6/geological_taxonomy#Basanite -->

    <owl:Class rdf:about="http://www.semanticweb.org/ontologies/2022/6/geological_taxonomy#Basanite">
        <rdfs:subClassOf rdf:resource="http://www.semanticweb.org/ontologies/2022/6/geological_taxonomy#Igneous_rocks"/>
        <rdfs:comment>Basanite is an igneous, volcanic (extrusive) rock with aphanitic to porphyritic texture.

Resource: https://en.wikipedia.org/wiki/Basanite</rdfs:comment>
    </owl:Class>
    


    <!-- http://www.semanticweb.org/ontologies/2022/6/geological_taxonomy#Bauxite -->

    <owl:Class rdf:about="http://www.semanticweb.org/ontologies/2022/6/geological_taxonomy#Bauxite">
        <rdfs:subClassOf rdf:resource="http://www.semanticweb.org/ontologies/2022/6/geological_taxonomy#Sedimentary_rocks"/>
        <rdfs:comment>Bauxite is an aluminum-rich sedimentary rock. It is a principal ore of aluminum.

Resource: https://www.sandatlas.org/rock-types/</rdfs:comment>
    </owl:Class>
    


    <!-- http://www.semanticweb.org/ontologies/2022/6/geological_taxonomy#Benmoreite -->

    <owl:Class rdf:about="http://www.semanticweb.org/ontologies/2022/6/geological_taxonomy#Benmoreite">
        <rdfs:subClassOf rdf:resource="http://www.semanticweb.org/ontologies/2022/6/geological_taxonomy#Trachyandesite"/>
        <rdfs:comment>Benmoreite is a silica-undersaturated volcanic rock of intermediate composition.

Resource: https://en.wikipedia.org/wiki/List_of_rock_types</rdfs:comment>
    </owl:Class>
    


    <!-- http://www.semanticweb.org/ontologies/2022/6/geological_taxonomy#Blairmorite -->

    <owl:Class rdf:about="http://www.semanticweb.org/ontologies/2022/6/geological_taxonomy#Blairmorite">
        <rdfs:subClassOf rdf:resource="http://www.semanticweb.org/ontologies/2022/6/geological_taxonomy#Igneous_rocks"/>
        <rdfs:comment>Blairmorite is a very rare porphyritic volcanic rock named after the community of Blairmore in southwestern Alberta, Canada.

Resource: https://en.wikipedia.org/wiki/Blairmorite</rdfs:comment>
    </owl:Class>
    


    <!-- http://www.semanticweb.org/ontologies/2022/6/geological_taxonomy#Blizzard -->

    <owl:Class rdf:about="http://www.semanticweb.org/ontologies/2022/6/geological_taxonomy#Blizzard">
        <rdfs:subClassOf rdf:resource="http://www.semanticweb.org/ontologies/2022/6/geological_taxonomy#Extratropical_cyclone"/>
        <owl:disjointWith rdf:resource="http://www.semanticweb.org/ontologies/2022/6/geological_taxonomy#Nor&apos;easter"/>
        <rdfs:comment>A blizzard is a severe snowstorm characterized by strong sustained winds and low visibility, lasting for a prolonged period of time

Resource: https://en.wikipedia.org/wiki/Blizzard</rdfs:comment>
    </owl:Class>
    


    <!-- http://www.semanticweb.org/ontologies/2022/6/geological_taxonomy#Block_slide -->

    <owl:Class rdf:about="http://www.semanticweb.org/ontologies/2022/6/geological_taxonomy#Block_slide">
        <rdfs:subClassOf rdf:resource="http://www.semanticweb.org/ontologies/2022/6/geological_taxonomy#Translational_slide"/>
        <rdfs:comment>translational slide in which the moving mass consists of a single unit or a few closely related units that move downslope as a relatively coherent mass

Resource: https://pubs.usgs.gov/fs/2004/3072/pdf/fs2004-3072.pdf

Justification: Based on the type of material</rdfs:comment>
    </owl:Class>
    


    <!-- http://www.semanticweb.org/ontologies/2022/6/geological_taxonomy#Blueschist -->

    <owl:Class rdf:about="http://www.semanticweb.org/ontologies/2022/6/geological_taxonomy#Blueschist">
        <rdfs:subClassOf rdf:resource="http://www.semanticweb.org/ontologies/2022/6/geological_taxonomy#Metamorphic_rocks"/>
        <rdfs:comment>A metamorphic rock composed of sodic amphiboles with a distinct blue color

Resource: https://geology.fandom.com/wiki/List_of_rock_types</rdfs:comment>
    </owl:Class>
    


    <!-- http://www.semanticweb.org/ontologies/2022/6/geological_taxonomy#Bog_iron -->

    <owl:Class rdf:about="http://www.semanticweb.org/ontologies/2022/6/geological_taxonomy#Bog_iron">
        <rdfs:subClassOf rdf:resource="http://www.semanticweb.org/ontologies/2022/6/geological_taxonomy#Sedimentary_rocks"/>
        <rdfs:comment>Bog iron is a type of iron ore composed of limonite with impurities like clay or plant debris.

Resource: https://www.sandatlas.org/rock-types/</rdfs:comment>
    </owl:Class>
    


    <!-- http://www.semanticweb.org/ontologies/2022/6/geological_taxonomy#Boninite -->

    <owl:Class rdf:about="http://www.semanticweb.org/ontologies/2022/6/geological_taxonomy#Boninite">
        <rdfs:subClassOf rdf:resource="http://www.semanticweb.org/ontologies/2022/6/geological_taxonomy#Igneous_rocks"/>
        <rdfs:comment>Boninite is an extrusive rock high in both magnesium and silica, thought to be usually formed in fore-arc environments, typically during the early stages of subduction. 

Resource: https://en.wikipedia.org/wiki/Boninite</rdfs:comment>
    </owl:Class>
    


    <!-- http://www.semanticweb.org/ontologies/2022/6/geological_taxonomy#Borates -->

    <owl:Class rdf:about="http://www.semanticweb.org/ontologies/2022/6/geological_taxonomy#Borates">
        <rdfs:subClassOf rdf:resource="http://www.semanticweb.org/ontologies/2022/6/geological_taxonomy#Mineral"/>
        <rdfs:comment>Borate mineral, any of various naturally occurring compounds of boron and oxygen.	

Resource: https://www.britannica.com/science/borate-mineral</rdfs:comment>
    </owl:Class>
    


    <!-- http://www.semanticweb.org/ontologies/2022/6/geological_taxonomy#Breaching_of_a_barrier -->

    <owl:Class rdf:about="http://www.semanticweb.org/ontologies/2022/6/geological_taxonomy#Breaching_of_a_barrier">
        <rdfs:subClassOf rdf:resource="http://www.semanticweb.org/ontologies/2022/6/geological_taxonomy#Coastal_Flood"/>
        <rdfs:comment>Breaching occurs when the barrier is broken down or destroyed by waves allowing the seawater to extend inland and flood the areas	

Resource: https://en.wikipedia.org/wiki/Coastal_flooding</rdfs:comment>
    </owl:Class>
    


    <!-- http://www.semanticweb.org/ontologies/2022/6/geological_taxonomy#Breccia -->

    <owl:Class rdf:about="http://www.semanticweb.org/ontologies/2022/6/geological_taxonomy#Breccia">
        <rdfs:subClassOf rdf:resource="http://www.semanticweb.org/ontologies/2022/6/geological_taxonomy#Sedimentary_rocks"/>
        <rdfs:comment>A sedimentary or tectonic rock composed of fragments of other, broken rocks

Resource: https://geology.fandom.com/wiki/List_of_rock_types</rdfs:comment>
    </owl:Class>
    


    <!-- http://www.semanticweb.org/ontologies/2022/6/geological_taxonomy#Calcarenite -->

    <owl:Class rdf:about="http://www.semanticweb.org/ontologies/2022/6/geological_taxonomy#Calcarenite">
        <rdfs:subClassOf rdf:resource="http://www.semanticweb.org/ontologies/2022/6/geological_taxonomy#Sedimentary_rocks"/>
        <rdfs:comment>A clastic sedimentary rock that is made up predominantly of recycled carbonate particles of sand size; a consolidated calcareous sand

Resource: https://mrdata.usgs.gov/geology/state/sgmc-lith.php?text=calcarenite</rdfs:comment>
    </owl:Class>
    


    <!-- http://www.semanticweb.org/ontologies/2022/6/geological_taxonomy#Calcflinta -->

    <owl:Class rdf:about="http://www.semanticweb.org/ontologies/2022/6/geological_taxonomy#Calcflinta">
        <rdfs:subClassOf rdf:resource="http://www.semanticweb.org/ontologies/2022/6/geological_taxonomy#Hornfels"/>
        <rdfs:comment>Calcflinta, or calc-flinta, is a fine grained calc–silicate rock found amongst the metamorphic rocks of the eastern Highlands of Scotland

Resource: https://en.wikipedia.org/wiki/Calcflinta</rdfs:comment>
    </owl:Class>
    


    <!-- http://www.semanticweb.org/ontologies/2022/6/geological_taxonomy#Calcids -->

    <owl:Class rdf:about="http://www.semanticweb.org/ontologies/2022/6/geological_taxonomy#Calcids">
        <rdfs:subClassOf rdf:resource="http://www.semanticweb.org/ontologies/2022/6/geological_taxonomy#Aridisols"/>
        <rdfs:comment>Characterized by an accumulation of carbonates, the soils have a calcic, petrocalcic, or a hypercalcic horizon.

Resource: https://www.sciencedirect.com/topics/agricultural-and-biological-sciences/aridisol</rdfs:comment>
    </owl:Class>
    


    <!-- http://www.semanticweb.org/ontologies/2022/6/geological_taxonomy#Cambids -->

    <owl:Class rdf:about="http://www.semanticweb.org/ontologies/2022/6/geological_taxonomy#Cambids">
        <rdfs:subClassOf rdf:resource="http://www.semanticweb.org/ontologies/2022/6/geological_taxonomy#Aridisols"/>
        <rdfs:comment>Characterized by a transformation of material, these soils are the most extensive of the Aridisols

Resource: https://www.sciencedirect.com/topics/agricultural-and-biological-sciences/aridisol</rdfs:comment>
    </owl:Class>
    


    <!-- http://www.semanticweb.org/ontologies/2022/6/geological_taxonomy#Carbonates -->

    <owl:Class rdf:about="http://www.semanticweb.org/ontologies/2022/6/geological_taxonomy#Carbonates">
        <rdfs:subClassOf rdf:resource="http://www.semanticweb.org/ontologies/2022/6/geological_taxonomy#Mineral"/>
        <rdfs:comment>The carbonate minerals are those in which the main anionic group is carbonate, [CO3]2−	

Resource: https://en.wikipedia.org/wiki/Mineral#Classification

Justification: classified based on the presence of hydroxyl anion(OH-)</rdfs:comment>
    </owl:Class>
    


    <!-- http://www.semanticweb.org/ontologies/2022/6/geological_taxonomy#Carbonatite -->

    <owl:Class rdf:about="http://www.semanticweb.org/ontologies/2022/6/geological_taxonomy#Carbonatite">
        <rdfs:subClassOf rdf:resource="http://www.semanticweb.org/ontologies/2022/6/geological_taxonomy#Igneous_rocks"/>
        <rdfs:comment>Carbonatite is a type of intrusive or extrusive igneous rock defined by mineralogic composition consisting of greater than 50% carbonate minerals. 

Resource: https://en.wikipedia.org/wiki/Carbonatite</rdfs:comment>
    </owl:Class>
    


    <!-- http://www.semanticweb.org/ontologies/2022/6/geological_taxonomy#Cataclasite -->

    <owl:Class rdf:about="http://www.semanticweb.org/ontologies/2022/6/geological_taxonomy#Cataclasite">
        <rdfs:subClassOf rdf:resource="http://www.semanticweb.org/ontologies/2022/6/geological_taxonomy#Metamorphic_rocks"/>
        <rdfs:comment>Cataclasite is a metamorphic rock that is formed by mechanical shear stress during faulting.

Resource: https://www.chemeurope.com/en/encyclopedia/Cataclasite.html</rdfs:comment>
    </owl:Class>
    


    <!-- http://www.semanticweb.org/ontologies/2022/6/geological_taxonomy#Chalk -->

    <owl:Class rdf:about="http://www.semanticweb.org/ontologies/2022/6/geological_taxonomy#Chalk">
        <rdfs:subClassOf rdf:resource="http://www.semanticweb.org/ontologies/2022/6/geological_taxonomy#Sedimentary_rocks"/>
        <rdfs:comment>A sedimentary rock composed primarily of coccolith fossils

Resource: https://geology.fandom.com/wiki/List_of_rock_types</rdfs:comment>
    </owl:Class>
    


    <!-- http://www.semanticweb.org/ontologies/2022/6/geological_taxonomy#Charnockite -->

    <owl:Class rdf:about="http://www.semanticweb.org/ontologies/2022/6/geological_taxonomy#Charnockite">
        <rdfs:subClassOf rdf:resource="http://www.semanticweb.org/ontologies/2022/6/geological_taxonomy#Igneous_rocks"/>
        <rdfs:comment>Charnockite, any member of a series of metamorphic rocks with variable chemical composition, first described from the state of Tamil Nadu in southern India and named for Job Charnock. 

Resource: https://www.britannica.com/science/charnockite

Justification: Classified based on presence of quartz, pyroxene.</rdfs:comment>
    </owl:Class>
    


    <!-- http://www.semanticweb.org/ontologies/2022/6/geological_taxonomy#Chert -->

    <owl:Class rdf:about="http://www.semanticweb.org/ontologies/2022/6/geological_taxonomy#Chert">
        <rdfs:subClassOf rdf:resource="http://www.semanticweb.org/ontologies/2022/6/geological_taxonomy#Sedimentary_rocks"/>
        <rdfs:comment>A fine grained chemical sedimentary rock composed of silica

Resource: https://geology.fandom.com/wiki/List_of_rock_types</rdfs:comment>
    </owl:Class>
    


    <!-- http://www.semanticweb.org/ontologies/2022/6/geological_taxonomy#Claystone -->

    <owl:Class rdf:about="http://www.semanticweb.org/ontologies/2022/6/geological_taxonomy#Claystone">
        <rdfs:subClassOf rdf:resource="http://www.semanticweb.org/ontologies/2022/6/geological_taxonomy#Sedimentary_rocks"/>
        <rdfs:comment>A sedimentary rock formed from clay

Resource: https://geology.fandom.com/wiki/List_of_rock_types</rdfs:comment>
    </owl:Class>
    


    <!-- http://www.semanticweb.org/ontologies/2022/6/geological_taxonomy#Cloudy -->

    <owl:Class rdf:about="http://www.semanticweb.org/ontologies/2022/6/geological_taxonomy#Cloudy">
        <rdfs:subClassOf rdf:resource="http://www.semanticweb.org/ontologies/2022/6/geological_taxonomy#Weather_conditions"/>
        <rdfs:comment>Cloudy weather is when a significant amount of clouds is covering the sky (at least half the sky).

Resource: https://weather.fandom.com/wiki/Types_of_Weather#Cloudy

Justification: Classified based on the covering of sky by clouds</rdfs:comment>
    </owl:Class>
    


    <!-- http://www.semanticweb.org/ontologies/2022/6/geological_taxonomy#Coal -->

    <owl:Class rdf:about="http://www.semanticweb.org/ontologies/2022/6/geological_taxonomy#Coal">
        <rdfs:subClassOf rdf:resource="http://www.semanticweb.org/ontologies/2022/6/geological_taxonomy#Sedimentary_rocks"/>
        <rdfs:comment>A sedimentary rock formed from organic matter

Resource: https://geology.fandom.com/wiki/List_of_rock_types</rdfs:comment>
    </owl:Class>
    


    <!-- http://www.semanticweb.org/ontologies/2022/6/geological_taxonomy#Coastal_Flood -->

    <owl:Class rdf:about="http://www.semanticweb.org/ontologies/2022/6/geological_taxonomy#Coastal_Flood">
        <rdfs:subClassOf rdf:resource="http://www.semanticweb.org/ontologies/2022/6/geological_taxonomy#Flood"/>
        <rdfs:comment>Coastal flooding normally occurs when dry and low-lying land is submerged by seawater.

Resource: https://en.wikipedia.org/wiki/Coastal_flooding

Justification: Classified based on how seawater enters the land</rdfs:comment>
    </owl:Class>
    


    <!-- http://www.semanticweb.org/ontologies/2022/6/geological_taxonomy#Cold_wave -->

    <owl:Class rdf:about="http://www.semanticweb.org/ontologies/2022/6/geological_taxonomy#Cold_wave">
        <rdfs:subClassOf rdf:resource="http://www.semanticweb.org/ontologies/2022/6/geological_taxonomy#Extreme_Temperature"/>
        <owl:disjointWith rdf:resource="http://www.semanticweb.org/ontologies/2022/6/geological_taxonomy#Heat_wave"/>
        <rdfs:comment>A period of abnormally cold weather.

Resource: http://desinventar.cimafoundation.org/definitions.html</rdfs:comment>
    </owl:Class>
    


    <!-- http://www.semanticweb.org/ontologies/2022/6/geological_taxonomy#Collapse_Earthquake -->

    <owl:Class rdf:about="http://www.semanticweb.org/ontologies/2022/6/geological_taxonomy#Collapse_Earthquake">
        <rdfs:subClassOf rdf:resource="http://www.semanticweb.org/ontologies/2022/6/geological_taxonomy#Earthquake"/>
        <rdfs:comment>A collapse earthquake are small earthquakes in underground caverns and mines that are caused by seismic waves produced from the explosion of rock on the surface.

Resource: https://www.un-spider.org/category/disaster-type/earthquake</rdfs:comment>
    </owl:Class>
    


    <!-- http://www.semanticweb.org/ontologies/2022/6/geological_taxonomy#Comendite -->

    <owl:Class rdf:about="http://www.semanticweb.org/ontologies/2022/6/geological_taxonomy#Comendite">
        <rdfs:subClassOf rdf:resource="http://www.semanticweb.org/ontologies/2022/6/geological_taxonomy#Rhyolite"/>
        <owl:disjointWith rdf:resource="http://www.semanticweb.org/ontologies/2022/6/geological_taxonomy#Pantellerite"/>
        <rdfs:comment>Hard, peralkaline igneous rock, a type of light blue grey rhyolite

Resource: https://en.wikipedia.org/wiki/List_of_rock_types</rdfs:comment>
    </owl:Class>
    


    <!-- http://www.semanticweb.org/ontologies/2022/6/geological_taxonomy#Conglomerate -->

    <owl:Class rdf:about="http://www.semanticweb.org/ontologies/2022/6/geological_taxonomy#Conglomerate">
        <rdfs:subClassOf rdf:resource="http://www.semanticweb.org/ontologies/2022/6/geological_taxonomy#Sedimentary_rocks"/>
        <rdfs:comment>A sedimentary rock composed of large rounded fragments of other rocks

Resource: https://geology.fandom.com/wiki/List_of_rock_types

Justification: Depending upon the method of deposition.</rdfs:comment>
    </owl:Class>
    


    <!-- http://www.semanticweb.org/ontologies/2022/6/geological_taxonomy#Continental_crust -->

    <owl:Class rdf:about="http://www.semanticweb.org/ontologies/2022/6/geological_taxonomy#Continental_crust">
        <rdfs:subClassOf rdf:resource="http://www.semanticweb.org/ontologies/2022/6/geological_taxonomy#Crust"/>
        <owl:disjointWith rdf:resource="http://www.semanticweb.org/ontologies/2022/6/geological_taxonomy#Oceanic_crust"/>
        <rdfs:comment>layer of rocks that forms the continents and the areas of shallow seabed close to their shores, known as continental shelves, is less dense and composed of (felsic) sodium potassium aluminium silicate rocks, like granite.

Resource: https://en.wikipedia.org/wiki/Continental_crust</rdfs:comment>
    </owl:Class>
    


    <!-- http://www.semanticweb.org/ontologies/2022/6/geological_taxonomy#Continental_lithosphere -->

    <owl:Class rdf:about="http://www.semanticweb.org/ontologies/2022/6/geological_taxonomy#Continental_lithosphere">
        <rdfs:subClassOf rdf:resource="http://www.semanticweb.org/ontologies/2022/6/geological_taxonomy#Lithosphere"/>
        <owl:disjointWith rdf:resource="http://www.semanticweb.org/ontologies/2022/6/geological_taxonomy#Oceanic_lithosphere"/>
        <rdfs:comment>Continental lithosphere is associated with continental crust and underlies the continents and continental shelfs.

Resource: https://en.wikipedia.org/wiki/Lithosphere</rdfs:comment>
    </owl:Class>
    


    <!-- http://www.semanticweb.org/ontologies/2022/6/geological_taxonomy#Continuous_creep -->

    <owl:Class rdf:about="http://www.semanticweb.org/ontologies/2022/6/geological_taxonomy#Continuous_creep">
        <rdfs:subClassOf rdf:resource="http://www.semanticweb.org/ontologies/2022/6/geological_taxonomy#Creep"/>
        <rdfs:comment>Shear stress continuously exceeds the strength of the material(rock debris and soil)

Resource: https://www.nature.scot/landforms-and-geology/scotlands-rocks-landforms-and-soils/landforms/landslides/types-landslide
https://courses.lumenlearning.com/geo/chapter/reading-slump-and-creep/</rdfs:comment>
    </owl:Class>
    


    <!-- http://www.semanticweb.org/ontologies/2022/6/geological_taxonomy#Coquina -->

    <owl:Class rdf:about="http://www.semanticweb.org/ontologies/2022/6/geological_taxonomy#Coquina">
        <rdfs:subClassOf rdf:resource="http://www.semanticweb.org/ontologies/2022/6/geological_taxonomy#Sedimentary_rocks"/>
        <rdfs:comment>A sedimentary carbonate rock formed by accumulation of abundant shell fossils and fragments

Resource: https://geology.fandom.com/wiki/List_of_rock_types</rdfs:comment>
    </owl:Class>
    


    <!-- http://www.semanticweb.org/ontologies/2022/6/geological_taxonomy#Creep -->

    <owl:Class rdf:about="http://www.semanticweb.org/ontologies/2022/6/geological_taxonomy#Creep">
        <rdfs:subClassOf rdf:resource="http://www.semanticweb.org/ontologies/2022/6/geological_taxonomy#Flow"/>
        <owl:disjointWith rdf:resource="http://www.semanticweb.org/ontologies/2022/6/geological_taxonomy#Lateral_Spread"/>
        <rdfs:comment>slow downslope movement of particles that occurs on every slope covered with loose, weathered material.

Resource: https://www.britannica.com/science/creep-slope-movement

Justification: Classification based on the effects of seasonal changes, gravitational force, point of failure</rdfs:comment>
    </owl:Class>
    


    <!-- http://www.semanticweb.org/ontologies/2022/6/geological_taxonomy#Crown_Fire -->

    <owl:Class rdf:about="http://www.semanticweb.org/ontologies/2022/6/geological_taxonomy#Crown_Fire">
        <rdfs:subClassOf rdf:resource="http://www.semanticweb.org/ontologies/2022/6/geological_taxonomy#Wildfire"/>
        <rdfs:comment>These fires burn and spread from treetop to treetop. spread at a rapid pace.	

Resource: https://www.supplycache.com/blogs/news/the-different-types-of-wildland-fires</rdfs:comment>
    </owl:Class>
    


    <!-- http://www.semanticweb.org/ontologies/2022/6/geological_taxonomy#Crust -->

    <owl:Class rdf:about="http://www.semanticweb.org/ontologies/2022/6/geological_taxonomy#Crust">
        <rdfs:subClassOf rdf:resource="http://www.semanticweb.org/ontologies/2022/6/geological_taxonomy#Units_of_Earth_structure"/>
        <rdfs:comment>outermost solid shell of a rocky planet, dwarf planet or natural satellite, which is chemically distinct from the underlying mantle

Resource: https://en.wikipedia.org/wiki/Crust_(geology)

Justification: depending on composition of density, different rocks</rdfs:comment>
    </owl:Class>
    


    <!-- http://www.semanticweb.org/ontologies/2022/6/geological_taxonomy#Cryalfs -->

    <owl:Class rdf:about="http://www.semanticweb.org/ontologies/2022/6/geological_taxonomy#Cryalfs">
        <rdfs:subClassOf rdf:resource="http://www.semanticweb.org/ontologies/2022/6/geological_taxonomy#Alfisols"/>
        <rdfs:comment>Alfisols that have a cryic or isofrigid temperature regime. 

Resource: https://sites.google.com/site/dinpuithai/Home/taxonomy/j-alfisols</rdfs:comment>
    </owl:Class>
    


    <!-- http://www.semanticweb.org/ontologies/2022/6/geological_taxonomy#Cryands -->

    <owl:Class rdf:about="http://www.semanticweb.org/ontologies/2022/6/geological_taxonomy#Cryands">
        <rdfs:subClassOf rdf:resource="http://www.semanticweb.org/ontologies/2022/6/geological_taxonomy#Andisols"/>
        <rdfs:comment>Andisols that have a cryic soil temperature regime.


Resource: https://sites.google.com/site/dinpuithai/Home/key10/key10d</rdfs:comment>
    </owl:Class>
    


    <!-- http://www.semanticweb.org/ontologies/2022/6/geological_taxonomy#Cryepts -->

    <owl:Class rdf:about="http://www.semanticweb.org/ontologies/2022/6/geological_taxonomy#Cryepts">
        <rdfs:subClassOf rdf:resource="http://www.semanticweb.org/ontologies/2022/6/geological_taxonomy#Inceptisols"/>
        <rdfs:comment>Inceptisols that have a cryic soil temperature regime.

Resource: https://sites.google.com/site/dinpuithai/Home/key10/key10k</rdfs:comment>
    </owl:Class>
    


    <!-- http://www.semanticweb.org/ontologies/2022/6/geological_taxonomy#Cryerts -->

    <owl:Class rdf:about="http://www.semanticweb.org/ontologies/2022/6/geological_taxonomy#Cryerts">
        <rdfs:subClassOf rdf:resource="http://www.semanticweb.org/ontologies/2022/6/geological_taxonomy#Vertisols"/>
        <rdfs:comment>Vertisols that have a cryic soil temperature regime

Resource: https://sites.google.com/site/dinpuithai/Home/key10/key10f</rdfs:comment>
    </owl:Class>
    


    <!-- http://www.semanticweb.org/ontologies/2022/6/geological_taxonomy#Cryids -->

    <owl:Class rdf:about="http://www.semanticweb.org/ontologies/2022/6/geological_taxonomy#Cryids">
        <rdfs:subClassOf rdf:resource="http://www.semanticweb.org/ontologies/2022/6/geological_taxonomy#Aridisols"/>
        <rdfs:comment>Aridisols that have a cryic soil temperature regime

Resource: https://sites.google.com/site/dinpuithai/Home/key10/key10g</rdfs:comment>
    </owl:Class>
    


    <!-- http://www.semanticweb.org/ontologies/2022/6/geological_taxonomy#Cryods -->

    <owl:Class rdf:about="http://www.semanticweb.org/ontologies/2022/6/geological_taxonomy#Cryods">
        <rdfs:subClassOf rdf:resource="http://www.semanticweb.org/ontologies/2022/6/geological_taxonomy#Spodosols"/>
        <rdfs:comment>Cold Spodosols (cryic temperature regime)

Resource: &quot;Illustrated Guide to Soil Taxonomy&quot; book by Unites States Department of Agriculture</rdfs:comment>
    </owl:Class>
    


    <!-- http://www.semanticweb.org/ontologies/2022/6/geological_taxonomy#Cryolls -->

    <owl:Class rdf:about="http://www.semanticweb.org/ontologies/2022/6/geological_taxonomy#Cryolls">
        <rdfs:subClassOf rdf:resource="http://www.semanticweb.org/ontologies/2022/6/geological_taxonomy#Mollisols"/>
        <rdfs:comment>Cryolls have a frigid, cryic, or pergelic Soil temperature regimes

Resource: https://www.sciencedirect.com/topics/agricultural-and-biological-sciences/mollisol</rdfs:comment>
    </owl:Class>
    


    <!-- http://www.semanticweb.org/ontologies/2022/6/geological_taxonomy#Cyclone -->

    <owl:Class rdf:about="http://www.semanticweb.org/ontologies/2022/6/geological_taxonomy#Cyclone">
        <rdfs:subClassOf rdf:resource="http://www.semanticweb.org/ontologies/2022/6/geological_taxonomy#Natural_disaster"/>
        <rdfs:comment>Cyclone is a large air mass that rotates around a strong center of low atmospheric pressure

Resource: https://en.wikipedia.org/wiki/Cyclone

Justification: depending upon where it originates, affecting size of area</rdfs:comment>
    </owl:Class>
    


    <!-- http://www.semanticweb.org/ontologies/2022/6/geological_taxonomy#Dacite -->

    <owl:Class rdf:about="http://www.semanticweb.org/ontologies/2022/6/geological_taxonomy#Dacite">
        <rdfs:subClassOf rdf:resource="http://www.semanticweb.org/ontologies/2022/6/geological_taxonomy#Igneous_rocks"/>
        <rdfs:comment>A felsic to intermediate volcanic rock with high iron content

Resource: https://geology.fandom.com/wiki/Dacite</rdfs:comment>
    </owl:Class>
    


    <!-- http://www.semanticweb.org/ontologies/2022/6/geological_taxonomy#Debris_fall -->

    <owl:Class rdf:about="http://www.semanticweb.org/ontologies/2022/6/geological_taxonomy#Debris_fall">
        <rdfs:subClassOf rdf:resource="http://www.semanticweb.org/ontologies/2022/6/geological_taxonomy#Fall"/>
        <owl:disjointWith rdf:resource="http://www.semanticweb.org/ontologies/2022/6/geological_taxonomy#Rockfall"/>
        <rdfs:comment>A relatively free downward or forward falling of unconsolidated or poorly consolidated earth or rocky debris from a cliff, cave, or arch

Resource: https://encyclopedia2.thefreedictionary.com/debris+fall</rdfs:comment>
    </owl:Class>
    


    <!-- http://www.semanticweb.org/ontologies/2022/6/geological_taxonomy#Debris_slide -->

    <owl:Class rdf:about="http://www.semanticweb.org/ontologies/2022/6/geological_taxonomy#Debris_slide">
        <rdfs:subClassOf rdf:resource="http://www.semanticweb.org/ontologies/2022/6/geological_taxonomy#Block_slide"/>
        <owl:disjointWith rdf:resource="http://www.semanticweb.org/ontologies/2022/6/geological_taxonomy#Rock_slide"/>
        <rdfs:comment>If debris slide down a slope on a distinct shear plane, the movements are called debris slides.

Resource: http://www.wrds.uwyo.edu/wrds/wsgs/hazards/landslides/classscheme.htm</rdfs:comment>
    </owl:Class>
    


    <!-- http://www.semanticweb.org/ontologies/2022/6/geological_taxonomy#Debris_topple -->

    <owl:Class rdf:about="http://www.semanticweb.org/ontologies/2022/6/geological_taxonomy#Debris_topple">
        <rdfs:subClassOf rdf:resource="http://www.semanticweb.org/ontologies/2022/6/geological_taxonomy#Topple"/>
        <owl:disjointWith rdf:resource="http://www.semanticweb.org/ontologies/2022/6/geological_taxonomy#Rock_topple"/>
        <rdfs:comment>Topples in which debris are the material type

Resource: https://en.wikipedia.org/wiki/Landslide_classification#Types_and_classification</rdfs:comment>
    </owl:Class>
    


    <!-- http://www.semanticweb.org/ontologies/2022/6/geological_taxonomy#Diabase -->

    <owl:Class rdf:about="http://www.semanticweb.org/ontologies/2022/6/geological_taxonomy#Diabase">
        <rdfs:subClassOf rdf:resource="http://www.semanticweb.org/ontologies/2022/6/geological_taxonomy#Igneous_rocks"/>
        <rdfs:comment>Diabase, also called dolerite or microgabbro, is a mafic, holocrystalline, subvolcanic rock equivalent to volcanic basalt or plutonic gabbro.

Resource: https://en.wikipedia.org/wiki/Diabase</rdfs:comment>
    </owl:Class>
    


    <!-- http://www.semanticweb.org/ontologies/2022/6/geological_taxonomy#Diamictite -->

    <owl:Class rdf:about="http://www.semanticweb.org/ontologies/2022/6/geological_taxonomy#Diamictite">
        <rdfs:subClassOf rdf:resource="http://www.semanticweb.org/ontologies/2022/6/geological_taxonomy#Conglomerate"/>
        <rdfs:comment>Diamictite is a poorly sorted or non-sorted terrigenous non-calcareous sedimentary rock.

Resource: https://www.sandatlas.org/rock-types/#Diamictite</rdfs:comment>
    </owl:Class>
    


    <!-- http://www.semanticweb.org/ontologies/2022/6/geological_taxonomy#Diatomite -->

    <owl:Class rdf:about="http://www.semanticweb.org/ontologies/2022/6/geological_taxonomy#Diatomite">
        <rdfs:subClassOf rdf:resource="http://www.semanticweb.org/ontologies/2022/6/geological_taxonomy#Sedimentary_rocks"/>
        <rdfs:comment>A sedimentary rock formed from diatom fossils

Resource: https://geology.fandom.com/wiki/List_of_rock_types</rdfs:comment>
    </owl:Class>
    


    <!-- http://www.semanticweb.org/ontologies/2022/6/geological_taxonomy#Diorite -->

    <owl:Class rdf:about="http://www.semanticweb.org/ontologies/2022/6/geological_taxonomy#Diorite">
        <rdfs:subClassOf rdf:resource="http://www.semanticweb.org/ontologies/2022/6/geological_taxonomy#Igneous_rocks"/>
        <rdfs:comment>Diorite is an intrusive igneous rock formed by the slow cooling underground of magma that has a moderate content of silica and a relatively low content of alkali metals.

Resource: https://en.wikipedia.org/wiki/Diorite

Justification: Based on presence of orbicular structure</rdfs:comment>
    </owl:Class>
    


    <!-- http://www.semanticweb.org/ontologies/2022/6/geological_taxonomy#Direct_flooding -->

    <owl:Class rdf:about="http://www.semanticweb.org/ontologies/2022/6/geological_taxonomy#Direct_flooding">
        <rdfs:subClassOf rdf:resource="http://www.semanticweb.org/ontologies/2022/6/geological_taxonomy#Coastal_Flood"/>
        <rdfs:comment>where the sea height exceeds the elevation of the land, often where waves have not built up a natural barrier such as a dune	

Resource: https://en.wikipedia.org/wiki/Coastal_flooding</rdfs:comment>
    </owl:Class>
    


    <!-- http://www.semanticweb.org/ontologies/2022/6/geological_taxonomy#Dolomite -->

    <owl:Class rdf:about="http://www.semanticweb.org/ontologies/2022/6/geological_taxonomy#Dolomite">
        <rdfs:subClassOf rdf:resource="http://www.semanticweb.org/ontologies/2022/6/geological_taxonomy#Sedimentary_rocks"/>
    </owl:Class>
    


    <!-- http://www.semanticweb.org/ontologies/2022/6/geological_taxonomy#Drought -->

    <owl:Class rdf:about="http://www.semanticweb.org/ontologies/2022/6/geological_taxonomy#Drought">
        <rdfs:subClassOf rdf:resource="http://www.semanticweb.org/ontologies/2022/6/geological_taxonomy#Natural_disaster"/>
        <rdfs:comment>A drought is an event of prolonged shortages in the water supply, whether atmospheric (below-average precipitation), surface water or ground water.	

Resource: https://en.wikipedia.org/wiki/Drought

Justification: Classified based Palmer Drought Severity Index(PDSI)
https://droughtmonitor.unl.edu/About/WhatistheUSDM.aspx</rdfs:comment>
    </owl:Class>
    


    <!-- http://www.semanticweb.org/ontologies/2022/6/geological_taxonomy#Dunite -->

    <owl:Class rdf:about="http://www.semanticweb.org/ontologies/2022/6/geological_taxonomy#Dunite">
        <rdfs:subClassOf rdf:resource="http://www.semanticweb.org/ontologies/2022/6/geological_taxonomy#Igneous_rocks"/>
        <rdfs:comment>Dunite, also known as olivinite, is an intrusive igneous rock of ultramafic composition and with phaneritic (coarse-grained) texture.

Resource: https://en.wikipedia.org/wiki/Dunite</rdfs:comment>
    </owl:Class>
    


    <!-- http://www.semanticweb.org/ontologies/2022/6/geological_taxonomy#Durids -->

    <owl:Class rdf:about="http://www.semanticweb.org/ontologies/2022/6/geological_taxonomy#Durids">
        <rdfs:subClassOf rdf:resource="http://www.semanticweb.org/ontologies/2022/6/geological_taxonomy#Aridisols"/>
        <rdfs:comment>Characterized by accumulations of silica, but infrequently found; associated with soils formed from volcanic materials. 

Resource: https://www.sciencedirect.com/topics/agricultural-and-biological-sciences/aridisol</rdfs:comment>
    </owl:Class>
    


    <!-- http://www.semanticweb.org/ontologies/2022/6/geological_taxonomy#Earthquake -->

    <owl:Class rdf:about="http://www.semanticweb.org/ontologies/2022/6/geological_taxonomy#Earthquake">
        <rdfs:subClassOf rdf:resource="http://www.semanticweb.org/ontologies/2022/6/geological_taxonomy#Natural_disaster"/>
        <rdfs:comment>shaking of the surface of the Earth resulting from a sudden release of energy in the Earth&apos;s lithosphere that creates seismic waves.

Resource: https://en.wikipedia.org/wiki/Earthquake

Justification: Classified based on the origin of earthquake process</rdfs:comment>
    </owl:Class>
    


    <!-- http://www.semanticweb.org/ontologies/2022/6/geological_taxonomy#Eclogite -->

    <owl:Class rdf:about="http://www.semanticweb.org/ontologies/2022/6/geological_taxonomy#Eclogite">
        <rdfs:subClassOf rdf:resource="http://www.semanticweb.org/ontologies/2022/6/geological_taxonomy#Metamorphic_rocks"/>
        <rdfs:comment>An ultra-high grade metamorphosed basalt or gabbro; also a facies of metamorphic rocks

Resource: https://geology.fandom.com/wiki/List_of_rock_types</rdfs:comment>
    </owl:Class>
    


    <!-- http://www.semanticweb.org/ontologies/2022/6/geological_taxonomy#Elements -->

    <owl:Class rdf:about="http://www.semanticweb.org/ontologies/2022/6/geological_taxonomy#Elements">
        <rdfs:subClassOf rdf:resource="http://www.semanticweb.org/ontologies/2022/6/geological_taxonomy#Mineral"/>
        <rdfs:comment>Native element minerals are those elements that occur in nature in uncombined form with a distinct mineral structure.	

Resource: https://en.wikipedia.org/wiki/Native_element_mineral

Justification: Classified based on physical characters and chemical relations
https://www.911metallurgist.com/blog/descriptive-mineralogy-classification</rdfs:comment>
    </owl:Class>
    


    <!-- http://www.semanticweb.org/ontologies/2022/6/geological_taxonomy#Enderbite -->

    <owl:Class rdf:about="http://www.semanticweb.org/ontologies/2022/6/geological_taxonomy#Enderbite">
        <rdfs:subClassOf rdf:resource="http://www.semanticweb.org/ontologies/2022/6/geological_taxonomy#Charnockite"/>
        <rdfs:comment>Enderbite is an igneous rock of the charnockite series, consisting essentially of quartz, antiperthite (or perthite), orthopyroxene (usually hypersthene) and magnetite, and is equivalent to an orthopyroxene bearing tonalite.

Resource: https://en.wikipedia.org/wiki/Enderbite</rdfs:comment>
    </owl:Class>
    


    <!-- http://www.semanticweb.org/ontologies/2022/6/geological_taxonomy#Entisols -->

    <owl:Class rdf:about="http://www.semanticweb.org/ontologies/2022/6/geological_taxonomy#Entisols">
        <rdfs:subClassOf rdf:resource="http://www.semanticweb.org/ontologies/2022/6/geological_taxonomy#Soil"/>
        <rdfs:comment>The central concept of Entisols is that of soils that have little or no evidence of development of pedogenic horizons. 

Resource: https://www.nrcs.usda.gov/wps/portal/nrcs/detail/soils/survey/class/maps/?cid=nrcs142p2_053596

Justification: Divided between  near surface saturation; sandy texture; formation in recent stratified alluvial sediments; and a virtual lack of horizon formation, mostly in areas of young erosional surfaces.
&quot;Illustrated Guide to Soil Taxonomy&quot; book by Unites States Department of Agriculture</rdfs:comment>
    </owl:Class>
    


    <!-- http://www.semanticweb.org/ontologies/2022/6/geological_taxonomy#Epidosite -->

    <owl:Class rdf:about="http://www.semanticweb.org/ontologies/2022/6/geological_taxonomy#Epidosite">
        <rdfs:subClassOf rdf:resource="http://www.semanticweb.org/ontologies/2022/6/geological_taxonomy#Metamorphic_rocks"/>
        <rdfs:comment>Epidosite is a metamorphic rock consisting of epidote and quartz. This rock type is a product of hydrothermal metamorphism.

Resource: https://www.sandatlas.org/epidosite/</rdfs:comment>
    </owl:Class>
    


    <!-- http://www.semanticweb.org/ontologies/2022/6/geological_taxonomy#Essexite -->

    <owl:Class rdf:about="http://www.semanticweb.org/ontologies/2022/6/geological_taxonomy#Essexite">
        <rdfs:subClassOf rdf:resource="http://www.semanticweb.org/ontologies/2022/6/geological_taxonomy#Igneous_rocks"/>
        <rdfs:comment>Essexite, also called nepheline monzogabbro, is a dark gray or black holocrystalline plutonic igneous rock.

Resource: https://en.wikipedia.org/wiki/Essexite</rdfs:comment>
    </owl:Class>
    


    <!-- http://www.semanticweb.org/ontologies/2022/6/geological_taxonomy#Evaporite -->

    <owl:Class rdf:about="http://www.semanticweb.org/ontologies/2022/6/geological_taxonomy#Evaporite">
        <rdfs:subClassOf rdf:resource="http://www.semanticweb.org/ontologies/2022/6/geological_taxonomy#Sedimentary_rocks"/>
        <rdfs:comment>A chemical sedimentary rock formed by accumulation of minerals after evaporation

Resource: https://geology.fandom.com/wiki/List_of_rock_types</rdfs:comment>
    </owl:Class>
    


    <!-- http://www.semanticweb.org/ontologies/2022/6/geological_taxonomy#Exceptional_Drought -->

    <owl:Class rdf:about="http://www.semanticweb.org/ontologies/2022/6/geological_taxonomy#Exceptional_Drought">
        <rdfs:subClassOf rdf:resource="http://www.semanticweb.org/ontologies/2022/6/geological_taxonomy#Drought"/>
        <rdfs:comment>It is D4 category and causes exceptional crop/pasture losses and shortages of water in reservoirs, streams, and wells creating water emergencies.

Resource: https://droughtmonitor.unl.edu/About/WhatistheUSDM.aspx</rdfs:comment>
    </owl:Class>
    


    <!-- http://www.semanticweb.org/ontologies/2022/6/geological_taxonomy#Explosion_Earthquake -->

    <owl:Class rdf:about="http://www.semanticweb.org/ontologies/2022/6/geological_taxonomy#Explosion_Earthquake">
        <rdfs:subClassOf rdf:resource="http://www.semanticweb.org/ontologies/2022/6/geological_taxonomy#Earthquake"/>
        <rdfs:comment>Man triggered kind of earthquakes and represent the biggest impact of modern-day nuclear war.

Resource: https://www.conserve-energy-future.com/howearthquakesoccur.php</rdfs:comment>
    </owl:Class>
    


    <!-- http://www.semanticweb.org/ontologies/2022/6/geological_taxonomy#Extratropical_cyclone -->

    <owl:Class rdf:about="http://www.semanticweb.org/ontologies/2022/6/geological_taxonomy#Extratropical_cyclone">
        <rdfs:subClassOf rdf:resource="http://www.semanticweb.org/ontologies/2022/6/geological_taxonomy#Cyclone"/>
        <owl:disjointWith rdf:resource="http://www.semanticweb.org/ontologies/2022/6/geological_taxonomy#Tropical_cyclone"/>
        <rdfs:comment>Extratropical cyclones cover and affects a larger area and can originate over the land and sea.

Resource: https://www.insightsonindia.com/world-geography/physical-geography-of-the-world/climatology/cyclones-and-anticyclones/difference-between-extratropical-and-tropical-cyclones/#:~:text=Extratropical%20cyclones%20cover%20a%20larger,compared%20to%20the%20tropical%20cyclone.

Justification: depending upon direction of winds</rdfs:comment>
    </owl:Class>
    


    <!-- http://www.semanticweb.org/ontologies/2022/6/geological_taxonomy#Extreme_Drought -->

    <owl:Class rdf:about="http://www.semanticweb.org/ontologies/2022/6/geological_taxonomy#Extreme_Drought">
        <rdfs:subClassOf rdf:resource="http://www.semanticweb.org/ontologies/2022/6/geological_taxonomy#Drought"/>
        <rdfs:comment>It is D3 category and causes major crop/pasture losses.

Resource: https://droughtmonitor.unl.edu/About/WhatistheUSDM.aspx</rdfs:comment>
    </owl:Class>
    


    <!-- http://www.semanticweb.org/ontologies/2022/6/geological_taxonomy#Extreme_Temperature -->

    <owl:Class rdf:about="http://www.semanticweb.org/ontologies/2022/6/geological_taxonomy#Extreme_Temperature">
        <rdfs:subClassOf rdf:resource="http://www.semanticweb.org/ontologies/2022/6/geological_taxonomy#Natural_disaster"/>
        <rdfs:comment>A general term for temperature variations above (extreme heat) or below (extreme cold) normal conditions.

Resource: http://desinventar.cimafoundation.org/definitions.html

Justification: Classified based on temperature</rdfs:comment>
    </owl:Class>
    


    <!-- http://www.semanticweb.org/ontologies/2022/6/geological_taxonomy#Fall -->

    <owl:Class rdf:about="http://www.semanticweb.org/ontologies/2022/6/geological_taxonomy#Fall">
        <rdfs:subClassOf rdf:resource="http://www.semanticweb.org/ontologies/2022/6/geological_taxonomy#Landslide"/>
        <rdfs:comment>Detachment of soil or rock from a steep slope along a surface on which little or no shear displacement takes place.

Resource: https://en.wikipedia.org/wiki/Landslide_classification#Types_and_classification

Justification: Divided based on type of material</rdfs:comment>
    </owl:Class>
    


    <!-- http://www.semanticweb.org/ontologies/2022/6/geological_taxonomy#Fenite -->

    <owl:Class rdf:about="http://www.semanticweb.org/ontologies/2022/6/geological_taxonomy#Fenite">
        <rdfs:subClassOf rdf:resource="http://www.semanticweb.org/ontologies/2022/6/geological_taxonomy#Metamorphic_rocks"/>
        <rdfs:comment>Fenite is a metasomatic alteration associated particularly with carbonatite intrusions and created, very rarely, by advanced carbon dioxide alteration (carbonation) of felsic and mafic rocks.

Resource: https://en.wikipedia.org/wiki/Fenite</rdfs:comment>
    </owl:Class>
    


    <!-- http://www.semanticweb.org/ontologies/2022/6/geological_taxonomy#Fibrists -->

    <owl:Class rdf:about="http://www.semanticweb.org/ontologies/2022/6/geological_taxonomy#Fibrists">
        <rdfs:subClassOf rdf:resource="http://www.semanticweb.org/ontologies/2022/6/geological_taxonomy#Histosols"/>
        <rdfs:comment>Histosols that are primarily made up of only slightly decomposed organic materials, often called peat.

Resource: https://en.wikipedia.org/wiki/Histosol</rdfs:comment>
    </owl:Class>
    


    <!-- http://www.semanticweb.org/ontologies/2022/6/geological_taxonomy#Flash_flood -->

    <owl:Class rdf:about="http://www.semanticweb.org/ontologies/2022/6/geological_taxonomy#Flash_flood">
        <rdfs:subClassOf rdf:resource="http://www.semanticweb.org/ontologies/2022/6/geological_taxonomy#Flood"/>
        <rdfs:comment>A flash flood is a rapid flooding of low-lying areas: washes, rivers, dry lakes and depressions.	

Resource: https://en.wikipedia.org/wiki/Flash_flood</rdfs:comment>
    </owl:Class>
    


    <!-- http://www.semanticweb.org/ontologies/2022/6/geological_taxonomy#Flint -->

    <owl:Class rdf:about="http://www.semanticweb.org/ontologies/2022/6/geological_taxonomy#Flint">
        <rdfs:subClassOf rdf:resource="http://www.semanticweb.org/ontologies/2022/6/geological_taxonomy#Sedimentary_rocks"/>
        <rdfs:comment>Flint is a sedimentary cryptocrystalline form of the mineral quartz,[1][2] categorized as the variety of chert that occurs in chalk or marly limestone.

Resource: https://en.wikipedia.org/wiki/Flint</rdfs:comment>
    </owl:Class>
    


    <!-- http://www.semanticweb.org/ontologies/2022/6/geological_taxonomy#Flood -->

    <owl:Class rdf:about="http://www.semanticweb.org/ontologies/2022/6/geological_taxonomy#Flood">
        <rdfs:subClassOf rdf:resource="http://www.semanticweb.org/ontologies/2022/6/geological_taxonomy#Natural_disaster"/>
        <rdfs:comment>A flood is an overflow of water that submerges land that is usually dry.	

Resource: https://en.wikipedia.org/wiki/Flood

Justification: Depending upon the area affected</rdfs:comment>
    </owl:Class>
    


    <!-- http://www.semanticweb.org/ontologies/2022/6/geological_taxonomy#Flow -->

    <owl:Class rdf:about="http://www.semanticweb.org/ontologies/2022/6/geological_taxonomy#Flow">
        <rdfs:subClassOf rdf:resource="http://www.semanticweb.org/ontologies/2022/6/geological_taxonomy#Landslide"/>
        <rdfs:comment>A flow is a spatially continuous movement in which surfaces of shear are short-lived, closely spaced, and usually not preserved.

Resource: https://en.wikipedia.org/wiki/Landslide_classification

Justification: Classified based on the speed of the material flowing
https://geology.com/usgs/landslides/#flows</rdfs:comment>
    </owl:Class>
    


    <!-- http://www.semanticweb.org/ontologies/2022/6/geological_taxonomy#Fluvents -->

    <owl:Class rdf:about="http://www.semanticweb.org/ontologies/2022/6/geological_taxonomy#Fluvents">
        <rdfs:subClassOf rdf:resource="http://www.semanticweb.org/ontologies/2022/6/geological_taxonomy#Entisols"/>
        <rdfs:comment>Entisols that formed in stratified alluvial sediments as evidenced
by the irregular decrease/increase of carbon content with increasing depth

Resource: &quot;Illustrated Guide to Soil Taxonomy&quot; book by Unites States Department of Agriculture</rdfs:comment>
    </owl:Class>
    


    <!-- http://www.semanticweb.org/ontologies/2022/6/geological_taxonomy#Fog -->

    <owl:Class rdf:about="http://www.semanticweb.org/ontologies/2022/6/geological_taxonomy#Fog">
        <rdfs:subClassOf rdf:resource="http://www.semanticweb.org/ontologies/2022/6/geological_taxonomy#Weather_conditions"/>
        <rdfs:comment>Fog is literally a cloud at ground level, which raises ambient humidity to its maximum, and considerably decreases visibility.

Resource: https://weather.fandom.com/wiki/Types_of_Weather#Fog</rdfs:comment>
    </owl:Class>
    


    <!-- http://www.semanticweb.org/ontologies/2022/6/geological_taxonomy#Foidolite -->

    <owl:Class rdf:about="http://www.semanticweb.org/ontologies/2022/6/geological_taxonomy#Foidolite">
        <rdfs:subClassOf rdf:resource="http://www.semanticweb.org/ontologies/2022/6/geological_taxonomy#Igneous_rocks"/>
        <rdfs:comment>Foidolite is a rare phaneritic (coarse-grained) intrusive igneous rock in which more than 60% of light-coloured minerals are feldspathoids.

Resource: https://en.wikipedia.org/wiki/Foidolite</rdfs:comment>
    </owl:Class>
    


    <!-- http://www.semanticweb.org/ontologies/2022/6/geological_taxonomy#Folists -->

    <owl:Class rdf:about="http://www.semanticweb.org/ontologies/2022/6/geological_taxonomy#Folists">
        <rdfs:subClassOf rdf:resource="http://www.semanticweb.org/ontologies/2022/6/geological_taxonomy#Histosols"/>
        <rdfs:comment>Histosols that are not saturated with water for long periods of time during the year.

Resource: https://en.wikipedia.org/wiki/Histosol</rdfs:comment>
    </owl:Class>
    


    <!-- http://www.semanticweb.org/ontologies/2022/6/geological_taxonomy#Foyaite -->

    <owl:Class rdf:about="http://www.semanticweb.org/ontologies/2022/6/geological_taxonomy#Foyaite">
        <rdfs:subClassOf rdf:resource="http://www.semanticweb.org/ontologies/2022/6/geological_taxonomy#Igneous_rocks"/>
        <rdfs:comment>Foyaite is a rare igneous rock consisting of nepheline and alkali feldspar with a trachytic texture. Foyaite is a variety of nepheline syenite.

Resource: https://www.sandatlas.org/rock-types/#Foyaite</rdfs:comment>
    </owl:Class>
    


    <!-- http://www.semanticweb.org/ontologies/2022/6/geological_taxonomy#Gabbro -->

    <owl:Class rdf:about="http://www.semanticweb.org/ontologies/2022/6/geological_taxonomy#Gabbro">
        <rdfs:subClassOf rdf:resource="http://www.semanticweb.org/ontologies/2022/6/geological_taxonomy#Igneous_rocks"/>
        <rdfs:comment>Gabbro is a phaneritic (coarse-grained), mafic intrusive igneous rock formed from the slow cooling of magnesium-rich and iron-rich magma into a holocrystalline mass deep beneath the Earth&apos;s surface.

Resource: https://en.wikipedia.org/wiki/Gabbro</rdfs:comment>
    </owl:Class>
    


    <!-- http://www.semanticweb.org/ontologies/2022/6/geological_taxonomy#Gelands -->

    <owl:Class rdf:about="http://www.semanticweb.org/ontologies/2022/6/geological_taxonomy#Gelands">
        <rdfs:subClassOf rdf:resource="http://www.semanticweb.org/ontologies/2022/6/geological_taxonomy#Andisols"/>
        <rdfs:comment>Andisols that have, in normal years, a mean annual soil temperature of 0 oC or colder and a mean summer soil temperature


Resource: https://sites.google.com/site/dinpuithai/Home/key10/key10d</rdfs:comment>
    </owl:Class>
    


    <!-- http://www.semanticweb.org/ontologies/2022/6/geological_taxonomy#Gelepts -->

    <owl:Class rdf:about="http://www.semanticweb.org/ontologies/2022/6/geological_taxonomy#Gelepts">
        <rdfs:subClassOf rdf:resource="http://www.semanticweb.org/ontologies/2022/6/geological_taxonomy#Inceptisols"/>
        <rdfs:comment>Inceptisols that have, in normal years, a mean annual soil temperature of 0 oC or colder and a mean summer soil temperature.

Resource: https://sites.google.com/site/dinpuithai/Home/key10/key10k</rdfs:comment>
    </owl:Class>
    


    <!-- http://www.semanticweb.org/ontologies/2022/6/geological_taxonomy#Gelisols -->

    <owl:Class rdf:about="http://www.semanticweb.org/ontologies/2022/6/geological_taxonomy#Gelisols">
        <rdfs:subClassOf rdf:resource="http://www.semanticweb.org/ontologies/2022/6/geological_taxonomy#Soil"/>
        <rdfs:comment>The central concept of Gelisols is that of soils that have permafrost within 100 cm of the soil surface and/or have gelic materials within 100 cm of the soil surface and have permafrost within 200 cm.

Resource: https://www.nrcs.usda.gov/wps/portal/nrcs/detail/soils/survey/class/maps/?cid=nrcs142p2_053598

Justification: Depending upon the soil material (organic vs. mineral) and the presence of gelic materials.
https://acsess.onlinelibrary.wiley.com/doi/full/10.2136/sh2013-54-4-gc</rdfs:comment>
    </owl:Class>
    


    <!-- http://www.semanticweb.org/ontologies/2022/6/geological_taxonomy#Gelods -->

    <owl:Class rdf:about="http://www.semanticweb.org/ontologies/2022/6/geological_taxonomy#Gelods">
        <rdfs:subClassOf rdf:resource="http://www.semanticweb.org/ontologies/2022/6/geological_taxonomy#Spodosols"/>
        <rdfs:comment>Very cold Spodosols that lack permafrost (gelic temperature
regime)

Resource: &quot;Illustrated Guide to Soil Taxonomy&quot; book by Unites States Department of Agriculture</rdfs:comment>
    </owl:Class>
    


    <!-- http://www.semanticweb.org/ontologies/2022/6/geological_taxonomy#Gelolls -->

    <owl:Class rdf:about="http://www.semanticweb.org/ontologies/2022/6/geological_taxonomy#Gelolls">
        <rdfs:subClassOf rdf:resource="http://www.semanticweb.org/ontologies/2022/6/geological_taxonomy#Mollisols"/>
        <rdfs:comment>Mollisols that have, in normal years, a mean annual soil temperature of 0 oC or colder and a mean summer soil temperature

Resource: https://sites.google.com/site/dinpuithai/Home/key10/key10i</rdfs:comment>
    </owl:Class>
    


    <!-- http://www.semanticweb.org/ontologies/2022/6/geological_taxonomy#Geological_Object -->

    <owl:Class rdf:about="http://www.semanticweb.org/ontologies/2022/6/geological_taxonomy#Geological_Object">
        <rdfs:subClassOf rdf:resource="http://www.semanticweb.org/ontologies/2022/6/geological_taxonomy#Geological_entities"/>
        <rdfs:comment>A material object constituted by some geological material.

Resource: https://github.com/Loop3D/GKM/blob/1.0.2/Loop3D-GSO/Modules/GSO-Geologic_Process.ttl

Justification: Classified based on the origination from distinct geological processes at different periods of time</rdfs:comment>
    </owl:Class>
    


    <!-- http://www.semanticweb.org/ontologies/2022/6/geological_taxonomy#Geological_entities -->

    <owl:Class rdf:about="http://www.semanticweb.org/ontologies/2022/6/geological_taxonomy#Geological_entities">
        <rdfs:comment>Geological thing with distinct and independent existence.

Justification: Different entities of geology</rdfs:comment>
    </owl:Class>
    


    <!-- http://www.semanticweb.org/ontologies/2022/6/geological_taxonomy#Geological_phenomena -->

    <owl:Class rdf:about="http://www.semanticweb.org/ontologies/2022/6/geological_taxonomy#Geological_phenomena">
        <rdfs:subClassOf rdf:resource="http://www.semanticweb.org/ontologies/2022/6/geological_taxonomy#Geological_entities"/>
        <rdfs:comment>Phenomenon which occurs without human inputs.

Justification: Classification based on the disaster and atmospheric conditions</rdfs:comment>
    </owl:Class>
    


    <!-- http://www.semanticweb.org/ontologies/2022/6/geological_taxonomy#Geyserite -->

    <owl:Class rdf:about="http://www.semanticweb.org/ontologies/2022/6/geological_taxonomy#Geyserite">
        <rdfs:subClassOf rdf:resource="http://www.semanticweb.org/ontologies/2022/6/geological_taxonomy#Sedimentary_rocks"/>
        <rdfs:comment>Geyserite, or siliceous sinter, is a form of opaline silica that is often found as crusts or layers around hot springs and geysers.

Resource: https://en.wikipedia.org/wiki/Geyserite</rdfs:comment>
    </owl:Class>
    


    <!-- http://www.semanticweb.org/ontologies/2022/6/geological_taxonomy#Gneiss -->

    <owl:Class rdf:about="http://www.semanticweb.org/ontologies/2022/6/geological_taxonomy#Gneiss">
        <rdfs:subClassOf rdf:resource="http://www.semanticweb.org/ontologies/2022/6/geological_taxonomy#Metamorphic_rocks"/>
        <rdfs:comment>A coarse grained metamorphic rock

Resource: https://geology.fandom.com/wiki/List_of_rock_types</rdfs:comment>
    </owl:Class>
    


    <!-- http://www.semanticweb.org/ontologies/2022/6/geological_taxonomy#Gossan -->

    <owl:Class rdf:about="http://www.semanticweb.org/ontologies/2022/6/geological_taxonomy#Gossan">
        <rdfs:subClassOf rdf:resource="http://www.semanticweb.org/ontologies/2022/6/geological_taxonomy#Metamorphic_rocks"/>
        <rdfs:comment>Gossan is intensely oxidized, weathered or decomposed rock, usually the upper and exposed part of an ore deposit or mineral vein.

Resource: https://en.wikipedia.org/wiki/Gossan</rdfs:comment>
    </owl:Class>
    


    <!-- http://www.semanticweb.org/ontologies/2022/6/geological_taxonomy#Granite -->

    <owl:Class rdf:about="http://www.semanticweb.org/ontologies/2022/6/geological_taxonomy#Granite">
        <rdfs:subClassOf rdf:resource="http://www.semanticweb.org/ontologies/2022/6/geological_taxonomy#Igneous_rocks"/>
        <rdfs:comment>Granite ( or is a coarse-grained intrusive igneous rock composed mostly of quartz, alkali feldspar, and plagioclase.

Resource: https://en.wikipedia.org/wiki/Granite</rdfs:comment>
    </owl:Class>
    


    <!-- http://www.semanticweb.org/ontologies/2022/6/geological_taxonomy#Granodiorite -->

    <owl:Class rdf:about="http://www.semanticweb.org/ontologies/2022/6/geological_taxonomy#Granodiorite">
        <rdfs:subClassOf rdf:resource="http://www.semanticweb.org/ontologies/2022/6/geological_taxonomy#Igneous_rocks"/>
        <rdfs:comment>Granodiorite is a coarse-grained (phaneritic) intrusive igneous rock similar to granite, but containing more plagioclase feldspar than orthoclase feldspar.

Resource: https://en.wikipedia.org/wiki/Granodiorite</rdfs:comment>
    </owl:Class>
    


    <!-- http://www.semanticweb.org/ontologies/2022/6/geological_taxonomy#Granophyre -->

    <owl:Class rdf:about="http://www.semanticweb.org/ontologies/2022/6/geological_taxonomy#Granophyre">
        <rdfs:subClassOf rdf:resource="http://www.semanticweb.org/ontologies/2022/6/geological_taxonomy#Igneous_rocks"/>
        <rdfs:comment>Granophyre is a subvolcanic rock that contains quartz and alkali feldspar in characteristic angular intergrowths such as those in the accompanying image.

Resource: https://en.wikipedia.org/wiki/Granophyre</rdfs:comment>
    </owl:Class>
    


    <!-- http://www.semanticweb.org/ontologies/2022/6/geological_taxonomy#Granulite -->

    <owl:Class rdf:about="http://www.semanticweb.org/ontologies/2022/6/geological_taxonomy#Granulite">
        <rdfs:subClassOf rdf:resource="http://www.semanticweb.org/ontologies/2022/6/geological_taxonomy#Metamorphic_rocks"/>
        <rdfs:comment>Granulites are a class of high-grade metamorphic rocks of the granulite facies that have experienced high-temperature and moderate-pressure metamorphism.

Resource: https://en.wikipedia.org/wiki/Granulite</rdfs:comment>
    </owl:Class>
    


    <!-- http://www.semanticweb.org/ontologies/2022/6/geological_taxonomy#Graywacke -->

    <owl:Class rdf:about="http://www.semanticweb.org/ontologies/2022/6/geological_taxonomy#Graywacke">
        <rdfs:subClassOf rdf:resource="http://www.semanticweb.org/ontologies/2022/6/geological_taxonomy#Sedimentary_rocks"/>
        <rdfs:comment>Greywacke or graywacke (German grauwacke, signifying a grey, earthy rock) is a variety of sandstone generally characterized by its hardness, dark color, and poorly sorted angular grains of quartz, feldspar, and small rock fragments or lithic fragments set in a compact, clay-fine matrix. It is a texturally immature sedimentary rock generally found in Paleozoic strata.

Resource: https://en.wikipedia.org/wiki/Greywacke</rdfs:comment>
    </owl:Class>
    


    <!-- http://www.semanticweb.org/ontologies/2022/6/geological_taxonomy#Greenschist -->

    <owl:Class rdf:about="http://www.semanticweb.org/ontologies/2022/6/geological_taxonomy#Greenschist">
        <rdfs:subClassOf rdf:resource="http://www.semanticweb.org/ontologies/2022/6/geological_taxonomy#Metamorphic_rocks"/>
        <rdfs:comment>Greenschists are metamorphic rocks that formed under the lowest temperatures and pressures usually produced by regional metamorphism, typically 300–450 °C (570–840 °F) and 2–10 kilobars (29,000–145,000 psi).

Resource: https://en.wikipedia.org/wiki/Greenschist

Justification: Depending upon the alteration to a greenish color by the formation of the minerals</rdfs:comment>
    </owl:Class>
    


    <!-- http://www.semanticweb.org/ontologies/2022/6/geological_taxonomy#Greenstone -->

    <owl:Class rdf:about="http://www.semanticweb.org/ontologies/2022/6/geological_taxonomy#Greenstone">
        <rdfs:subClassOf rdf:resource="http://www.semanticweb.org/ontologies/2022/6/geological_taxonomy#Greenschist"/>
        <rdfs:comment>A field term applied to any compact, dark-green, altered or metamorphosed basic igneous rock (e.g. spilite, basalt, gabbro, diabase) that owes its color to the presence of chlorite, actinolite, or epidote.

Resource: https://mrdata.usgs.gov/geology/state/sgmc-lith.php?code=5.3.3.3</rdfs:comment>
    </owl:Class>
    


    <!-- http://www.semanticweb.org/ontologies/2022/6/geological_taxonomy#Greisen -->

    <owl:Class rdf:about="http://www.semanticweb.org/ontologies/2022/6/geological_taxonomy#Greisen">
        <rdfs:subClassOf rdf:resource="http://www.semanticweb.org/ontologies/2022/6/geological_taxonomy#Metamorphic_rocks"/>
        <rdfs:comment>Greisen is a pneumatolytically altered granitic rock. Greisen contains lots of quartz and mica plus several exotic minerals like cassiterite, tourmaline, topaz, etc. Greised is a metamorphic rock that metamorphosed itself — hot fluids that altered the rock were provided by the cooling magma body itself

Resource: https://www.sandatlas.org/rock-types/</rdfs:comment>
    </owl:Class>
    


    <!-- http://www.semanticweb.org/ontologies/2022/6/geological_taxonomy#Greywacke -->

    <owl:Class rdf:about="http://www.semanticweb.org/ontologies/2022/6/geological_taxonomy#Greywacke">
        <rdfs:subClassOf rdf:resource="http://www.semanticweb.org/ontologies/2022/6/geological_taxonomy#Sedimentary_rocks"/>
        <rdfs:comment>Greywacke or graywacke (German grauwacke, signifying a grey, earthy rock) is a variety of sandstone generally characterized by its hardness, dark color, and poorly sorted angular grains of quartz, feldspar, and small rock fragments or lithic fragments set in a compact, clay-fine matrix. 

Resource: https://en.wikipedia.org/wiki/Greywacke</rdfs:comment>
    </owl:Class>
    


    <!-- http://www.semanticweb.org/ontologies/2022/6/geological_taxonomy#Gritstone -->

    <owl:Class rdf:about="http://www.semanticweb.org/ontologies/2022/6/geological_taxonomy#Gritstone">
        <rdfs:subClassOf rdf:resource="http://www.semanticweb.org/ontologies/2022/6/geological_taxonomy#Sedimentary_rocks"/>
        <rdfs:comment>Essentially a coarse sandstone formed from small pebbles

Resource: https://geology.fandom.com/wiki/List_of_rock_types</rdfs:comment>
    </owl:Class>
    


    <!-- http://www.semanticweb.org/ontologies/2022/6/geological_taxonomy#Ground_Fire -->

    <owl:Class rdf:about="http://www.semanticweb.org/ontologies/2022/6/geological_taxonomy#Ground_Fire">
        <rdfs:subClassOf rdf:resource="http://www.semanticweb.org/ontologies/2022/6/geological_taxonomy#Wildfire"/>
        <rdfs:comment>A ground fire is a type of wildfire that occurs in the subsurface where fuels such as peat, coal, tree roots, and other buried organic matter ignite and burn under the ground.	

Resource: https://www.supplycache.com/blogs/news/the-different-types-of-wildland-fires</rdfs:comment>
    </owl:Class>
    


    <!-- http://www.semanticweb.org/ontologies/2022/6/geological_taxonomy#Gypsids -->

    <owl:Class rdf:about="http://www.semanticweb.org/ontologies/2022/6/geological_taxonomy#Gypsids">
        <rdfs:subClassOf rdf:resource="http://www.semanticweb.org/ontologies/2022/6/geological_taxonomy#Aridisols"/>
        <rdfs:comment>Characterized by an accumulation of gypsum

Resource: https://www.sciencedirect.com/topics/agricultural-and-biological-sciences/aridisol</rdfs:comment>
    </owl:Class>
    


    <!-- http://www.semanticweb.org/ontologies/2022/6/geological_taxonomy#Gypsum -->

    <owl:Class rdf:about="http://www.semanticweb.org/ontologies/2022/6/geological_taxonomy#Gypsum">
        <rdfs:subClassOf rdf:resource="http://www.semanticweb.org/ontologies/2022/6/geological_taxonomy#Sedimentary_rocks"/>
        <rdfs:comment>Rock gypsum (a.k.a. gyprock) is a chemical sedimentary rock.  It is an example of an evaporite - it forms by the evaporation of water (usually seawater) and the precipitation of dissolved minerals.

Resource: http://www.jsjgeology.net/Rock-gypsum.htm</rdfs:comment>
    </owl:Class>
    


    <!-- http://www.semanticweb.org/ontologies/2022/6/geological_taxonomy#Halides -->

    <owl:Class rdf:about="http://www.semanticweb.org/ontologies/2022/6/geological_taxonomy#Halides">
        <rdfs:subClassOf rdf:resource="http://www.semanticweb.org/ontologies/2022/6/geological_taxonomy#Mineral"/>
        <rdfs:comment>The halide minerals are compounds in which a halogen (fluorine, chlorine, iodine, or bromine) is the main anion.	

Resource: https://en.wikipedia.org/wiki/Mineral#Classification</rdfs:comment>
    </owl:Class>
    


    <!-- http://www.semanticweb.org/ontologies/2022/6/geological_taxonomy#Harzburgite -->

    <owl:Class rdf:about="http://www.semanticweb.org/ontologies/2022/6/geological_taxonomy#Harzburgite">
        <rdfs:subClassOf rdf:resource="http://www.semanticweb.org/ontologies/2022/6/geological_taxonomy#Igneous_rocks"/>
        <rdfs:comment>Harzburgite, an ultramafic, igneous rock, is a variety of peridotite consisting mostly of the two minerals olivine and low-calcium (Ca) pyroxene (enstatite)

Resource: https://en.wikipedia.org/wiki/Harzburgite</rdfs:comment>
    </owl:Class>
    


    <!-- http://www.semanticweb.org/ontologies/2022/6/geological_taxonomy#Hawaiite -->

    <owl:Class rdf:about="http://www.semanticweb.org/ontologies/2022/6/geological_taxonomy#Hawaiite">
        <rdfs:subClassOf rdf:resource="http://www.semanticweb.org/ontologies/2022/6/geological_taxonomy#Basalt"/>
        <rdfs:comment>A class of basalts formed from ocean island (hot spot) magmatism.

Resource: https://geology.fandom.com/wiki/List_of_rock_types</rdfs:comment>
    </owl:Class>
    


    <!-- http://www.semanticweb.org/ontologies/2022/6/geological_taxonomy#Heat_wave -->

    <owl:Class rdf:about="http://www.semanticweb.org/ontologies/2022/6/geological_taxonomy#Heat_wave">
        <rdfs:subClassOf rdf:resource="http://www.semanticweb.org/ontologies/2022/6/geological_taxonomy#Extreme_Temperature"/>
        <rdfs:comment>A period of abnormally hot and/or unusually humid weather.

Resource: http://desinventar.cimafoundation.org/definitions.html</rdfs:comment>
    </owl:Class>
    


    <!-- http://www.semanticweb.org/ontologies/2022/6/geological_taxonomy#Hemists -->

    <owl:Class rdf:about="http://www.semanticweb.org/ontologies/2022/6/geological_taxonomy#Hemists">
        <rdfs:subClassOf rdf:resource="http://www.semanticweb.org/ontologies/2022/6/geological_taxonomy#Histosols"/>
        <rdfs:comment>Histosols that are primarily made up of moderately decomposed organic materials.

Resource: https://en.wikipedia.org/wiki/Histosol</rdfs:comment>
    </owl:Class>
    


    <!-- http://www.semanticweb.org/ontologies/2022/6/geological_taxonomy#Histels -->

    <owl:Class rdf:about="http://www.semanticweb.org/ontologies/2022/6/geological_taxonomy#Histels">
        <rdfs:subClassOf rdf:resource="http://www.semanticweb.org/ontologies/2022/6/geological_taxonomy#Gelisols"/>
        <rdfs:comment>Organic soil materials.

Resource: https://acsess.onlinelibrary.wiley.com/doi/full/10.2136/sh2013-54-4-gc</rdfs:comment>
    </owl:Class>
    


    <!-- http://www.semanticweb.org/ontologies/2022/6/geological_taxonomy#Histosols -->

    <owl:Class rdf:about="http://www.semanticweb.org/ontologies/2022/6/geological_taxonomy#Histosols">
        <rdfs:subClassOf rdf:resource="http://www.semanticweb.org/ontologies/2022/6/geological_taxonomy#Soil"/>
        <rdfs:comment>The central concept of Histosols is that of soils that are dominantly organic. 

Resource: https://www.nrcs.usda.gov/wps/portal/nrcs/detail/soils/survey/class/maps/?cid=nrcs142p2_053599

Justification: Depending upon the degree of decomposition of the organic matter.
https://www.sciencedirect.com/topics/agricultural-and-biological-sciences/histosols</rdfs:comment>
    </owl:Class>
    


    <!-- http://www.semanticweb.org/ontologies/2022/6/geological_taxonomy#Hornblendite -->

    <owl:Class rdf:about="http://www.semanticweb.org/ontologies/2022/6/geological_taxonomy#Hornblendite">
        <rdfs:subClassOf rdf:resource="http://www.semanticweb.org/ontologies/2022/6/geological_taxonomy#Igneous_rocks"/>
        <rdfs:comment>Hornblendite is a plutonic rock consisting mainly of the amphibole hornblende. Hornblende-rich ultramafic rocks are rare and when hornblende is the dominant mineral phase they are classified as hornblendites with qualifiers such as garnet hornblendite identifying a second abundant contained mineral.

Resource: https://en.wikipedia.org/wiki/Hornblendite</rdfs:comment>
    </owl:Class>
    


    <!-- http://www.semanticweb.org/ontologies/2022/6/geological_taxonomy#Hornfels -->

    <owl:Class rdf:about="http://www.semanticweb.org/ontologies/2022/6/geological_taxonomy#Hornfels">
        <rdfs:subClassOf rdf:resource="http://www.semanticweb.org/ontologies/2022/6/geological_taxonomy#Metamorphic_rocks"/>
        <rdfs:comment>Hornfels is the group name for a set of contact metamorphic rocks that have been baked and hardened by the heat of intrusive igneous masses and have been rendered massive, hard, splintery, and in some cases exceedingly tough and durable.

Resource: https://en.wikipedia.org/wiki/Hornfels

Justificaation: Depending upon the composition of hornfels</rdfs:comment>
    </owl:Class>
    


    <!-- http://www.semanticweb.org/ontologies/2022/6/geological_taxonomy#Humods -->

    <owl:Class rdf:about="http://www.semanticweb.org/ontologies/2022/6/geological_taxonomy#Humods">
        <rdfs:subClassOf rdf:resource="http://www.semanticweb.org/ontologies/2022/6/geological_taxonomy#Spodosols"/>
        <rdfs:comment>Spodosols with a large accumulation of carbon in the spodic
horizon

Resource: &quot;Illustrated Guide to Soil Taxonomy&quot; book by Unites States Department of Agriculture</rdfs:comment>
    </owl:Class>
    


    <!-- http://www.semanticweb.org/ontologies/2022/6/geological_taxonomy#Humults -->

    <owl:Class rdf:about="http://www.semanticweb.org/ontologies/2022/6/geological_taxonomy#Humults">
        <rdfs:subClassOf rdf:resource="http://www.semanticweb.org/ontologies/2022/6/geological_taxonomy#Ultisols"/>
        <rdfs:comment>Ultisols that have one or both of the following:
1. 0.9 percent (by weighted average) or more organic carbon in the upper 15 cm of the argillic or kandic horizon; or
2. 12 kg/m2 or more organic carbon between the mineral soil surface and a depth of 100 cm.


Resource: https://sites.google.com/site/dinpuithai/Home/key10/key10h</rdfs:comment>
    </owl:Class>
    


    <!-- http://www.semanticweb.org/ontologies/2022/6/geological_taxonomy#Hurricane -->

    <owl:Class rdf:about="http://www.semanticweb.org/ontologies/2022/6/geological_taxonomy#Hurricane">
        <rdfs:subClassOf rdf:resource="http://www.semanticweb.org/ontologies/2022/6/geological_taxonomy#Tropical_cyclone"/>
        <rdfs:comment>A tropical cyclone with maximum sustained winds of 74 mph (64 knots) or higher.	

Resource: https://www.nhc.noaa.gov/climo/</rdfs:comment>
    </owl:Class>
    


    <!-- http://www.semanticweb.org/ontologies/2022/6/geological_taxonomy#Hyaloclastite -->

    <owl:Class rdf:about="http://www.semanticweb.org/ontologies/2022/6/geological_taxonomy#Hyaloclastite">
        <rdfs:subClassOf rdf:resource="http://www.semanticweb.org/ontologies/2022/6/geological_taxonomy#Igneous_rocks"/>
        <rdfs:comment>Hyaloclastite is a volcanoclastic accumulation or breccia consisting of glass fragments (clasts) formed by quench fragmentation of lava flow surfaces during submarine or subglacial extrusion.

Resource: https://en.wikipedia.org/wiki/Hyaloclastite</rdfs:comment>
    </owl:Class>
    


    <!-- http://www.semanticweb.org/ontologies/2022/6/geological_taxonomy#Icelandite -->

    <owl:Class rdf:about="http://www.semanticweb.org/ontologies/2022/6/geological_taxonomy#Icelandite">
        <rdfs:subClassOf rdf:resource="http://www.semanticweb.org/ontologies/2022/6/geological_taxonomy#Igneous_rocks"/>
        <rdfs:comment>Icelandite is a type of volcanic rock, an andesite that is enriched in iron but deficient in aluminium (&lt; 16.5% Al2O3).

Resource: https://en.wikipedia.org/wiki/Icelandite</rdfs:comment>
    </owl:Class>
    


    <!-- http://www.semanticweb.org/ontologies/2022/6/geological_taxonomy#Igneous_rocks -->

    <owl:Class rdf:about="http://www.semanticweb.org/ontologies/2022/6/geological_taxonomy#Igneous_rocks">
        <rdfs:subClassOf rdf:resource="http://www.semanticweb.org/ontologies/2022/6/geological_taxonomy#Rock"/>
        <rdfs:comment>Igneous rock is formed through the cooling and solidification of magma or lava.

Resource: https://en.wikipedia.org/wiki/Igneous_rock

Justification: Igneous rocks are classified according to mode of occurrence, texture, mineralogy, chemical composition, and the geometry of the igneous body.
https://en.wikipedia.org/wiki/Igneous_rock#Classification</rdfs:comment>
    </owl:Class>
    


    <!-- http://www.semanticweb.org/ontologies/2022/6/geological_taxonomy#Ignimbrite -->

    <owl:Class rdf:about="http://www.semanticweb.org/ontologies/2022/6/geological_taxonomy#Ignimbrite">
        <rdfs:subClassOf rdf:resource="http://www.semanticweb.org/ontologies/2022/6/geological_taxonomy#Igneous_rocks"/>
        <rdfs:comment>Ignimbrite is a type of volcanic rock. More specifically, ignimbrite is a variety of hardened tuff. 

Resource: https://en.wikipedia.org/wiki/Ignimbrite</rdfs:comment>
    </owl:Class>
    


    <!-- http://www.semanticweb.org/ontologies/2022/6/geological_taxonomy#Ijolite -->

    <owl:Class rdf:about="http://www.semanticweb.org/ontologies/2022/6/geological_taxonomy#Ijolite">
        <rdfs:subClassOf rdf:resource="http://www.semanticweb.org/ontologies/2022/6/geological_taxonomy#Igneous_rocks"/>
        <rdfs:comment>Ijolite is an igneous rock consisting essentially of nepheline and augite.

Resource: https://en.wikipedia.org/wiki/Ijolite</rdfs:comment>
    </owl:Class>
    


    <!-- http://www.semanticweb.org/ontologies/2022/6/geological_taxonomy#Inceptisols -->

    <owl:Class rdf:about="http://www.semanticweb.org/ontologies/2022/6/geological_taxonomy#Inceptisols">
        <rdfs:subClassOf rdf:resource="http://www.semanticweb.org/ontologies/2022/6/geological_taxonomy#Soil"/>
        <rdfs:comment>The central concept of Inceptisols is that of soils of humid and subhumid regions that have altered horizons that have lost bases or iron and aluminum but retain some weatherable minerals.

Resource: https://www.nrcs.usda.gov/wps/portal/nrcs/detail/soils/survey/class/maps/?cid=nrcs142p2_053601

Justification: The suborders of Inceptisols are distinguished by soil moisture, epipedon properties, and soil temperature regime.
https://web.archive.org/web/20040918225129/http://grunwald.ifas.ufl.edu/Nat_resources/soil_orders/inceptisols.htm</rdfs:comment>
    </owl:Class>
    


    <!-- http://www.semanticweb.org/ontologies/2022/6/geological_taxonomy#Interplate_earthquake -->

    <owl:Class rdf:about="http://www.semanticweb.org/ontologies/2022/6/geological_taxonomy#Interplate_earthquake">
        <rdfs:subClassOf rdf:resource="http://www.semanticweb.org/ontologies/2022/6/geological_taxonomy#Tectonic_Earthquake"/>
        <owl:disjointWith rdf:resource="http://www.semanticweb.org/ontologies/2022/6/geological_taxonomy#Intraplate_earthquake"/>
        <rdfs:comment>Earthquake that occurs at the boundary between two tectonic plates.

Resource: https://en.wikipedia.org/wiki/Interplate_earthquake</rdfs:comment>
    </owl:Class>
    


    <!-- http://www.semanticweb.org/ontologies/2022/6/geological_taxonomy#Intraplate_earthquake -->

    <owl:Class rdf:about="http://www.semanticweb.org/ontologies/2022/6/geological_taxonomy#Intraplate_earthquake">
        <rdfs:subClassOf rdf:resource="http://www.semanticweb.org/ontologies/2022/6/geological_taxonomy#Tectonic_Earthquake"/>
        <rdfs:comment>Earthquake that occurs within the interior of a tectonic plate

Resource: https://en.wikipedia.org/wiki/Intraplate_earthquake</rdfs:comment>
    </owl:Class>
    


    <!-- http://www.semanticweb.org/ontologies/2022/6/geological_taxonomy#Itacolumite -->

    <owl:Class rdf:about="http://www.semanticweb.org/ontologies/2022/6/geological_taxonomy#Itacolumite">
        <rdfs:subClassOf rdf:resource="http://www.semanticweb.org/ontologies/2022/6/geological_taxonomy#Sedimentary_rocks"/>
        <rdfs:comment>Itacolumite is a naturally occurring porous, yellow sandstone that is flexible when cut into relatively thin slabs.

Resource: https://en.wikipedia.org/wiki/Itacolumite</rdfs:comment>
    </owl:Class>
    


    <!-- http://www.semanticweb.org/ontologies/2022/6/geological_taxonomy#Jaspillite -->

    <owl:Class rdf:about="http://www.semanticweb.org/ontologies/2022/6/geological_taxonomy#Jaspillite">
        <rdfs:subClassOf rdf:resource="http://www.semanticweb.org/ontologies/2022/6/geological_taxonomy#Sedimentary_rocks"/>
        <rdfs:comment>An iron-rich chemical sedimentary rock similar to chert or banded iron formation

Resource: https://geology.fandom.com/wiki/List_of_rock_types</rdfs:comment>
    </owl:Class>
    


    <!-- http://www.semanticweb.org/ontologies/2022/6/geological_taxonomy#Kimberlite -->

    <owl:Class rdf:about="http://www.semanticweb.org/ontologies/2022/6/geological_taxonomy#Kimberlite">
        <rdfs:subClassOf rdf:resource="http://www.semanticweb.org/ontologies/2022/6/geological_taxonomy#Igneous_rocks"/>
        <rdfs:comment>Kimberlite is an igneous rock and a rare variant of peridotite.

Resource: https://en.wikipedia.org/wiki/Kimberlite</rdfs:comment>
    </owl:Class>
    


    <!-- http://www.semanticweb.org/ontologies/2022/6/geological_taxonomy#Komatiite -->

    <owl:Class rdf:about="http://www.semanticweb.org/ontologies/2022/6/geological_taxonomy#Komatiite">
        <rdfs:subClassOf rdf:resource="http://www.semanticweb.org/ontologies/2022/6/geological_taxonomy#Igneous_rocks"/>
        <rdfs:comment>Komatiite is a type of ultramafic mantle-derived volcanic rock defined as having crystallised from a lava of at least 18 wt% MgO.

Resource: https://en.wikipedia.org/wiki/Komatiite</rdfs:comment>
    </owl:Class>
    


    <!-- http://www.semanticweb.org/ontologies/2022/6/geological_taxonomy#Lamproite -->

    <owl:Class rdf:about="http://www.semanticweb.org/ontologies/2022/6/geological_taxonomy#Lamproite">
        <rdfs:subClassOf rdf:resource="http://www.semanticweb.org/ontologies/2022/6/geological_taxonomy#Igneous_rocks"/>
        <rdfs:comment>Lamproite is an ultrapotassic mantle-derived volcanic or subvolcanic rock.

Resource: https://en.wikipedia.org/wiki/Lamproite</rdfs:comment>
    </owl:Class>
    


    <!-- http://www.semanticweb.org/ontologies/2022/6/geological_taxonomy#Lamprophyre -->

    <owl:Class rdf:about="http://www.semanticweb.org/ontologies/2022/6/geological_taxonomy#Lamprophyre">
        <rdfs:subClassOf rdf:resource="http://www.semanticweb.org/ontologies/2022/6/geological_taxonomy#Igneous_rocks"/>
        <rdfs:comment>Ultrapotassic igneous rocks – An ultramafic, ultrapotassic intrusive rock dominated by mafic phenocrysts in a feldspar groundmass

Resource: https://en.wikipedia.org/wiki/Lamprophyre</rdfs:comment>
    </owl:Class>
    


    <!-- http://www.semanticweb.org/ontologies/2022/6/geological_taxonomy#Landslide -->

    <owl:Class rdf:about="http://www.semanticweb.org/ontologies/2022/6/geological_taxonomy#Landslide">
        <rdfs:subClassOf rdf:resource="http://www.semanticweb.org/ontologies/2022/6/geological_taxonomy#Natural_disaster"/>
        <rdfs:comment>Landslides, also known as landslips, are several forms of mass wasting that may include a wide range of ground movements, such as rockfalls, deep-seated slope failures, mudflows, and debris flows.

Resource: https://en.wikipedia.org/wiki/Landslide

Justification: Classified based on the different movements of material across the slope</rdfs:comment>
    </owl:Class>
    


    <!-- http://www.semanticweb.org/ontologies/2022/6/geological_taxonomy#Lateral_Spread -->

    <owl:Class rdf:about="http://www.semanticweb.org/ontologies/2022/6/geological_taxonomy#Lateral_Spread">
        <rdfs:subClassOf rdf:resource="http://www.semanticweb.org/ontologies/2022/6/geological_taxonomy#Flow"/>
        <rdfs:comment>Lateral spread or flow are terms referring to landslides that commonly form on gentle slopes and that have rapid fluid-like flow movement, like water.

Resource: https://earthquake.usgs.gov/learn/glossary/?term=lateral%20spread%20or%20flow

Justification: Classified based on type of material</rdfs:comment>
    </owl:Class>
    


    <!-- http://www.semanticweb.org/ontologies/2022/6/geological_taxonomy#Laterite -->

    <owl:Class rdf:about="http://www.semanticweb.org/ontologies/2022/6/geological_taxonomy#Laterite">
        <rdfs:subClassOf rdf:resource="http://www.semanticweb.org/ontologies/2022/6/geological_taxonomy#Sedimentary_rocks"/>
        <rdfs:comment>A residual sedimentary rock formed from a parent rock under tropical conditions

Resource: https://geology.fandom.com/wiki/List_of_rock_types</rdfs:comment>
    </owl:Class>
    


    <!-- http://www.semanticweb.org/ontologies/2022/6/geological_taxonomy#Latite -->

    <owl:Class rdf:about="http://www.semanticweb.org/ontologies/2022/6/geological_taxonomy#Latite">
        <rdfs:subClassOf rdf:resource="http://www.semanticweb.org/ontologies/2022/6/geological_taxonomy#Igneous_rocks"/>
        <rdfs:comment>Latite is an igneous, volcanic rock, with aphanitic-aphyric to aphyric-porphyritic texture.

Resource: https://en.wikipedia.org/wiki/Latite</rdfs:comment>
    </owl:Class>
    


    <!-- http://www.semanticweb.org/ontologies/2022/6/geological_taxonomy#Lherzolite -->

    <owl:Class rdf:about="http://www.semanticweb.org/ontologies/2022/6/geological_taxonomy#Lherzolite">
        <rdfs:subClassOf rdf:resource="http://www.semanticweb.org/ontologies/2022/6/geological_taxonomy#Igneous_rocks"/>
        <rdfs:comment>Lherzolite is a type of ultramafic igneous rock. 

Resource: https://en.wikipedia.org/wiki/Lherzolite</rdfs:comment>
    </owl:Class>
    


    <!-- http://www.semanticweb.org/ontologies/2022/6/geological_taxonomy#Lignite -->

    <owl:Class rdf:about="http://www.semanticweb.org/ontologies/2022/6/geological_taxonomy#Lignite">
        <rdfs:subClassOf rdf:resource="http://www.semanticweb.org/ontologies/2022/6/geological_taxonomy#Sedimentary_rocks"/>
        <rdfs:comment>A sedimentary rock composed of organic material; otherwise known as Brown Coal

Resource: https://geology.fandom.com/wiki/List_of_rock_types</rdfs:comment>
    </owl:Class>
    


    <!-- http://www.semanticweb.org/ontologies/2022/6/geological_taxonomy#Limburgite -->

    <owl:Class rdf:about="http://www.semanticweb.org/ontologies/2022/6/geological_taxonomy#Limburgite">
        <rdfs:subClassOf rdf:resource="http://www.semanticweb.org/ontologies/2022/6/geological_taxonomy#Igneous_rocks"/>
        <rdfs:comment>imburgite is a dark-colored volcanic rock resembling basalt in appearance, but containing normally no feldspar.

Resource: https://en.wikipedia.org/wiki/Limburgite</rdfs:comment>
    </owl:Class>
    


    <!-- http://www.semanticweb.org/ontologies/2022/6/geological_taxonomy#Limestone -->

    <owl:Class rdf:about="http://www.semanticweb.org/ontologies/2022/6/geological_taxonomy#Limestone">
        <rdfs:subClassOf rdf:resource="http://www.semanticweb.org/ontologies/2022/6/geological_taxonomy#Sedimentary_rocks"/>
        <rdfs:comment>A sedimentary rock composed primarily of carbonate minerals

Resource: https://geology.fandom.com/wiki/List_of_rock_types</rdfs:comment>
    </owl:Class>
    


    <!-- http://www.semanticweb.org/ontologies/2022/6/geological_taxonomy#Limnic_Eruption -->

    <owl:Class rdf:about="http://www.semanticweb.org/ontologies/2022/6/geological_taxonomy#Limnic_Eruption">
        <rdfs:subClassOf rdf:resource="http://www.semanticweb.org/ontologies/2022/6/geological_taxonomy#Natural_disaster"/>
        <rdfs:comment>type of natural disaster in which dissolved carbon dioxide (CO2) suddenly erupts from deep lake waters, forming a gas cloud capable of suffocating wildlife, livestock, and humans. 	

Resource: https://en.wikipedia.org/wiki/Limnic_eruption</rdfs:comment>
    </owl:Class>
    


    <!-- http://www.semanticweb.org/ontologies/2022/6/geological_taxonomy#Litchfieldite -->

    <owl:Class rdf:about="http://www.semanticweb.org/ontologies/2022/6/geological_taxonomy#Litchfieldite">
        <rdfs:subClassOf rdf:resource="http://www.semanticweb.org/ontologies/2022/6/geological_taxonomy#Metamorphic_rocks"/>
        <rdfs:comment>Nepheline syenite gneiss

Resource: https://en.wikipedia.org/wiki/List_of_rock_types</rdfs:comment>
    </owl:Class>
    


    <!-- http://www.semanticweb.org/ontologies/2022/6/geological_taxonomy#Lithosphere -->

    <owl:Class rdf:about="http://www.semanticweb.org/ontologies/2022/6/geological_taxonomy#Lithosphere">
        <rdfs:subClassOf rdf:resource="http://www.semanticweb.org/ontologies/2022/6/geological_taxonomy#Upper_mantle"/>
        <rdfs:comment>outer, solid portion of the Earth. Also called the geosphere

Resource: https://education.nationalgeographic.org/resource/mantle

Justification: depending upon which crust it is associated</rdfs:comment>
    </owl:Class>
    


    <!-- http://www.semanticweb.org/ontologies/2022/6/geological_taxonomy#Local_tsunami -->

    <owl:Class rdf:about="http://www.semanticweb.org/ontologies/2022/6/geological_taxonomy#Local_tsunami">
        <rdfs:subClassOf rdf:resource="http://www.semanticweb.org/ontologies/2022/6/geological_taxonomy#Tsunami"/>
        <owl:disjointWith rdf:resource="http://www.semanticweb.org/ontologies/2022/6/geological_taxonomy#Teletsunami"/>
        <rdfs:comment>waves affecting coastlines close to the generating area (whether by tectonic or landslide activity)	

Resource: http://www.sfu.ca/geog355fall01/cobryne/types_of_tsunamis.html</rdfs:comment>
    </owl:Class>
    


    <!-- http://www.semanticweb.org/ontologies/2022/6/geological_taxonomy#Lower_mantle -->

    <owl:Class rdf:about="http://www.semanticweb.org/ontologies/2022/6/geological_taxonomy#Lower_mantle">
        <rdfs:subClassOf rdf:resource="http://www.semanticweb.org/ontologies/2022/6/geological_taxonomy#Mantle"/>
        <rdfs:comment>the region from 660 to 2900 km below Earth&apos;s surface; between the transition zone and the outer core.

Resource: https://en.wikipedia.org/wiki/Lower_mantle_(Earth)</rdfs:comment>
    </owl:Class>
    


    <!-- http://www.semanticweb.org/ontologies/2022/6/geological_taxonomy#Major_Hurricane -->

    <owl:Class rdf:about="http://www.semanticweb.org/ontologies/2022/6/geological_taxonomy#Major_Hurricane">
        <rdfs:subClassOf rdf:resource="http://www.semanticweb.org/ontologies/2022/6/geological_taxonomy#Tropical_cyclone"/>
        <rdfs:comment>A tropical cyclone with maximum sustained winds of 111 mph (96 knots) or higher,	

Resource: https://www.nhc.noaa.gov/climo/</rdfs:comment>
    </owl:Class>
    


    <!-- http://www.semanticweb.org/ontologies/2022/6/geological_taxonomy#Mantle -->

    <owl:Class rdf:about="http://www.semanticweb.org/ontologies/2022/6/geological_taxonomy#Mantle">
        <rdfs:subClassOf rdf:resource="http://www.semanticweb.org/ontologies/2022/6/geological_taxonomy#Units_of_Earth_structure"/>
        <rdfs:comment>part of the interior of the planet Earth

Resource: https://en.wikipedia.org/wiki/Mantle_(geology)

Justification: depending on changes in seismic velocity</rdfs:comment>
    </owl:Class>
    


    <!-- http://www.semanticweb.org/ontologies/2022/6/geological_taxonomy#Marble -->

    <owl:Class rdf:about="http://www.semanticweb.org/ontologies/2022/6/geological_taxonomy#Marble">
        <rdfs:subClassOf rdf:resource="http://www.semanticweb.org/ontologies/2022/6/geological_taxonomy#Metamorphic_rocks"/>
        <rdfs:comment>Marble is a metamorphic rock composed of recrystallized carbonate minerals, most commonly calcite or dolomite.

Resource: https://en.wikipedia.org/wiki/Marble</rdfs:comment>
    </owl:Class>
    


    <!-- http://www.semanticweb.org/ontologies/2022/6/geological_taxonomy#Marl -->

    <owl:Class rdf:about="http://www.semanticweb.org/ontologies/2022/6/geological_taxonomy#Marl">
        <rdfs:subClassOf rdf:resource="http://www.semanticweb.org/ontologies/2022/6/geological_taxonomy#Sedimentary_rocks"/>
        <rdfs:comment>A limestone with a considerable proportion of silicate material

Resource: https://geology.fandom.com/wiki/List_of_rock_types</rdfs:comment>
    </owl:Class>
    


    <!-- http://www.semanticweb.org/ontologies/2022/6/geological_taxonomy#Metamorphic_rocks -->

    <owl:Class rdf:about="http://www.semanticweb.org/ontologies/2022/6/geological_taxonomy#Metamorphic_rocks">
        <rdfs:subClassOf rdf:resource="http://www.semanticweb.org/ontologies/2022/6/geological_taxonomy#Rock"/>
        <rdfs:comment>Metamorphic rocks arise from the transformation of existing rock to new types of rock in a process called metamorphism

Resource: https://en.wikipedia.org/wiki/Metamorphic_rock

Justification: Classification of metamorphic rocks is based on mineral assemblage, texture, protolith, and bulk chemical composition of the rock.
https://www.geologyin.com/2014/07/classification-of-metamorphic-rocks.html</rdfs:comment>
    </owl:Class>
    


    <!-- http://www.semanticweb.org/ontologies/2022/6/geological_taxonomy#Metapelite -->

    <owl:Class rdf:about="http://www.semanticweb.org/ontologies/2022/6/geological_taxonomy#Metapelite">
        <rdfs:subClassOf rdf:resource="http://www.semanticweb.org/ontologies/2022/6/geological_taxonomy#Metamorphic_rocks"/>
        <rdfs:comment>A metamorphic rock with a protolith of clay-rich (siltstone) sedimentary rock

Resource: https://en.wikipedia.org/wiki/Metapelite</rdfs:comment>
    </owl:Class>
    


    <!-- http://www.semanticweb.org/ontologies/2022/6/geological_taxonomy#Metapsammite -->

    <owl:Class rdf:about="http://www.semanticweb.org/ontologies/2022/6/geological_taxonomy#Metapsammite">
        <rdfs:subClassOf rdf:resource="http://www.semanticweb.org/ontologies/2022/6/geological_taxonomy#Metamorphic_rocks"/>
        <rdfs:comment>A metamorphic rock with a protolith of quartz-rich (sandstone) sedimentary rock

Resource: https://en.wikipedia.org/wiki/List_of_rock_types</rdfs:comment>
    </owl:Class>
    


    <!-- http://www.semanticweb.org/ontologies/2022/6/geological_taxonomy#Migmatite -->

    <owl:Class rdf:about="http://www.semanticweb.org/ontologies/2022/6/geological_taxonomy#Migmatite">
        <rdfs:subClassOf rdf:resource="http://www.semanticweb.org/ontologies/2022/6/geological_taxonomy#Metamorphic_rocks"/>
        <rdfs:comment>Migmatite is a composite rock found in medium and high-grade metamorphic environments.

Resource: https://en.wikipedia.org/wiki/Migmatite</rdfs:comment>
    </owl:Class>
    


    <!-- http://www.semanticweb.org/ontologies/2022/6/geological_taxonomy#Mineral -->

    <owl:Class rdf:about="http://www.semanticweb.org/ontologies/2022/6/geological_taxonomy#Mineral">
        <rdfs:subClassOf rdf:resource="http://www.semanticweb.org/ontologies/2022/6/geological_taxonomy#Geological_Object"/>
        <rdfs:comment>Mineral or mineral species is, broadly speaking, a solid chemical compound with a fairly well-defined chemical composition and a specific crystal structure that occurs naturally in pure form.

Resource: https://en.wikipedia.org/wiki/Mineral

Justification: Classified based on chemical composition, mineral properties, crystal systems and silicate structures
https://sternberg.fhsu.edu/research-collections/geology/mineral-classification-page.html</rdfs:comment>
    </owl:Class>
    


    <!-- http://www.semanticweb.org/ontologies/2022/6/geological_taxonomy#Moderate_Drought -->

    <owl:Class rdf:about="http://www.semanticweb.org/ontologies/2022/6/geological_taxonomy#Moderate_Drought">
        <rdfs:subClassOf rdf:resource="http://www.semanticweb.org/ontologies/2022/6/geological_taxonomy#Drought"/>
        <rdfs:comment>It is D1 category, causes some damage to crops, pastures, streams, reservoirs, or wells low, some water shortages developing or imminent.

Resource: https://droughtmonitor.unl.edu/About/WhatistheUSDM.aspx</rdfs:comment>
    </owl:Class>
    


    <!-- http://www.semanticweb.org/ontologies/2022/6/geological_taxonomy#Mollisols -->

    <owl:Class rdf:about="http://www.semanticweb.org/ontologies/2022/6/geological_taxonomy#Mollisols">
        <rdfs:subClassOf rdf:resource="http://www.semanticweb.org/ontologies/2022/6/geological_taxonomy#Soil"/>
        <rdfs:comment>The central concept of Mollisols is that of soils that have a dark colored surface horizon and are base rich. Nearly all have a mollic epipedon.

Resource: https://www.nrcs.usda.gov/wps/portal/nrcs/detail/soils/survey/class/maps/?cid=nrcs142p2_053603

Justification: Soil temperature and moisture are principally used to separate.
https://www.sciencedirect.com/topics/agricultural-and-biological-sciences/mollisol</rdfs:comment>
    </owl:Class>
    


    <!-- http://www.semanticweb.org/ontologies/2022/6/geological_taxonomy#Monzogranite -->

    <owl:Class rdf:about="http://www.semanticweb.org/ontologies/2022/6/geological_taxonomy#Monzogranite">
        <rdfs:subClassOf rdf:resource="http://www.semanticweb.org/ontologies/2022/6/geological_taxonomy#Igneous_rocks"/>
        <rdfs:comment>Monzogranites are biotite granite rocks that are considered to be the final fractionation product of magma. 

Resource: https://en.wikipedia.org/wiki/Monzogranite</rdfs:comment>
    </owl:Class>
    


    <!-- http://www.semanticweb.org/ontologies/2022/6/geological_taxonomy#Monzonite -->

    <owl:Class rdf:about="http://www.semanticweb.org/ontologies/2022/6/geological_taxonomy#Monzonite">
        <rdfs:subClassOf rdf:resource="http://www.semanticweb.org/ontologies/2022/6/geological_taxonomy#Igneous_rocks"/>
        <rdfs:comment>Monzonite is an igneous intrusive rock, formed by slow cooling of underground magma that has a moderate silica content and is enriched in alkali metal oxides.

Resource: https://en.wikipedia.org/wiki/Monzonite</rdfs:comment>
    </owl:Class>
    


    <!-- http://www.semanticweb.org/ontologies/2022/6/geological_taxonomy#Mudstone -->

    <owl:Class rdf:about="http://www.semanticweb.org/ontologies/2022/6/geological_taxonomy#Mudstone">
        <rdfs:subClassOf rdf:resource="http://www.semanticweb.org/ontologies/2022/6/geological_taxonomy#Sedimentary_rocks"/>
        <rdfs:comment>A sedimentary rock composed of clay and muds

Resource: https://geology.fandom.com/wiki/List_of_rock_types</rdfs:comment>
    </owl:Class>
    


    <!-- http://www.semanticweb.org/ontologies/2022/6/geological_taxonomy#Mugearite -->

    <owl:Class rdf:about="http://www.semanticweb.org/ontologies/2022/6/geological_taxonomy#Mugearite">
        <rdfs:subClassOf rdf:resource="http://www.semanticweb.org/ontologies/2022/6/geological_taxonomy#Trachyandesite"/>
        <rdfs:comment>Sodic basaltic trachyandesite

Resource: https://geology.fandom.com/wiki/List_of_rock_types</rdfs:comment>
    </owl:Class>
    


    <!-- http://www.semanticweb.org/ontologies/2022/6/geological_taxonomy#Mylonite -->

    <owl:Class rdf:about="http://www.semanticweb.org/ontologies/2022/6/geological_taxonomy#Mylonite">
        <rdfs:subClassOf rdf:resource="http://www.semanticweb.org/ontologies/2022/6/geological_taxonomy#Metamorphic_rocks"/>
        <rdfs:comment>Mylonite is a fine-grained, compact metamorphic rock produced by dynamic recrystallization of the constituent minerals resulting in a reduction of the grain size of the rock.

Resource: https://en.wikipedia.org/wiki/Mylonite</rdfs:comment>
    </owl:Class>
    


    <!-- http://www.semanticweb.org/ontologies/2022/6/geological_taxonomy#Napoleonite -->

    <owl:Class rdf:about="http://www.semanticweb.org/ontologies/2022/6/geological_taxonomy#Napoleonite">
        <rdfs:subClassOf rdf:resource="http://www.semanticweb.org/ontologies/2022/6/geological_taxonomy#Diorite"/>
        <rdfs:comment>Napoleonite is a variety of diorite which is characterized by orbicular structure.

Resource: https://en.wikipedia.org/wiki/Napoleonite</rdfs:comment>
    </owl:Class>
    


    <!-- http://www.semanticweb.org/ontologies/2022/6/geological_taxonomy#Natural_disaster -->

    <owl:Class rdf:about="http://www.semanticweb.org/ontologies/2022/6/geological_taxonomy#Natural_disaster">
        <rdfs:subClassOf rdf:resource="http://www.semanticweb.org/ontologies/2022/6/geological_taxonomy#Geological_phenomena"/>
        <owl:disjointWith rdf:resource="http://www.semanticweb.org/ontologies/2022/6/geological_taxonomy#Weather_conditions"/>
        <rdfs:comment>A natural disaster is &quot;the negative impact following an actual occurrence of natural hazard in the event that it significantly harms a community&quot;.

Resource: https://en.wikipedia.org/wiki/Natural_disaster

Justification: Classified based on origin, cause of the disaster and due to weather conditions.</rdfs:comment>
    </owl:Class>
    


    <!-- http://www.semanticweb.org/ontologies/2022/6/geological_taxonomy#Nepheline_syenite -->

    <owl:Class rdf:about="http://www.semanticweb.org/ontologies/2022/6/geological_taxonomy#Nepheline_syenite">
        <rdfs:subClassOf rdf:resource="http://www.semanticweb.org/ontologies/2022/6/geological_taxonomy#Igneous_rocks"/>
        <rdfs:comment>Nepheline syenite is a holocrystalline plutonic rock that consists largely of nepheline and alkali feldspar. 

Resource: https://en.wikipedia.org/wiki/Nepheline_syenite</rdfs:comment>
    </owl:Class>
    


    <!-- http://www.semanticweb.org/ontologies/2022/6/geological_taxonomy#Nephelinite -->

    <owl:Class rdf:about="http://www.semanticweb.org/ontologies/2022/6/geological_taxonomy#Nephelinite">
        <rdfs:subClassOf rdf:resource="http://www.semanticweb.org/ontologies/2022/6/geological_taxonomy#Igneous_rocks"/>
        <rdfs:comment>Nephelinite is a fine-grained or aphanitic igneous rock made up almost entirely of nepheline and clinopyroxene.

Resource: https://en.wikipedia.org/wiki/Nephelinite</rdfs:comment>
    </owl:Class>
    


    <!-- http://www.semanticweb.org/ontologies/2022/6/geological_taxonomy#Norite -->

    <owl:Class rdf:about="http://www.semanticweb.org/ontologies/2022/6/geological_taxonomy#Norite">
        <rdfs:subClassOf rdf:resource="http://www.semanticweb.org/ontologies/2022/6/geological_taxonomy#Igneous_rocks"/>
        <rdfs:comment>Norite is a mafic intrusive igneous rock composed largely of the calcium-rich plagioclase labradorite, orthopyroxene, and olivine.

Resource: https://en.wikipedia.org/wiki/Norite</rdfs:comment>
    </owl:Class>
    


    <!-- http://www.semanticweb.org/ontologies/2022/6/geological_taxonomy#Obsidian -->

    <owl:Class rdf:about="http://www.semanticweb.org/ontologies/2022/6/geological_taxonomy#Obsidian">
        <rdfs:subClassOf rdf:resource="http://www.semanticweb.org/ontologies/2022/6/geological_taxonomy#Igneous_rocks"/>
        <rdfs:comment>Obsidian is an igneous rock that forms when molten rock material cools so rapidly that atoms are unable to arrange themselves into a crystalline structure.

Resource: https://geology.com/rocks/obsidian.shtml</rdfs:comment>
    </owl:Class>
    


    <!-- http://www.semanticweb.org/ontologies/2022/6/geological_taxonomy#Oceanic_crust -->

    <owl:Class rdf:about="http://www.semanticweb.org/ontologies/2022/6/geological_taxonomy#Oceanic_crust">
        <rdfs:subClassOf rdf:resource="http://www.semanticweb.org/ontologies/2022/6/geological_taxonomy#Crust"/>
        <rdfs:comment>Oceanic crust is the uppermost layer of the oceanic portion of the tectonic plates composed of dense (mafic) iron magnesium silicate igneous rocks, like basalt.

Resource: https://en.wikipedia.org/wiki/Oceanic_crust</rdfs:comment>
    </owl:Class>
    


    <!-- http://www.semanticweb.org/ontologies/2022/6/geological_taxonomy#Oceanic_lithosphere -->

    <owl:Class rdf:about="http://www.semanticweb.org/ontologies/2022/6/geological_taxonomy#Oceanic_lithosphere">
        <rdfs:subClassOf rdf:resource="http://www.semanticweb.org/ontologies/2022/6/geological_taxonomy#Lithosphere"/>
        <rdfs:comment>Oceanic lithosphere is associated with oceanic crust and exists in the ocean basins

Resource: https://en.wikipedia.org/wiki/Lithosphere</rdfs:comment>
    </owl:Class>
    


    <!-- http://www.semanticweb.org/ontologies/2022/6/geological_taxonomy#Oil_shale -->

    <owl:Class rdf:about="http://www.semanticweb.org/ontologies/2022/6/geological_taxonomy#Oil_shale">
        <rdfs:subClassOf rdf:resource="http://www.semanticweb.org/ontologies/2022/6/geological_taxonomy#Sedimentary_rocks"/>
        <rdfs:comment>A sedimentary rock composed dominantly of organic material

Resource: https://geology.fandom.com/wiki/List_of_rock_types</rdfs:comment>
    </owl:Class>
    


    <!-- http://www.semanticweb.org/ontologies/2022/6/geological_taxonomy#Oolite -->

    <owl:Class rdf:about="http://www.semanticweb.org/ontologies/2022/6/geological_taxonomy#Oolite">
        <rdfs:subClassOf rdf:resource="http://www.semanticweb.org/ontologies/2022/6/geological_taxonomy#Sedimentary_rocks"/>
        <rdfs:comment>Sedimentary rock formed from ooids

Resource: https://en.wikipedia.org/wiki/List_of_rock_types</rdfs:comment>
    </owl:Class>
    


    <!-- http://www.semanticweb.org/ontologies/2022/6/geological_taxonomy#Organic_compounds -->

    <owl:Class rdf:about="http://www.semanticweb.org/ontologies/2022/6/geological_taxonomy#Organic_compounds">
        <rdfs:subClassOf rdf:resource="http://www.semanticweb.org/ontologies/2022/6/geological_taxonomy#Mineral"/>
        <rdfs:comment>The nitrate minerals are characterized by their triangular (NO3)– groups that resemble the (CO3)2– groups of the carbonates, making the two mineral classes similar in structure.	

Resource: https://www.britannica.com/science/nitrate-mineral</rdfs:comment>
    </owl:Class>
    


    <!-- http://www.semanticweb.org/ontologies/2022/6/geological_taxonomy#Orthels -->

    <owl:Class rdf:about="http://www.semanticweb.org/ontologies/2022/6/geological_taxonomy#Orthels">
        <rdfs:subClassOf rdf:resource="http://www.semanticweb.org/ontologies/2022/6/geological_taxonomy#Gelisols"/>
        <rdfs:comment>Soils that show little or no cryoturbation (less than one-third of the depth of the active layer)

Resource: https://en.wikipedia.org/wiki/Gelisol#Suborders</rdfs:comment>
    </owl:Class>
    


    <!-- http://www.semanticweb.org/ontologies/2022/6/geological_taxonomy#Orthents -->

    <owl:Class rdf:about="http://www.semanticweb.org/ontologies/2022/6/geological_taxonomy#Orthents">
        <rdfs:subClassOf rdf:resource="http://www.semanticweb.org/ontologies/2022/6/geological_taxonomy#Entisols"/>
        <rdfs:comment>Entisols lacking in pedogenic development

Resource: &quot;Illustrated Guide to Soil Taxonomy&quot; book by Unites States Department of Agriculture</rdfs:comment>
    </owl:Class>
    


    <!-- http://www.semanticweb.org/ontologies/2022/6/geological_taxonomy#Orthods -->

    <owl:Class rdf:about="http://www.semanticweb.org/ontologies/2022/6/geological_taxonomy#Orthods">
        <rdfs:subClassOf rdf:resource="http://www.semanticweb.org/ontologies/2022/6/geological_taxonomy#Spodosols"/>
        <rdfs:comment>Simple Spodosols with varying amounts of illuvial carbon, aluminum, and iron in the spodic horizon

Resource: &quot;Illustrated Guide to Soil Taxonomy&quot; book by Unites States Department of Agriculture</rdfs:comment>
    </owl:Class>
    


    <!-- http://www.semanticweb.org/ontologies/2022/6/geological_taxonomy#Outer_core -->

    <owl:Class rdf:about="http://www.semanticweb.org/ontologies/2022/6/geological_taxonomy#Outer_core">
        <rdfs:subClassOf rdf:resource="http://www.semanticweb.org/ontologies/2022/6/geological_taxonomy#Planetary_core"/>
        <owl:disjointWith rdf:resource="http://www.semanticweb.org/ontologies/2022/6/geological_taxonomy#Earth&apos;s_inner_core"/>
        <rdfs:comment>Earth&apos;s outer core is a fluid layer about 2,260 km (1,400 mi) thick, composed of mostly iron and nickel that lies above Earth&apos;s solid inner core and below its mantle. Pressure of 135–330GPa (from 1.3 to 3.3million atmospheres).

Resource: https://en.wikipedia.org/wiki/Earth%27s_outer_core</rdfs:comment>
    </owl:Class>
    


    <!-- http://www.semanticweb.org/ontologies/2022/6/geological_taxonomy#Overtopping_of_a_barrier -->

    <owl:Class rdf:about="http://www.semanticweb.org/ontologies/2022/6/geological_taxonomy#Overtopping_of_a_barrier">
        <rdfs:subClassOf rdf:resource="http://www.semanticweb.org/ontologies/2022/6/geological_taxonomy#Coastal_Flood"/>
        <rdfs:comment>the barrier may be natural or human-engineered and overtopping occurs due to swelling conditions during storms or high tides often on open stretches of the coast.	

Resource: https://en.wikipedia.org/wiki/Coastal_flooding</rdfs:comment>
    </owl:Class>
    


    <!-- http://www.semanticweb.org/ontologies/2022/6/geological_taxonomy#Oxides -->

    <owl:Class rdf:about="http://www.semanticweb.org/ontologies/2022/6/geological_taxonomy#Oxides">
        <rdfs:subClassOf rdf:resource="http://www.semanticweb.org/ontologies/2022/6/geological_taxonomy#Mineral"/>
        <rdfs:comment>The oxide mineral class includes those minerals in which the oxide anion (O2−) is bonded to one or more metal alloys.	

Resource: https://en.wikipedia.org/wiki/Oxide_mineral

Justification: Classified based on the combination of oxygen with one metal or more than one metals</rdfs:comment>
    </owl:Class>
    


    <!-- http://www.semanticweb.org/ontologies/2022/6/geological_taxonomy#Oxisols -->

    <owl:Class rdf:about="http://www.semanticweb.org/ontologies/2022/6/geological_taxonomy#Oxisols">
        <rdfs:subClassOf rdf:resource="http://www.semanticweb.org/ontologies/2022/6/geological_taxonomy#Soil"/>
        <rdfs:comment>The central concept of Oxisols is that of soils of the tropical and subtropical regions. They have gentle slopes on surfaces of great age.

Resource: https://www.nrcs.usda.gov/wps/portal/nrcs/detail/soils/survey/class/maps/?cid=nrcs142p2_053605

Justification: Depening upon soil moisture regime</rdfs:comment>
    </owl:Class>
    


    <!-- http://www.semanticweb.org/ontologies/2022/6/geological_taxonomy#Pantellerite -->

    <owl:Class rdf:about="http://www.semanticweb.org/ontologies/2022/6/geological_taxonomy#Pantellerite">
        <rdfs:subClassOf rdf:resource="http://www.semanticweb.org/ontologies/2022/6/geological_taxonomy#Rhyolite"/>
        <rdfs:comment>Pantellerite is a type of volcanic rock, specifically a peralkaline rhyolite. It has a higher iron and lower aluminium composition than comendite.

Resource: https://en.wikipedia.org/wiki/Pantellerite</rdfs:comment>
    </owl:Class>
    


    <!-- http://www.semanticweb.org/ontologies/2022/6/geological_taxonomy#Pegmatite -->

    <owl:Class rdf:about="http://www.semanticweb.org/ontologies/2022/6/geological_taxonomy#Pegmatite">
        <rdfs:subClassOf rdf:resource="http://www.semanticweb.org/ontologies/2022/6/geological_taxonomy#Igneous_rocks"/>
        <rdfs:comment>A pegmatite is an igneous rock showing a very coarse texture, with large interlocking crystals usually greater in size than 1 cm (0.4 in) and sometimes greater than 1 meter (3 ft).

Resource: https://en.wikipedia.org/wiki/Pegmatite</rdfs:comment>
    </owl:Class>
    


    <!-- http://www.semanticweb.org/ontologies/2022/6/geological_taxonomy#Peridotite -->

    <owl:Class rdf:about="http://www.semanticweb.org/ontologies/2022/6/geological_taxonomy#Peridotite">
        <rdfs:subClassOf rdf:resource="http://www.semanticweb.org/ontologies/2022/6/geological_taxonomy#Igneous_rocks"/>
        <rdfs:comment>Peridotite is a dense, coarse-grained igneous rock consisting mostly of the silicate minerals olivine and pyroxene.

Resource: https://en.wikipedia.org/wiki/Peridotite</rdfs:comment>
    </owl:Class>
    


    <!-- http://www.semanticweb.org/ontologies/2022/6/geological_taxonomy#Perox -->

    <owl:Class rdf:about="http://www.semanticweb.org/ontologies/2022/6/geological_taxonomy#Perox">
        <rdfs:subClassOf rdf:resource="http://www.semanticweb.org/ontologies/2022/6/geological_taxonomy#Oxisols"/>
        <rdfs:comment>Oxisols that have a perudic moisture regime

Resource: https://sites.google.com/site/dinpuithai/Home/key10/key10e</rdfs:comment>
    </owl:Class>
    


    <!-- http://www.semanticweb.org/ontologies/2022/6/geological_taxonomy#Phonolite -->

    <owl:Class rdf:about="http://www.semanticweb.org/ontologies/2022/6/geological_taxonomy#Phonolite">
        <rdfs:subClassOf rdf:resource="http://www.semanticweb.org/ontologies/2022/6/geological_taxonomy#Igneous_rocks"/>
        <rdfs:comment>Phonolite is an uncommon extrusive rock, of intermediate chemical composition between felsic and mafic, with texture ranging from aphanitic (fine-grained) to porphyritic.

Resource: https://en.wikipedia.org/wiki/Phonolite</rdfs:comment>
    </owl:Class>
    


    <!-- http://www.semanticweb.org/ontologies/2022/6/geological_taxonomy#Phonotephrite -->

    <owl:Class rdf:about="http://www.semanticweb.org/ontologies/2022/6/geological_taxonomy#Phonotephrite">
        <rdfs:subClassOf rdf:resource="http://www.semanticweb.org/ontologies/2022/6/geological_taxonomy#Igneous_rocks"/>
        <rdfs:comment>Phonotephrite is a strongly alkaline volcanic rock with a composition between phonolite and tephrite.

Resource: https://en.wikipedia.org/wiki/Phonotephrite</rdfs:comment>
    </owl:Class>
    


    <!-- http://www.semanticweb.org/ontologies/2022/6/geological_taxonomy#Phosphates_Arsenates_Vanadates -->

    <owl:Class rdf:about="http://www.semanticweb.org/ontologies/2022/6/geological_taxonomy#Phosphates_Arsenates_Vanadates">
        <rdfs:subClassOf rdf:resource="http://www.semanticweb.org/ontologies/2022/6/geological_taxonomy#Mineral"/>
        <rdfs:comment>Phosphate minerals contain the tetrahedrally coordinated phosphate anion along sometimes with arsenate and vanadate substitutions, and chloride, fluoride, and hydroxide anions that also fit into the crystal structure.	

Resource: https://en.wikipedia.org/wiki/Phosphate_mineral</rdfs:comment>
    </owl:Class>
    


    <!-- http://www.semanticweb.org/ontologies/2022/6/geological_taxonomy#Phosphorite -->

    <owl:Class rdf:about="http://www.semanticweb.org/ontologies/2022/6/geological_taxonomy#Phosphorite">
        <rdfs:subClassOf rdf:resource="http://www.semanticweb.org/ontologies/2022/6/geological_taxonomy#Sedimentary_rocks"/>
        <rdfs:comment>Phosphorite is a sedimentary rock containing significant amount of phosphate material.

Resource: https://www.sandatlas.org/rock-types/</rdfs:comment>
    </owl:Class>
    


    <!-- http://www.semanticweb.org/ontologies/2022/6/geological_taxonomy#Phyllite -->

    <owl:Class rdf:about="http://www.semanticweb.org/ontologies/2022/6/geological_taxonomy#Phyllite">
        <rdfs:subClassOf rdf:resource="http://www.semanticweb.org/ontologies/2022/6/geological_taxonomy#Metamorphic_rocks"/>
        <rdfs:comment>Type of foliated metamorphic rock – A low grade metamorphic rock composed mostly of micaceous minerals

Resource: https://en.wikipedia.org/wiki/Phyllite</rdfs:comment>
    </owl:Class>
    


    <!-- http://www.semanticweb.org/ontologies/2022/6/geological_taxonomy#Picrite -->

    <owl:Class rdf:about="http://www.semanticweb.org/ontologies/2022/6/geological_taxonomy#Picrite">
        <rdfs:subClassOf rdf:resource="http://www.semanticweb.org/ontologies/2022/6/geological_taxonomy#Igneous_rocks"/>
        <rdfs:comment>Picrite, intrusive igneous rock of ultramafic (very silica-poor) composition that is composed largely of olivine and augite and is somewhat similar to peridotite. Picrites are dark, heavy rocks and contain a small but variable amount of plagioclase feldspar; hornblende and biotite may also be present.

Resource: https://www.britannica.com/science/picrite</rdfs:comment>
    </owl:Class>
    


    <!-- http://www.semanticweb.org/ontologies/2022/6/geological_taxonomy#Planetary_core -->

    <owl:Class rdf:about="http://www.semanticweb.org/ontologies/2022/6/geological_taxonomy#Planetary_core">
        <rdfs:subClassOf rdf:resource="http://www.semanticweb.org/ontologies/2022/6/geological_taxonomy#Units_of_Earth_structure"/>
        <rdfs:comment>Innermost layers of a planet

Resource: https://en.wikipedia.org/wiki/Planetary_core

Justification: Classified based on temperature , pressure , radius</rdfs:comment>
    </owl:Class>
    


    <!-- http://www.semanticweb.org/ontologies/2022/6/geological_taxonomy#Porphyry -->

    <owl:Class rdf:about="http://www.semanticweb.org/ontologies/2022/6/geological_taxonomy#Porphyry">
        <rdfs:subClassOf rdf:resource="http://www.semanticweb.org/ontologies/2022/6/geological_taxonomy#Igneous_rocks"/>
        <rdfs:comment>Porphyry is a textural term for an igneous rock consisting of coarse-grained crystals such as feldspar or quartz dispersed in a fine-grained silicate-rich, generally aphanitic matrix or groundmass.

Resource: https://en.wikipedia.org/wiki/Porphyry_(geology)</rdfs:comment>
    </owl:Class>
    


    <!-- http://www.semanticweb.org/ontologies/2022/6/geological_taxonomy#Primary_rockfall -->

    <owl:Class rdf:about="http://www.semanticweb.org/ontologies/2022/6/geological_taxonomy#Primary_rockfall">
        <rdfs:subClassOf rdf:resource="http://www.semanticweb.org/ontologies/2022/6/geological_taxonomy#Rockfall"/>
        <owl:disjointWith rdf:resource="http://www.semanticweb.org/ontologies/2022/6/geological_taxonomy#Secondary_rockfall"/>
        <rdfs:comment>The material then descends mainly through the air by falling, bouncing, or rolling

Resource: https://en.wikipedia.org/wiki/Landslide_classification#Types_and_classification</rdfs:comment>
    </owl:Class>
    


    <!-- http://www.semanticweb.org/ontologies/2022/6/geological_taxonomy#Progressive_creep -->

    <owl:Class rdf:about="http://www.semanticweb.org/ontologies/2022/6/geological_taxonomy#Progressive_creep">
        <rdfs:subClassOf rdf:resource="http://www.semanticweb.org/ontologies/2022/6/geological_taxonomy#Creep"/>
        <rdfs:comment>Slopes are reaching the point of failure as other types of mass movements.

Resource: https://www.nature.scot/landforms-and-geology/scotlands-rocks-landforms-and-soils/landforms/landslides/types-landslide</rdfs:comment>
    </owl:Class>
    


    <!-- http://www.semanticweb.org/ontologies/2022/6/geological_taxonomy#Psamments -->

    <owl:Class rdf:about="http://www.semanticweb.org/ontologies/2022/6/geological_taxonomy#Psamments">
        <rdfs:subClassOf rdf:resource="http://www.semanticweb.org/ontologies/2022/6/geological_taxonomy#Entisols"/>
        <rdfs:comment>Entisols dominated by sandy textures

Resource: &quot;Illustrated Guide to Soil Taxonomy&quot; book by Unites States Department of Agriculture</rdfs:comment>
    </owl:Class>
    


    <!-- http://www.semanticweb.org/ontologies/2022/6/geological_taxonomy#Pseudotachylite -->

    <owl:Class rdf:about="http://www.semanticweb.org/ontologies/2022/6/geological_taxonomy#Pseudotachylite">
        <rdfs:subClassOf rdf:resource="http://www.semanticweb.org/ontologies/2022/6/geological_taxonomy#Metamorphic_rocks"/>
        <rdfs:comment>Pseudotachylyte or Pseudotachylite is a cohesive glassy or very fine-grained rock that occurs as veins and often contains inclusions of wall-rock fragments.

Resource: https://en.wikipedia.org/wiki/Pseudotachylite</rdfs:comment>
    </owl:Class>
    


    <!-- http://www.semanticweb.org/ontologies/2022/6/geological_taxonomy#Pumice -->

    <owl:Class rdf:about="http://www.semanticweb.org/ontologies/2022/6/geological_taxonomy#Pumice">
        <rdfs:subClassOf rdf:resource="http://www.semanticweb.org/ontologies/2022/6/geological_taxonomy#Igneous_rocks"/>
        <rdfs:comment>Pumice, called pumicite in its powdered or dust form, is a volcanic rock that consists of highly vesicular rough-textured volcanic glass, which may or may not contain crystals. It is typically light-colored.

Resource: https://en.wikipedia.org/wiki/Pumice</rdfs:comment>
    </owl:Class>
    


    <!-- http://www.semanticweb.org/ontologies/2022/6/geological_taxonomy#Pyroxenite -->

    <owl:Class rdf:about="http://www.semanticweb.org/ontologies/2022/6/geological_taxonomy#Pyroxenite">
        <rdfs:subClassOf rdf:resource="http://www.semanticweb.org/ontologies/2022/6/geological_taxonomy#Igneous_rocks"/>
        <rdfs:comment>Igneous rock - a coarse grained plutonic rock composed of &gt;90% pyroxene

Resource: https://en.wikipedia.org/wiki/Pyroxenite</rdfs:comment>
    </owl:Class>
    


    <!-- http://www.semanticweb.org/ontologies/2022/6/geological_taxonomy#Pāhoehoe -->

    <owl:Class rdf:about="http://www.semanticweb.org/ontologies/2022/6/geological_taxonomy#Pāhoehoe">
        <rdfs:subClassOf rdf:resource="http://www.semanticweb.org/ontologies/2022/6/geological_taxonomy#Basalt"/>
        <rdfs:comment>Basaltic lava with a flowing, often ropy appearance

Resource: https://en.wikipedia.org/wiki/P%C4%81hoehoe</rdfs:comment>
    </owl:Class>
    


    <!-- http://www.semanticweb.org/ontologies/2022/6/geological_taxonomy#Quartz_diorite -->

    <owl:Class rdf:about="http://www.semanticweb.org/ontologies/2022/6/geological_taxonomy#Quartz_diorite">
        <rdfs:subClassOf rdf:resource="http://www.semanticweb.org/ontologies/2022/6/geological_taxonomy#Igneous_rocks"/>
        <rdfs:comment>Igneous, plutonic rock – A diorite with &gt;5% modal quartz

Resource: https://en.wikipedia.org/wiki/Quartz_diorite</rdfs:comment>
    </owl:Class>
    


    <!-- http://www.semanticweb.org/ontologies/2022/6/geological_taxonomy#Quartz_monzonite -->

    <owl:Class rdf:about="http://www.semanticweb.org/ontologies/2022/6/geological_taxonomy#Quartz_monzonite">
        <rdfs:subClassOf rdf:resource="http://www.semanticweb.org/ontologies/2022/6/geological_taxonomy#Igneous_rocks"/>
        <rdfs:comment>Type of igneous rock – An intermediate plutonic rock, essentially a monzonite with 5–10% modal quartz

Resource: https://en.wikipedia.org/wiki/Quartz_monzonite</rdfs:comment>
    </owl:Class>
    


    <!-- http://www.semanticweb.org/ontologies/2022/6/geological_taxonomy#Quartzite -->

    <owl:Class rdf:about="http://www.semanticweb.org/ontologies/2022/6/geological_taxonomy#Quartzite">
        <rdfs:subClassOf rdf:resource="http://www.semanticweb.org/ontologies/2022/6/geological_taxonomy#Metamorphic_rocks"/>
        <rdfs:comment>A metamorphosed sandstone typically composed of &gt;95% quartz

Resource: https://geology.fandom.com/wiki/List_of_rock_types</rdfs:comment>
    </owl:Class>
    


    <!-- http://www.semanticweb.org/ontologies/2022/6/geological_taxonomy#Quartzolite -->

    <owl:Class rdf:about="http://www.semanticweb.org/ontologies/2022/6/geological_taxonomy#Quartzolite">
        <rdfs:subClassOf rdf:resource="http://www.semanticweb.org/ontologies/2022/6/geological_taxonomy#Igneous_rocks"/>
        <rdfs:comment>Extremely rare igneous rock made mostly of quartz – An intrusive rock composed mostly of quartz

Resource: https://en.wikipedia.org/wiki/Quartzolite</rdfs:comment>
    </owl:Class>
    


    <!-- http://www.semanticweb.org/ontologies/2022/6/geological_taxonomy#Rain -->

    <owl:Class rdf:about="http://www.semanticweb.org/ontologies/2022/6/geological_taxonomy#Rain">
        <rdfs:subClassOf rdf:resource="http://www.semanticweb.org/ontologies/2022/6/geological_taxonomy#Weather_conditions"/>
        <rdfs:comment>Rain is the condensed moisture of the atmosphere above falling under the form of liquid droplets. It is an extremely important phenomenon that allows life to flourish on continents

Resource: https://weather.fandom.com/wiki/Types_of_Weather#Rain</rdfs:comment>
    </owl:Class>
    


    <!-- http://www.semanticweb.org/ontologies/2022/6/geological_taxonomy#Rapakivi -->

    <owl:Class rdf:about="http://www.semanticweb.org/ontologies/2022/6/geological_taxonomy#Rapakivi">
        <rdfs:subClassOf rdf:resource="http://www.semanticweb.org/ontologies/2022/6/geological_taxonomy#Igneous_rocks"/>
        <rdfs:comment>Rapakivi is a variety of granite with K-feldspar phenocrysts that are mantled with plagioclase

Resource: https://www.sandatlas.org/rock-types/#Rapakivi</rdfs:comment>
    </owl:Class>
    


    <!-- http://www.semanticweb.org/ontologies/2022/6/geological_taxonomy#Rendolls -->

    <owl:Class rdf:about="http://www.semanticweb.org/ontologies/2022/6/geological_taxonomy#Rendolls">
        <rdfs:subClassOf rdf:resource="http://www.semanticweb.org/ontologies/2022/6/geological_taxonomy#Mollisols"/>
        <rdfs:comment>Rendolls are shallow and stony soils formed on limestone and have an udic Soil moisture regime

Resource: https://www.sciencedirect.com/topics/agricultural-and-biological-sciences/mollisol</rdfs:comment>
    </owl:Class>
    


    <!-- http://www.semanticweb.org/ontologies/2022/6/geological_taxonomy#Rhomb-porphyry -->

    <owl:Class rdf:about="http://www.semanticweb.org/ontologies/2022/6/geological_taxonomy#Rhomb-porphyry">
        <rdfs:subClassOf rdf:resource="http://www.semanticweb.org/ontologies/2022/6/geological_taxonomy#Igneous_rocks"/>
        <rdfs:comment>Rhomb-porphyry is a porphyritic igneous rock with abundant wedge- or lens-shaped anorthoclase (feldspar) phenocrysts. Rhomb-porphyry is a rare rock type.

Resource: https://www.sandatlas.org/rhomb-porphyry/</rdfs:comment>
    </owl:Class>
    


    <!-- http://www.semanticweb.org/ontologies/2022/6/geological_taxonomy#Rhyodacite -->

    <owl:Class rdf:about="http://www.semanticweb.org/ontologies/2022/6/geological_taxonomy#Rhyodacite">
        <rdfs:subClassOf rdf:resource="http://www.semanticweb.org/ontologies/2022/6/geological_taxonomy#Igneous_rocks"/>
        <rdfs:comment>Volcanic rock rich in silica and low in alkali metal oxides – A felsic volcanic rock which is intermediate between a rhyolite and a dacite

Resource: https://en.wikipedia.org/wiki/Rhyodacite</rdfs:comment>
    </owl:Class>
    


    <!-- http://www.semanticweb.org/ontologies/2022/6/geological_taxonomy#Rhyolite -->

    <owl:Class rdf:about="http://www.semanticweb.org/ontologies/2022/6/geological_taxonomy#Rhyolite">
        <rdfs:subClassOf rdf:resource="http://www.semanticweb.org/ontologies/2022/6/geological_taxonomy#Igneous_rocks"/>
        <rdfs:comment>Rhyolite is the most silica-rich of volcanic rocks. It is generally glassy or fine-grained (aphanitic) in texture, but may be porphyritic, containing larger mineral crystals (phenocrysts) in an otherwise fine-grained groundmass.

Resource: https://en.wikipedia.org/wiki/Rhyolite

Justification: Depending upon the composition of iron and aluminium.</rdfs:comment>
    </owl:Class>
    


    <!-- http://www.semanticweb.org/ontologies/2022/6/geological_taxonomy#Rock -->

    <owl:Class rdf:about="http://www.semanticweb.org/ontologies/2022/6/geological_taxonomy#Rock">
        <rdfs:subClassOf rdf:resource="http://www.semanticweb.org/ontologies/2022/6/geological_taxonomy#Geological_Object"/>
        <rdfs:comment>In geology, a rock (or stone) is any naturally occurring solid mass or aggregate of minerals or mineraloid matter without any chemical composition

Resource: https://en.wikipedia.org/wiki/Rock_(geology)

Justification: Depending upon the mode of their formation</rdfs:comment>
    </owl:Class>
    


    <!-- http://www.semanticweb.org/ontologies/2022/6/geological_taxonomy#Rock_Gypsum- -->

    <owl:Class rdf:about="http://www.semanticweb.org/ontologies/2022/6/geological_taxonomy#Rock_Gypsum-">
        <rdfs:subClassOf rdf:resource="http://www.semanticweb.org/ontologies/2022/6/geological_taxonomy#Sedimentary_rocks"/>
        <rdfs:comment>Rock gypsum (a.k.a. gyprock) is a chemical sedimentary rock.  It is an example of an evaporite - it forms by the evaporation of water (usually seawater) and the precipitation of dissolved minerals.

Resource: http://www.jsjgeology.net/Rock-gypsum.htm</rdfs:comment>
    </owl:Class>
    


    <!-- http://www.semanticweb.org/ontologies/2022/6/geological_taxonomy#Rock_slide -->

    <owl:Class rdf:about="http://www.semanticweb.org/ontologies/2022/6/geological_taxonomy#Rock_slide">
        <rdfs:subClassOf rdf:resource="http://www.semanticweb.org/ontologies/2022/6/geological_taxonomy#Block_slide"/>
        <rdfs:comment>sliding of rock material down a mountain

Resource: https://www.geologyin.com/2015/02/types-of-wasting-slump-rockslide-debris.html</rdfs:comment>
    </owl:Class>
    


    <!-- http://www.semanticweb.org/ontologies/2022/6/geological_taxonomy#Rock_topple -->

    <owl:Class rdf:about="http://www.semanticweb.org/ontologies/2022/6/geological_taxonomy#Rock_topple">
        <rdfs:subClassOf rdf:resource="http://www.semanticweb.org/ontologies/2022/6/geological_taxonomy#Topple"/>
        <rdfs:comment>A topple is the forward rotation, out of the slope, of a mass of soil and rock about a point or axis below the centre of gravity of the displaced mass.

Resource: http://www.ukgeohazards.info/pages/eng_geol/landslide_geohazard/eng_geol_landslides_rocktopple_index.htm</rdfs:comment>
    </owl:Class>
    


    <!-- http://www.semanticweb.org/ontologies/2022/6/geological_taxonomy#Rockfall -->

    <owl:Class rdf:about="http://www.semanticweb.org/ontologies/2022/6/geological_taxonomy#Rockfall">
        <rdfs:subClassOf rdf:resource="http://www.semanticweb.org/ontologies/2022/6/geological_taxonomy#Fall"/>
        <rdfs:comment>A rockfall is a quantity of rock that has fallen freely from a cliff face.

Resource: https://en.wikipedia.org/wiki/Rockfall

Justification: Classified based on how detaching of bodies happen</rdfs:comment>
    </owl:Class>
    


    <!-- http://www.semanticweb.org/ontologies/2022/6/geological_taxonomy#Rotational_slide -->

    <owl:Class rdf:about="http://www.semanticweb.org/ontologies/2022/6/geological_taxonomy#Rotational_slide">
        <rdfs:subClassOf rdf:resource="http://www.semanticweb.org/ontologies/2022/6/geological_taxonomy#Slide"/>
        <owl:disjointWith rdf:resource="http://www.semanticweb.org/ontologies/2022/6/geological_taxonomy#Translational_slide"/>
        <rdfs:comment>Rotational slides move along a surface of rupture that is curved and concave

Resource: https://en.wikipedia.org/wiki/Landslide_classification#Types_and_classification</rdfs:comment>
    </owl:Class>
    


    <!-- http://www.semanticweb.org/ontologies/2022/6/geological_taxonomy#Salids -->

    <owl:Class rdf:about="http://www.semanticweb.org/ontologies/2022/6/geological_taxonomy#Salids">
        <rdfs:subClassOf rdf:resource="http://www.semanticweb.org/ontologies/2022/6/geological_taxonomy#Aridisols"/>
        <rdfs:comment>Characterized by accumulation of salts more soluble than gypsum; the typical soils of the playas or desert depressions, or closed basins.

Resource: https://www.sciencedirect.com/topics/agricultural-and-biological-sciences/aridisol</rdfs:comment>
    </owl:Class>
    


    <!-- http://www.semanticweb.org/ontologies/2022/6/geological_taxonomy#Sandstone -->

    <owl:Class rdf:about="http://www.semanticweb.org/ontologies/2022/6/geological_taxonomy#Sandstone">
        <rdfs:subClassOf rdf:resource="http://www.semanticweb.org/ontologies/2022/6/geological_taxonomy#Sedimentary_rocks"/>
        <rdfs:comment>A clastic sedimentary rock defined by its grain size

Resource: https://geology.fandom.com/wiki/List_of_rock_types</rdfs:comment>
    </owl:Class>
    


    <!-- http://www.semanticweb.org/ontologies/2022/6/geological_taxonomy#Saprists -->

    <owl:Class rdf:about="http://www.semanticweb.org/ontologies/2022/6/geological_taxonomy#Saprists">
        <rdfs:subClassOf rdf:resource="http://www.semanticweb.org/ontologies/2022/6/geological_taxonomy#Histosols"/>
        <rdfs:comment>Histosols that are primarily made up of highly decomposed organic materials, often called muck.

Resource: https://en.wikipedia.org/wiki/Histosol</rdfs:comment>
    </owl:Class>
    


    <!-- http://www.semanticweb.org/ontologies/2022/6/geological_taxonomy#Schist -->

    <owl:Class rdf:about="http://www.semanticweb.org/ontologies/2022/6/geological_taxonomy#Schist">
        <rdfs:subClassOf rdf:resource="http://www.semanticweb.org/ontologies/2022/6/geological_taxonomy#Metamorphic_rocks"/>
        <rdfs:comment>Schist is a medium-grained metamorphic rock showing pronounced schistosity.

Resource: https://en.wikipedia.org/wiki/Schist</rdfs:comment>
    </owl:Class>
    


    <!-- http://www.semanticweb.org/ontologies/2022/6/geological_taxonomy#Scoria -->

    <owl:Class rdf:about="http://www.semanticweb.org/ontologies/2022/6/geological_taxonomy#Scoria">
        <rdfs:subClassOf rdf:resource="http://www.semanticweb.org/ontologies/2022/6/geological_taxonomy#Igneous_rocks"/>
        <rdfs:comment>Scoria is a pyroclastic, highly vesicular, dark-colored volcanic rock that was ejected from a volcano as a molten blob and cooled in the air to form discrete grains or clasts.

Resource: https://en.wikipedia.org/wiki/Scoria</rdfs:comment>
    </owl:Class>
    


    <!-- http://www.semanticweb.org/ontologies/2022/6/geological_taxonomy#Seasonal_creep -->

    <owl:Class rdf:about="http://www.semanticweb.org/ontologies/2022/6/geological_taxonomy#Seasonal_creep">
        <rdfs:subClassOf rdf:resource="http://www.semanticweb.org/ontologies/2022/6/geological_taxonomy#Creep"/>
        <rdfs:comment>Movement is within the depth of soil affected by seasonal changes in soil moisture and soil temperature

Resource: https://courses.lumenlearning.com/geo/chapter/reading-slump-and-creep/</rdfs:comment>
    </owl:Class>
    


    <!-- http://www.semanticweb.org/ontologies/2022/6/geological_taxonomy#Secondary_rockfall -->

    <owl:Class rdf:about="http://www.semanticweb.org/ontologies/2022/6/geological_taxonomy#Secondary_rockfall">
        <rdfs:subClassOf rdf:resource="http://www.semanticweb.org/ontologies/2022/6/geological_taxonomy#Rockfall"/>
        <rdfs:comment>Secondary falls involves rock bodies already physically detached from cliff and merely lodged upon it

Resource: https://en.wikipedia.org/wiki/Landslide_classification#Types_and_classification</rdfs:comment>
    </owl:Class>
    


    <!-- http://www.semanticweb.org/ontologies/2022/6/geological_taxonomy#Sedimentary_rocks -->

    <owl:Class rdf:about="http://www.semanticweb.org/ontologies/2022/6/geological_taxonomy#Sedimentary_rocks">
        <rdfs:subClassOf rdf:resource="http://www.semanticweb.org/ontologies/2022/6/geological_taxonomy#Rock"/>
        <rdfs:comment>Sedimentary rocks are types of rock that are formed by the accumulation or deposition of mineral or organic particles at Earth&apos;s surface, followed by cementation.

Resource: https://en.wikipedia.org/wiki/Sedimentary_rock

Justification: depending upon the composition of different minerals and amount of organic material</rdfs:comment>
    </owl:Class>
    


    <!-- http://www.semanticweb.org/ontologies/2022/6/geological_taxonomy#Serpentinite -->

    <owl:Class rdf:about="http://www.semanticweb.org/ontologies/2022/6/geological_taxonomy#Serpentinite">
        <rdfs:subClassOf rdf:resource="http://www.semanticweb.org/ontologies/2022/6/geological_taxonomy#Metamorphic_rocks"/>
        <rdfs:comment>Serpentinite is a rock composed of one or more serpentine group minerals, the name originating from the similarity of the texture of the rock to that of the skin of a snake.

Resource: https://en.wikipedia.org/wiki/Serpentinite</rdfs:comment>
    </owl:Class>
    


    <!-- http://www.semanticweb.org/ontologies/2022/6/geological_taxonomy#Severe_Drought -->

    <owl:Class rdf:about="http://www.semanticweb.org/ontologies/2022/6/geological_taxonomy#Severe_Drought">
        <rdfs:subClassOf rdf:resource="http://www.semanticweb.org/ontologies/2022/6/geological_taxonomy#Drought"/>
        <rdfs:comment>It is D2 category and causes water shortages

Resource: https://droughtmonitor.unl.edu/About/WhatistheUSDM.aspx</rdfs:comment>
    </owl:Class>
    


    <!-- http://www.semanticweb.org/ontologies/2022/6/geological_taxonomy#Shale -->

    <owl:Class rdf:about="http://www.semanticweb.org/ontologies/2022/6/geological_taxonomy#Shale">
        <rdfs:subClassOf rdf:resource="http://www.semanticweb.org/ontologies/2022/6/geological_taxonomy#Sedimentary_rocks"/>
        <rdfs:comment>Shale is a fine-grained, clastic sedimentary rock formed from mud that is a mix of flakes of clay minerals and tiny fragments (silt-sized particles) of other minerals, especially quartz and calcite.

Resource: https://en.wikipedia.org/wiki/Shale</rdfs:comment>
    </owl:Class>
    


    <!-- http://www.semanticweb.org/ontologies/2022/6/geological_taxonomy#Shonkinite -->

    <owl:Class rdf:about="http://www.semanticweb.org/ontologies/2022/6/geological_taxonomy#Shonkinite">
        <rdfs:subClassOf rdf:resource="http://www.semanticweb.org/ontologies/2022/6/geological_taxonomy#Igneous_rocks"/>
        <rdfs:comment>Shonkinite is an intrusive igneous rock found in few places in the world. It is unique in having low silica, feldspathoid minerals, and large blocky crystals of black augite.

Resource: https://en.wikipedia.org/wiki/Shonkinite</rdfs:comment>
    </owl:Class>
    


    <!-- http://www.semanticweb.org/ontologies/2022/6/geological_taxonomy#Shoshonite -->

    <owl:Class rdf:about="http://www.semanticweb.org/ontologies/2022/6/geological_taxonomy#Shoshonite">
        <rdfs:subClassOf rdf:resource="http://www.semanticweb.org/ontologies/2022/6/geological_taxonomy#Trachyandesite"/>
        <rdfs:comment>Shoshonite is a potassium-rich variety of basaltic trachyandesite, composed of olivine, augite and plagioclase phenocrysts in a groundmass with calcic plagioclase and sanidine and some dark-colored volcanic glass.

Resource: https://en.wikipedia.org/wiki/List_of_rock_types</rdfs:comment>
    </owl:Class>
    


    <!-- http://www.semanticweb.org/ontologies/2022/6/geological_taxonomy#Shungite -->

    <owl:Class rdf:about="http://www.semanticweb.org/ontologies/2022/6/geological_taxonomy#Shungite">
        <rdfs:subClassOf rdf:resource="http://www.semanticweb.org/ontologies/2022/6/geological_taxonomy#Metamorphic_rocks"/>
        <rdfs:comment>Shungite is a metamorphosed oil shale consisting of structureless carbon.

Resource: https://www.sandatlas.org/rock-types/</rdfs:comment>
    </owl:Class>
    


    <!-- http://www.semanticweb.org/ontologies/2022/6/geological_taxonomy#Silicates -->

    <owl:Class rdf:about="http://www.semanticweb.org/ontologies/2022/6/geological_taxonomy#Silicates">
        <rdfs:subClassOf rdf:resource="http://www.semanticweb.org/ontologies/2022/6/geological_taxonomy#Mineral"/>
        <rdfs:comment>Silicate minerals are rock-forming minerals made up of silicate groups.	

Resource: https://en.wikipedia.org/wiki/Silicate_mineral

Justification: Classified according to structural configuration, which arises from the sharing of one, two, three, or all oxygen ions of a tetrahedron.
https://www.britannica.com/science/mineral-chemical-compound/Silicates</rdfs:comment>
    </owl:Class>
    


    <!-- http://www.semanticweb.org/ontologies/2022/6/geological_taxonomy#Siltstone -->

    <owl:Class rdf:about="http://www.semanticweb.org/ontologies/2022/6/geological_taxonomy#Siltstone">
        <rdfs:subClassOf rdf:resource="http://www.semanticweb.org/ontologies/2022/6/geological_taxonomy#Sedimentary_rocks"/>
        <rdfs:comment>A clastic sedimentary rock defined by its grain size

Resource: https://geology.fandom.com/wiki/List_of_rock_types</rdfs:comment>
    </owl:Class>
    


    <!-- http://www.semanticweb.org/ontologies/2022/6/geological_taxonomy#Skarn -->

    <owl:Class rdf:about="http://www.semanticweb.org/ontologies/2022/6/geological_taxonomy#Skarn">
        <rdfs:subClassOf rdf:resource="http://www.semanticweb.org/ontologies/2022/6/geological_taxonomy#Metamorphic_rocks"/>
        <rdfs:comment>Skarns or tactites are hard, coarse-grained metamorphic rocks that form by a process called metasomatism.

Resource: https://en.wikipedia.org/wiki/Skarn</rdfs:comment>
    </owl:Class>
    


    <!-- http://www.semanticweb.org/ontologies/2022/6/geological_taxonomy#Slate -->

    <owl:Class rdf:about="http://www.semanticweb.org/ontologies/2022/6/geological_taxonomy#Slate">
        <rdfs:subClassOf rdf:resource="http://www.semanticweb.org/ontologies/2022/6/geological_taxonomy#Metamorphic_rocks"/>
        <rdfs:comment>Slate is a fine-grained, foliated, homogeneous metamorphic rock derived from an original shale-type sedimentary rock composed of clay or volcanic ash through low-grade regional metamorphism.

Resource: https://en.wikipedia.org/wiki/Slate</rdfs:comment>
    </owl:Class>
    


    <!-- http://www.semanticweb.org/ontologies/2022/6/geological_taxonomy#Slide -->

    <owl:Class rdf:about="http://www.semanticweb.org/ontologies/2022/6/geological_taxonomy#Slide">
        <rdfs:subClassOf rdf:resource="http://www.semanticweb.org/ontologies/2022/6/geological_taxonomy#Landslide"/>
        <rdfs:comment>A slide is a downslope movement of soil or rock mass occurring dominantly on the surface of rupture or on relatively thin zones of intense shear strain

Resource: https://en.wikipedia.org/wiki/Landslide_classification#Types_and_classification

Justification: Classified based on how the land of mass slides</rdfs:comment>
    </owl:Class>
    


    <!-- http://www.semanticweb.org/ontologies/2022/6/geological_taxonomy#Snow -->

    <owl:Class rdf:about="http://www.semanticweb.org/ontologies/2022/6/geological_taxonomy#Snow">
        <rdfs:subClassOf rdf:resource="http://www.semanticweb.org/ontologies/2022/6/geological_taxonomy#Weather_conditions"/>
        <rdfs:comment>Snow is atmospheric water that froze and fell to the ground, covering it. It happens when the temperature of the air falls at 0 °C (32 °F). Snow remains as long as the temperature of the ground doesn&apos;t go beyond 0 °C (32 °F).

Resource: https://weather.fandom.com/wiki/Types_of_Weather#Snow</rdfs:comment>
    </owl:Class>
    


    <!-- http://www.semanticweb.org/ontologies/2022/6/geological_taxonomy#Soapstone -->

    <owl:Class rdf:about="http://www.semanticweb.org/ontologies/2022/6/geological_taxonomy#Soapstone">
        <rdfs:subClassOf rdf:resource="http://www.semanticweb.org/ontologies/2022/6/geological_taxonomy#Talc_carbonate"/>
        <rdfs:comment>Soapstone is a soft rock composed of talc with other silicates like micas, pyroxene, amphibole, chlorite, etc.

Resource: https://www.sandatlas.org/rock-types/</rdfs:comment>
    </owl:Class>
    


    <!-- http://www.semanticweb.org/ontologies/2022/6/geological_taxonomy#Soil -->

    <owl:Class rdf:about="http://www.semanticweb.org/ontologies/2022/6/geological_taxonomy#Soil">
        <rdfs:subClassOf rdf:resource="http://www.semanticweb.org/ontologies/2022/6/geological_taxonomy#Geological_Object"/>
        <rdfs:comment>Soil, also commonly referred to as earth or dirt, is a mixture of organic matter, minerals, gases, liquids, and organisms that together support life.Soil consists of a solid phase of minerals and organic matter (the soil matrix), as well as a porous phase that holds gases (the soil atmosphere) and water (the soil solution).

Resource: https://en.wikipedia.org/wiki/Soil

Justification: Categorized based on the soil properties like depth, moisture, temperature, texture, structure, cation exchange capacity, base saturation, clay mineralogy, organic matter content and salt content. 
https://en.wikipedia.org/wiki/USDA_soil_taxonomy</rdfs:comment>
    </owl:Class>
    


    <!-- http://www.semanticweb.org/ontologies/2022/6/geological_taxonomy#Sovite -->

    <owl:Class rdf:about="http://www.semanticweb.org/ontologies/2022/6/geological_taxonomy#Sovite">
        <rdfs:subClassOf rdf:resource="http://www.semanticweb.org/ontologies/2022/6/geological_taxonomy#Igneous_rocks"/>
        <rdfs:comment>Sövite is a type of plutonic carbonatite where the dominant carbonate mineral is calcite. Sövite is the most common variety of carbonatite.

Resource: https://www.sandatlas.org/rock-types/#S%C3%B6vite</rdfs:comment>
    </owl:Class>
    


    <!-- http://www.semanticweb.org/ontologies/2022/6/geological_taxonomy#Spodosols -->

    <owl:Class rdf:about="http://www.semanticweb.org/ontologies/2022/6/geological_taxonomy#Spodosols">
        <rdfs:subClassOf rdf:resource="http://www.semanticweb.org/ontologies/2022/6/geological_taxonomy#Soil"/>
        <rdfs:comment>The central concept of Spodosols is that of soils in which amorphous mixtures of organic matter and aluminum, with or without iron, have accumulated.

Resource: https://www.nrcs.usda.gov/wps/portal/nrcs/detail/soils/survey/class/maps/?cid=nrcs142p2_053607

Justification: Based on soil wetness, cold soil temperatures, spodic horizons dominated by illuvial accumulation of organic matter, and varying amounts of illuvial carbon, aluminum, and iron in the spodic horizons
&quot;Illustrated Guide to Soil Taxonomy&quot; book by Unites States Department of Agriculture</rdfs:comment>
    </owl:Class>
    


    <!-- http://www.semanticweb.org/ontologies/2022/6/geological_taxonomy#Stormy -->

    <owl:Class rdf:about="http://www.semanticweb.org/ontologies/2022/6/geological_taxonomy#Stormy">
        <rdfs:subClassOf rdf:resource="http://www.semanticweb.org/ontologies/2022/6/geological_taxonomy#Weather_conditions"/>
        <rdfs:comment>A storm is any disturbed state of the natural environment or the atmosphere of an astronomical body. It may be marked by significant disruptions to normal conditions such as strong wind, tornadoes, hail, thunder and lightning (a thunderstorm), heavy precipitation (snowstorm, rainstorm), heavy freezing rain (ice storm), strong winds (tropical cyclone, windstorm), wind transporting some substance through the atmosphere such as in a dust storm, among other forms of severe weather.

Resource: https://en.wikipedia.org/wiki/Storm</rdfs:comment>
    </owl:Class>
    


    <!-- http://www.semanticweb.org/ontologies/2022/6/geological_taxonomy#Subsidence -->

    <owl:Class rdf:about="http://www.semanticweb.org/ontologies/2022/6/geological_taxonomy#Subsidence">
        <rdfs:subClassOf rdf:resource="http://www.semanticweb.org/ontologies/2022/6/geological_taxonomy#Landslide"/>
        <rdfs:comment>Subsidence is a general term for downward vertical movement of the Earth&apos;s surface, which can be caused by both natural processes and human activities.</rdfs:comment>
    </owl:Class>
    


    <!-- http://www.semanticweb.org/ontologies/2022/6/geological_taxonomy#Suevite -->

    <owl:Class rdf:about="http://www.semanticweb.org/ontologies/2022/6/geological_taxonomy#Suevite">
        <rdfs:subClassOf rdf:resource="http://www.semanticweb.org/ontologies/2022/6/geological_taxonomy#Metamorphic_rocks"/>
        <rdfs:comment>Suevite is a rock consisting partly of melted material, typically forming a breccia containing glass and crystal or lithic fragments, formed during an impact event.

Resource: https://en.wikipedia.org/wiki/Suevite</rdfs:comment>
    </owl:Class>
    


    <!-- http://www.semanticweb.org/ontologies/2022/6/geological_taxonomy#Sulfates -->

    <owl:Class rdf:about="http://www.semanticweb.org/ontologies/2022/6/geological_taxonomy#Sulfates">
        <rdfs:subClassOf rdf:resource="http://www.semanticweb.org/ontologies/2022/6/geological_taxonomy#Mineral"/>
        <rdfs:comment>The sulfate minerals are a class of minerals that include the sulfate ion within their structure.	

Resource: https://en.wikipedia.org/wiki/Sulfate_mineral

Justification: Classification depending upon presence of water in the chemical structure</rdfs:comment>
    </owl:Class>
    


    <!-- http://www.semanticweb.org/ontologies/2022/6/geological_taxonomy#Sulfides_and_Sulfosalts -->

    <owl:Class rdf:about="http://www.semanticweb.org/ontologies/2022/6/geological_taxonomy#Sulfides_and_Sulfosalts">
        <rdfs:subClassOf rdf:resource="http://www.semanticweb.org/ontologies/2022/6/geological_taxonomy#Mineral"/>
        <rdfs:comment>The sulfide minerals are a class of minerals containing sulfide or disulfide as the major anion.	

Resource: https://en.wikipedia.org/wiki/Sulfide_mineral</rdfs:comment>
    </owl:Class>
    


    <!-- http://www.semanticweb.org/ontologies/2022/6/geological_taxonomy#Sunny -->

    <owl:Class rdf:about="http://www.semanticweb.org/ontologies/2022/6/geological_taxonomy#Sunny">
        <rdfs:subClassOf rdf:resource="http://www.semanticweb.org/ontologies/2022/6/geological_taxonomy#Weather_conditions"/>
        <rdfs:comment>A sunny day, or clear sky during nighttime, is when there are clouds above the horizon.

Resource: https://weather.fandom.com/wiki/Types_of_Weather#Sunny/Clear</rdfs:comment>
    </owl:Class>
    


    <!-- http://www.semanticweb.org/ontologies/2022/6/geological_taxonomy#Surface_Fire -->

    <owl:Class rdf:about="http://www.semanticweb.org/ontologies/2022/6/geological_taxonomy#Surface_Fire">
        <rdfs:subClassOf rdf:resource="http://www.semanticweb.org/ontologies/2022/6/geological_taxonomy#Wildfire"/>
        <rdfs:comment>A surface fire refers to a fire that ranges from low to high intensity depending on the conditions.  burn on the surface of the ground and are primarily fueled by low-lying vegetation such as twigs or dried leaves.	

Resource: https://www.supplycache.com/blogs/news/the-different-types-of-wildland-fires</rdfs:comment>
    </owl:Class>
    


    <!-- http://www.semanticweb.org/ontologies/2022/6/geological_taxonomy#Syenite -->

    <owl:Class rdf:about="http://www.semanticweb.org/ontologies/2022/6/geological_taxonomy#Syenite">
        <rdfs:subClassOf rdf:resource="http://www.semanticweb.org/ontologies/2022/6/geological_taxonomy#Igneous_rocks"/>
        <rdfs:comment>Intrusive igneous rock – A plutonic rock dominated by orthoclase feldspar; a type of granitoid

Resource: https://en.wikipedia.org/wiki/Syenite</rdfs:comment>
    </owl:Class>
    


    <!-- http://www.semanticweb.org/ontologies/2022/6/geological_taxonomy#Sylvinite -->

    <owl:Class rdf:about="http://www.semanticweb.org/ontologies/2022/6/geological_taxonomy#Sylvinite">
        <rdfs:subClassOf rdf:resource="http://www.semanticweb.org/ontologies/2022/6/geological_taxonomy#Sedimentary_rocks"/>
        <rdfs:comment>A sedimentary rock made of a mechanical mixture of sylvite and halite

Resource: https://en.wikipedia.org/wiki/List_of_rock_types</rdfs:comment>
    </owl:Class>
    


    <!-- http://www.semanticweb.org/ontologies/2022/6/geological_taxonomy#Sövite -->

    <owl:Class rdf:about="http://www.semanticweb.org/ontologies/2022/6/geological_taxonomy#Sövite">
        <rdfs:subClassOf rdf:resource="http://www.semanticweb.org/ontologies/2022/6/geological_taxonomy#Igneous_rocks"/>
        <rdfs:comment>Sovite (or sövite) is the coarse-grained variety (or facies) of carbonatite, an intrusive, igneous rock. 

Resource: https://en.wikipedia.org/wiki/Sovite</rdfs:comment>
    </owl:Class>
    


    <!-- http://www.semanticweb.org/ontologies/2022/6/geological_taxonomy#Tachylyte -->

    <owl:Class rdf:about="http://www.semanticweb.org/ontologies/2022/6/geological_taxonomy#Tachylyte">
        <rdfs:subClassOf rdf:resource="http://www.semanticweb.org/ontologies/2022/6/geological_taxonomy#Igneous_rocks"/>
        <rdfs:comment>Tachylite is a form of basaltic volcanic glass. This glass is formed naturally by the rapid cooling of molten basalt. It is a type of mafic igneous rock.

Resource: https://en.wikipedia.org/wiki/Tachylite</rdfs:comment>
    </owl:Class>
    


    <!-- http://www.semanticweb.org/ontologies/2022/6/geological_taxonomy#Talc_carbonate -->

    <owl:Class rdf:about="http://www.semanticweb.org/ontologies/2022/6/geological_taxonomy#Talc_carbonate">
        <rdfs:subClassOf rdf:resource="http://www.semanticweb.org/ontologies/2022/6/geological_taxonomy#Metamorphic_rocks"/>
        <rdfs:comment>Talc carbonates are a suite of rock and mineral compositions found in metamorphosed ultramafic rocks.

Resource: https://en.wikipedia.org/wiki/Talc_carbonate

Justification: Depending upon the amounts of chlorite and amphiboles</rdfs:comment>
    </owl:Class>
    


    <!-- http://www.semanticweb.org/ontologies/2022/6/geological_taxonomy#Tectonic_Earthquake -->

    <owl:Class rdf:about="http://www.semanticweb.org/ontologies/2022/6/geological_taxonomy#Tectonic_Earthquake">
        <rdfs:subClassOf rdf:resource="http://www.semanticweb.org/ontologies/2022/6/geological_taxonomy#Earthquake"/>
        <rdfs:comment>Tectonic earthquakes are produced by sudden movement along faults and plate boundaries.

Resource: https://www.phivolcs.dost.gov.ph/index.php/earthquake/introduction-to-earthquake

Justification: depending upon where the earthquake takes place considering the plates</rdfs:comment>
    </owl:Class>
    


    <!-- http://www.semanticweb.org/ontologies/2022/6/geological_taxonomy#Tectonite -->

    <owl:Class rdf:about="http://www.semanticweb.org/ontologies/2022/6/geological_taxonomy#Tectonite">
        <rdfs:subClassOf rdf:resource="http://www.semanticweb.org/ontologies/2022/6/geological_taxonomy#Metamorphic_rocks"/>
        <rdfs:comment>Tectonites are metamorphic or tectonically deformed rocks whose fabric reflects the history of their deformation, or rocks with fabric that clearly displays coordinated geometric features that indicate continuous solid (ductile) flow during formation.

Resource: https://en.wikipedia.org/wiki/Tectonite</rdfs:comment>
    </owl:Class>
    


    <!-- http://www.semanticweb.org/ontologies/2022/6/geological_taxonomy#Teletsunami -->

    <owl:Class rdf:about="http://www.semanticweb.org/ontologies/2022/6/geological_taxonomy#Teletsunami">
        <rdfs:subClassOf rdf:resource="http://www.semanticweb.org/ontologies/2022/6/geological_taxonomy#Tsunami"/>
        <rdfs:comment>waves generated more then 1000 kilometers from the affected shore. 	

Resource: http://www.sfu.ca/geog355fall01/cobryne/types_of_tsunamis.html</rdfs:comment>
    </owl:Class>
    


    <!-- http://www.semanticweb.org/ontologies/2022/6/geological_taxonomy#Tephriphonolite -->

    <owl:Class rdf:about="http://www.semanticweb.org/ontologies/2022/6/geological_taxonomy#Tephriphonolite">
        <rdfs:subClassOf rdf:resource="http://www.semanticweb.org/ontologies/2022/6/geological_taxonomy#Igneous_rocks"/>
        <rdfs:comment>Tephriphonolite is a mafic to intermediate extrusive igneous rock in composition between phonotephrite and phonolite.[1] It contains 9 to 14% alkali content and 48 to 57% silica content.

Resource: https://en.wikipedia.org/wiki/Tephriphonolite</rdfs:comment>
    </owl:Class>
    


    <!-- http://www.semanticweb.org/ontologies/2022/6/geological_taxonomy#Tephrite -->

    <owl:Class rdf:about="http://www.semanticweb.org/ontologies/2022/6/geological_taxonomy#Tephrite">
        <rdfs:subClassOf rdf:resource="http://www.semanticweb.org/ontologies/2022/6/geological_taxonomy#Igneous_rocks"/>
        <rdfs:comment>Tephrite is an igneous, volcanic (extrusive) rock, with aphanitic to porphyritic texture

Resource: https://en.wikipedia.org/wiki/Tephrite</rdfs:comment>
    </owl:Class>
    


    <!-- http://www.semanticweb.org/ontologies/2022/6/geological_taxonomy#Tillite -->

    <owl:Class rdf:about="http://www.semanticweb.org/ontologies/2022/6/geological_taxonomy#Tillite">
        <rdfs:subClassOf rdf:resource="http://www.semanticweb.org/ontologies/2022/6/geological_taxonomy#Sedimentary_rocks"/>
        <rdfs:comment>Tillite is a poorly sorted glacial sedimentary rock — consolidated glacial till.

Resource: https://www.sandatlas.org/rock-types/</rdfs:comment>
    </owl:Class>
    


    <!-- http://www.semanticweb.org/ontologies/2022/6/geological_taxonomy#Tonalite -->

    <owl:Class rdf:about="http://www.semanticweb.org/ontologies/2022/6/geological_taxonomy#Tonalite">
        <rdfs:subClassOf rdf:resource="http://www.semanticweb.org/ontologies/2022/6/geological_taxonomy#Igneous_rocks"/>
        <rdfs:comment>Tonalite is an igneous, plutonic (intrusive) rock, of felsic composition, with phaneritic (coarse-grained) texture.

Resource: https://en.wikipedia.org/wiki/Tonalite</rdfs:comment>
    </owl:Class>
    


    <!-- http://www.semanticweb.org/ontologies/2022/6/geological_taxonomy#Topple -->

    <owl:Class rdf:about="http://www.semanticweb.org/ontologies/2022/6/geological_taxonomy#Topple">
        <rdfs:subClassOf rdf:resource="http://www.semanticweb.org/ontologies/2022/6/geological_taxonomy#Landslide"/>
        <rdfs:comment>Toppling is the forward rotation out of the slope of a mass of soil or rock about a point or axis below the centre of gravity of the displaced mass.

Resource: https://en.wikipedia.org/wiki/Landslide_classification#Types_and_classification

Justification: Divided based on type of material</rdfs:comment>
    </owl:Class>
    


    <!-- http://www.semanticweb.org/ontologies/2022/6/geological_taxonomy#Torrands -->

    <owl:Class rdf:about="http://www.semanticweb.org/ontologies/2022/6/geological_taxonomy#Torrands">
        <rdfs:subClassOf rdf:resource="http://www.semanticweb.org/ontologies/2022/6/geological_taxonomy#Andisols"/>
        <rdfs:comment>Andisols that have an aridic moisture regime. 

Resource: https://sites.google.com/site/dinpuithai/Home/key10/key10d</rdfs:comment>
    </owl:Class>
    


    <!-- http://www.semanticweb.org/ontologies/2022/6/geological_taxonomy#Torrerts -->

    <owl:Class rdf:about="http://www.semanticweb.org/ontologies/2022/6/geological_taxonomy#Torrerts">
        <rdfs:subClassOf rdf:resource="http://www.semanticweb.org/ontologies/2022/6/geological_taxonomy#Vertisols"/>
        <rdfs:comment>Vertisols that, if not irrigated during the year, have cracks in normal years that remain closed for less than 60 consecutive days during a period when the soil temperature at a depth of 50 cm from the soil surface is higher than 8 oC.

Resource: https://sites.google.com/site/dinpuithai/Home/key10/key10f</rdfs:comment>
    </owl:Class>
    


    <!-- http://www.semanticweb.org/ontologies/2022/6/geological_taxonomy#Torrox -->

    <owl:Class rdf:about="http://www.semanticweb.org/ontologies/2022/6/geological_taxonomy#Torrox">
        <rdfs:subClassOf rdf:resource="http://www.semanticweb.org/ontologies/2022/6/geological_taxonomy#Oxisols"/>
        <rdfs:comment>Oxisols that have an aridic moisture regime

Resource: https://sites.google.com/site/dinpuithai/Home/key10/key10e</rdfs:comment>
    </owl:Class>
    


    <!-- http://www.semanticweb.org/ontologies/2022/6/geological_taxonomy#Trachyandesite -->

    <owl:Class rdf:about="http://www.semanticweb.org/ontologies/2022/6/geological_taxonomy#Trachyandesite">
        <rdfs:subClassOf rdf:resource="http://www.semanticweb.org/ontologies/2022/6/geological_taxonomy#Igneous_rocks"/>
        <rdfs:comment>Trachyandesite is an extrusive igneous rock with a composition between trachyte and andesite.

Resource: https://en.wikipedia.org/wiki/Trachyandesite

Justification: divided into sodium-rich benmoreite and potassium-rich latite.</rdfs:comment>
    </owl:Class>
    


    <!-- http://www.semanticweb.org/ontologies/2022/6/geological_taxonomy#Trachybasalt -->

    <owl:Class rdf:about="http://www.semanticweb.org/ontologies/2022/6/geological_taxonomy#Trachybasalt">
        <rdfs:subClassOf rdf:resource="http://www.semanticweb.org/ontologies/2022/6/geological_taxonomy#Igneous_rocks"/>
        <rdfs:comment>Trachybasalt is a volcanic rock with a composition between trachyte and basalt. It resembles basalt but has a high content of alkali metal oxides.

Resource: https://en.wikipedia.org/wiki/Trachybasalt</rdfs:comment>
    </owl:Class>
    


    <!-- http://www.semanticweb.org/ontologies/2022/6/geological_taxonomy#Trachyte -->

    <owl:Class rdf:about="http://www.semanticweb.org/ontologies/2022/6/geological_taxonomy#Trachyte">
        <rdfs:subClassOf rdf:resource="http://www.semanticweb.org/ontologies/2022/6/geological_taxonomy#Igneous_rocks"/>
        <rdfs:comment>Trachyte is an extrusive igneous rock composed mostly of alkali feldspar.

Resource: https://en.wikipedia.org/wiki/Trachyte</rdfs:comment>
    </owl:Class>
    


    <!-- http://www.semanticweb.org/ontologies/2022/6/geological_taxonomy#Translational_slide -->

    <owl:Class rdf:about="http://www.semanticweb.org/ontologies/2022/6/geological_taxonomy#Translational_slide">
        <rdfs:subClassOf rdf:resource="http://www.semanticweb.org/ontologies/2022/6/geological_taxonomy#Slide"/>
        <rdfs:comment>In translational slides the mass displaces along a planar or undulating surface of rupture, sliding out over the original ground surface.

Resource: https://en.wikipedia.org/wiki/Landslide_classification#Types_and_classification</rdfs:comment>
    </owl:Class>
    


    <!-- http://www.semanticweb.org/ontologies/2022/6/geological_taxonomy#Travertine -->

    <owl:Class rdf:about="http://www.semanticweb.org/ontologies/2022/6/geological_taxonomy#Travertine">
        <rdfs:subClassOf rdf:resource="http://www.semanticweb.org/ontologies/2022/6/geological_taxonomy#Sedimentary_rocks"/>
        <rdfs:comment>A sedimentary rock containing calcite and iron oxides

Resource: https://geology.fandom.com/wiki/List_of_rock_types</rdfs:comment>
    </owl:Class>
    


    <!-- http://www.semanticweb.org/ontologies/2022/6/geological_taxonomy#Troctolite -->

    <owl:Class rdf:about="http://www.semanticweb.org/ontologies/2022/6/geological_taxonomy#Troctolite">
        <rdfs:subClassOf rdf:resource="http://www.semanticweb.org/ontologies/2022/6/geological_taxonomy#Igneous_rocks"/>
        <rdfs:comment>Troctolite is a mafic intrusive rock type. It consists essentially of major but variable amounts of olivine and calcic plagioclase along with minor pyroxene.

Resource: https://en.wikipedia.org/wiki/Troctolite</rdfs:comment>
    </owl:Class>
    


    <!-- http://www.semanticweb.org/ontologies/2022/6/geological_taxonomy#Trondhjemite -->

    <owl:Class rdf:about="http://www.semanticweb.org/ontologies/2022/6/geological_taxonomy#Trondhjemite">
        <rdfs:subClassOf rdf:resource="http://www.semanticweb.org/ontologies/2022/6/geological_taxonomy#Igneous_rocks"/>
        <rdfs:comment>Light-colored intrusive igneous rock – A form of tonalite where plagioclase-group feldspar is oligoclase

Resource: https://en.wikipedia.org/wiki/Trondhjemite</rdfs:comment>
    </owl:Class>
    


    <!-- http://www.semanticweb.org/ontologies/2022/6/geological_taxonomy#Tropical_Depression -->

    <owl:Class rdf:about="http://www.semanticweb.org/ontologies/2022/6/geological_taxonomy#Tropical_Depression">
        <rdfs:subClassOf rdf:resource="http://www.semanticweb.org/ontologies/2022/6/geological_taxonomy#Tropical_cyclone"/>
        <rdfs:comment>A tropical cyclone with maximum sustained winds of 38 mph (33 knots) or less

Resource: https://www.nhc.noaa.gov/climo/</rdfs:comment>
    </owl:Class>
    


    <!-- http://www.semanticweb.org/ontologies/2022/6/geological_taxonomy#Tropical_Storm -->

    <owl:Class rdf:about="http://www.semanticweb.org/ontologies/2022/6/geological_taxonomy#Tropical_Storm">
        <rdfs:subClassOf rdf:resource="http://www.semanticweb.org/ontologies/2022/6/geological_taxonomy#Tropical_cyclone"/>
        <rdfs:comment>A tropical cyclone with maximum sustained winds of 39 to 73 mph (34 to 63 knots).	

Resource: https://www.nhc.noaa.gov/climo/</rdfs:comment>
    </owl:Class>
    


    <!-- http://www.semanticweb.org/ontologies/2022/6/geological_taxonomy#Tropical_cyclone -->

    <owl:Class rdf:about="http://www.semanticweb.org/ontologies/2022/6/geological_taxonomy#Tropical_cyclone">
        <rdfs:subClassOf rdf:resource="http://www.semanticweb.org/ontologies/2022/6/geological_taxonomy#Cyclone"/>
        <rdfs:comment>Tropical cyclones originate only over the seas.

Resource: https://www.insightsonindia.com/world-geography/physical-geography-of-the-world/climatology/cyclones-and-anticyclones/difference-between-extratropical-and-tropical-cyclones/#:~:text=Extratropical%20cyclones%20cover%20a%20larger,compared%20to%20the%20tropical%20cyclone.

Justification: depending upon speed and region
https://www.nhc.noaa.gov/climo/</rdfs:comment>
    </owl:Class>
    


    <!-- http://www.semanticweb.org/ontologies/2022/6/geological_taxonomy#Tsunami -->

    <owl:Class rdf:about="http://www.semanticweb.org/ontologies/2022/6/geological_taxonomy#Tsunami">
        <rdfs:subClassOf rdf:resource="http://www.semanticweb.org/ontologies/2022/6/geological_taxonomy#Natural_disaster"/>
        <rdfs:comment>series of waves in a water body caused by the displacement of a large volume of water, generally in an ocean or a large lake.	

Resource: https://en.wikipedia.org/wiki/Tsunami

Justification: catagorized by the magnitude of the largest wave of the set
http://www.sfu.ca/geog355fall01/cobryne/types_of_tsunamis.html</rdfs:comment>
    </owl:Class>
    


    <!-- http://www.semanticweb.org/ontologies/2022/6/geological_taxonomy#Tufa -->

    <owl:Class rdf:about="http://www.semanticweb.org/ontologies/2022/6/geological_taxonomy#Tufa">
        <rdfs:subClassOf rdf:resource="http://www.semanticweb.org/ontologies/2022/6/geological_taxonomy#Sedimentary_rocks"/>
        <rdfs:comment>Tufa is a highly porous, sedimentary rock (limestone) composed of calcium carbonate, CaCO3. It is formed by biological and chemical precipitation of Calcite or aragonite from cold, supersaturated surface or ground waters.

Resource: http://chc.sbg.ac.at/sri/thesaurus/node.php?id=58</rdfs:comment>
    </owl:Class>
    


    <!-- http://www.semanticweb.org/ontologies/2022/6/geological_taxonomy#Tuff -->

    <owl:Class rdf:about="http://www.semanticweb.org/ontologies/2022/6/geological_taxonomy#Tuff">
        <rdfs:subClassOf rdf:resource="http://www.semanticweb.org/ontologies/2022/6/geological_taxonomy#Igneous_rocks"/>
        <rdfs:comment>Tuff is an igneous rock that forms from the products of an explosive volcanic eruption. In these eruptions, the volcano blasts rock, ash, magma and other materials from its vent.

Resource: https://geology.com/rocks/tuff.shtml</rdfs:comment>
    </owl:Class>
    


    <!-- http://www.semanticweb.org/ontologies/2022/6/geological_taxonomy#Turbels -->

    <owl:Class rdf:about="http://www.semanticweb.org/ontologies/2022/6/geological_taxonomy#Turbels">
        <rdfs:subClassOf rdf:resource="http://www.semanticweb.org/ontologies/2022/6/geological_taxonomy#Gelisols"/>
        <rdfs:comment>Gelisols that have one or more horizons showing cryoturbation in the form of irregular, broken, or distorted horizon boundaries, involutions, the accumulation of organic matter on top of the permafrost, ice or sand wedges, and oriented rock fragments.

Resource: https://sites.google.com/site/dinpuithai/Home/key10/key10a
https://acsess.onlinelibrary.wiley.com/doi/full/10.2136/sh2013-54-4-gc</rdfs:comment>
    </owl:Class>
    


    <!-- http://www.semanticweb.org/ontologies/2022/6/geological_taxonomy#Turbidite -->

    <owl:Class rdf:about="http://www.semanticweb.org/ontologies/2022/6/geological_taxonomy#Turbidite">
        <rdfs:subClassOf rdf:resource="http://www.semanticweb.org/ontologies/2022/6/geological_taxonomy#Sedimentary_rocks"/>
        <rdfs:comment>A particular sequence of sedimentary rocks which form within the deep ocean environment

Resource: https://geology.fandom.com/wiki/List_of_rock_types</rdfs:comment>
    </owl:Class>
    


    <!-- http://www.semanticweb.org/ontologies/2022/6/geological_taxonomy#Udalfs -->

    <owl:Class rdf:about="http://www.semanticweb.org/ontologies/2022/6/geological_taxonomy#Udalfs">
        <rdfs:subClassOf rdf:resource="http://www.semanticweb.org/ontologies/2022/6/geological_taxonomy#Alfisols"/>
        <rdfs:comment>Alfisols which are located in humid or subhumid climates.

Resource: https://en.wikipedia.org/wiki/Alfisol#Suborders</rdfs:comment>
    </owl:Class>
    


    <!-- http://www.semanticweb.org/ontologies/2022/6/geological_taxonomy#Udands -->

    <owl:Class rdf:about="http://www.semanticweb.org/ontologies/2022/6/geological_taxonomy#Udands">
        <rdfs:subClassOf rdf:resource="http://www.semanticweb.org/ontologies/2022/6/geological_taxonomy#Andisols"/>
        <rdfs:comment>Andisols of humid climates.

Resource: https://en.wikipedia.org/wiki/Andisol</rdfs:comment>
    </owl:Class>
    


    <!-- http://www.semanticweb.org/ontologies/2022/6/geological_taxonomy#Udepts -->

    <owl:Class rdf:about="http://www.semanticweb.org/ontologies/2022/6/geological_taxonomy#Udepts">
        <rdfs:subClassOf rdf:resource="http://www.semanticweb.org/ontologies/2022/6/geological_taxonomy#Inceptisols"/>
        <rdfs:comment>Inceptisols that have a udic soil moisture regime.

Resource: https://sites.google.com/site/dinpuithai/Home/taxonomy/k-inceptisols/kg</rdfs:comment>
    </owl:Class>
    


    <!-- http://www.semanticweb.org/ontologies/2022/6/geological_taxonomy#Uderts -->

    <owl:Class rdf:about="http://www.semanticweb.org/ontologies/2022/6/geological_taxonomy#Uderts">
        <rdfs:subClassOf rdf:resource="http://www.semanticweb.org/ontologies/2022/6/geological_taxonomy#Vertisols"/>
        <rdfs:comment>Vertisols with seasonal cracking pattern indicative of a udic
moisture regime (seasonally well-distributed rainfall)

Resource: &quot;Illustrated Guide to Soil Taxonomy&quot; book by Unites States Department of Agriculture</rdfs:comment>
    </owl:Class>
    


    <!-- http://www.semanticweb.org/ontologies/2022/6/geological_taxonomy#Udolls -->

    <owl:Class rdf:about="http://www.semanticweb.org/ontologies/2022/6/geological_taxonomy#Udolls">
        <rdfs:subClassOf rdf:resource="http://www.semanticweb.org/ontologies/2022/6/geological_taxonomy#Mollisols"/>
        <rdfs:comment>Udolls have an udic Soil Moisture Regime

Resource: https://www.sciencedirect.com/topics/agricultural-and-biological-sciences/mollisol</rdfs:comment>
    </owl:Class>
    


    <!-- http://www.semanticweb.org/ontologies/2022/6/geological_taxonomy#Udox -->

    <owl:Class rdf:about="http://www.semanticweb.org/ontologies/2022/6/geological_taxonomy#Udox">
        <rdfs:subClassOf rdf:resource="http://www.semanticweb.org/ontologies/2022/6/geological_taxonomy#Oxisols"/>
        <rdfs:comment>Udox are well drained Oxisols with a udic soil moisture regime.

Resource: https://www.nrcs.usda.gov/wps/portal/nrcs/detail/soils/survey/class/maps/?cid=nrcs142p2_053606</rdfs:comment>
    </owl:Class>
    


    <!-- http://www.semanticweb.org/ontologies/2022/6/geological_taxonomy#Udults -->

    <owl:Class rdf:about="http://www.semanticweb.org/ontologies/2022/6/geological_taxonomy#Udults">
        <rdfs:subClassOf rdf:resource="http://www.semanticweb.org/ontologies/2022/6/geological_taxonomy#Ultisols"/>
        <rdfs:comment>Ultisols that have a udic moisture regime.

Resource: https://sites.google.com/site/dinpuithai/Home/key10/key10h</rdfs:comment>
    </owl:Class>
    


    <!-- http://www.semanticweb.org/ontologies/2022/6/geological_taxonomy#Ultisols -->

    <owl:Class rdf:about="http://www.semanticweb.org/ontologies/2022/6/geological_taxonomy#Ultisols">
        <rdfs:subClassOf rdf:resource="http://www.semanticweb.org/ontologies/2022/6/geological_taxonomy#Soil"/>
        <rdfs:comment>The central concept of Ultisols is that of soils that have a horizon that contains an appreciable amount of translocated silicate clay (an argillic or kandic horizon) and few bases (base saturation less than 35 percent).

Resource: https://www.nrcs.usda.gov/wps/portal/nrcs/detail/soils/survey/class/maps/?cid=nrcs142p2_053609

Justification: Depending upon soil moisture regime and different horizons</rdfs:comment>
    </owl:Class>
    


    <!-- http://www.semanticweb.org/ontologies/2022/6/geological_taxonomy#Umber -->

    <owl:Class rdf:about="http://www.semanticweb.org/ontologies/2022/6/geological_taxonomy#Umber">
        <rdfs:subClassOf rdf:resource="http://www.semanticweb.org/ontologies/2022/6/geological_taxonomy#Sedimentary_rocks"/>
        <rdfs:comment>Umber is a marine sediment associated with black smokers.

Resource: https://www.sandatlas.org/rock-types/</rdfs:comment>
    </owl:Class>
    


    <!-- http://www.semanticweb.org/ontologies/2022/6/geological_taxonomy#Units_of_Earth_structure -->

    <owl:Class rdf:about="http://www.semanticweb.org/ontologies/2022/6/geological_taxonomy#Units_of_Earth_structure">
        <rdfs:subClassOf rdf:resource="http://www.semanticweb.org/ontologies/2022/6/geological_taxonomy#Geological_entities"/>
        <rdfs:comment>inner structure of the planet Earth, consisting of several concentric spherical layers

Resource: https://en.wikipedia.org/wiki/Structure_of_Earth

Justification: Layers are classified based on chemical composition</rdfs:comment>
    </owl:Class>
    


    <!-- http://www.semanticweb.org/ontologies/2022/6/geological_taxonomy#Upper_mantle -->

    <owl:Class rdf:about="http://www.semanticweb.org/ontologies/2022/6/geological_taxonomy#Upper_mantle">
        <rdfs:subClassOf rdf:resource="http://www.semanticweb.org/ontologies/2022/6/geological_taxonomy#Mantle"/>
        <rdfs:comment>The upper mantle of Earth is a very thick layer of rock inside the planet, which begins just beneath the crust and ends at the top of the lower mantle

Resource: https://en.wikipedia.org/wiki/Upper_mantle_(Earth)

Justification: Classified based on different mechanical properties</rdfs:comment>
    </owl:Class>
    


    <!-- http://www.semanticweb.org/ontologies/2022/6/geological_taxonomy#Ustalfs -->

    <owl:Class rdf:about="http://www.semanticweb.org/ontologies/2022/6/geological_taxonomy#Ustalfs">
        <rdfs:subClassOf rdf:resource="http://www.semanticweb.org/ontologies/2022/6/geological_taxonomy#Alfisols"/>
        <rdfs:comment>Alfisols that have an ustic moisture regime.

Resource: https://sites.google.com/site/dinpuithai/Home/taxonomy/j-alfisols</rdfs:comment>
    </owl:Class>
    


    <!-- http://www.semanticweb.org/ontologies/2022/6/geological_taxonomy#Ustands -->

    <owl:Class rdf:about="http://www.semanticweb.org/ontologies/2022/6/geological_taxonomy#Ustands">
        <rdfs:subClassOf rdf:resource="http://www.semanticweb.org/ontologies/2022/6/geological_taxonomy#Andisols"/>
        <rdfs:comment>Andisols that have an ustic moisture regime.

Resource: https://sites.google.com/site/dinpuithai/Home/key10/key10d</rdfs:comment>
    </owl:Class>
    


    <!-- http://www.semanticweb.org/ontologies/2022/6/geological_taxonomy#Ustepts -->

    <owl:Class rdf:about="http://www.semanticweb.org/ontologies/2022/6/geological_taxonomy#Ustepts">
        <rdfs:subClassOf rdf:resource="http://www.semanticweb.org/ontologies/2022/6/geological_taxonomy#Inceptisols"/>
        <rdfs:comment>Inceptisols that have an ustic soil moisture regime

Resource: https://sites.google.com/site/dinpuithai/Home/key10/key10k</rdfs:comment>
    </owl:Class>
    


    <!-- http://www.semanticweb.org/ontologies/2022/6/geological_taxonomy#Usterts -->

    <owl:Class rdf:about="http://www.semanticweb.org/ontologies/2022/6/geological_taxonomy#Usterts">
        <rdfs:subClassOf rdf:resource="http://www.semanticweb.org/ontologies/2022/6/geological_taxonomy#Vertisols"/>
        <rdfs:comment>Vertisols that, if not irrigated during the year, have cracks in normal years that are 5 mm or more wide, through a thickness of 25 cm or more within 50 cm of the mineral soil surface, for 90 or more cumulative days per year.

Resource: https://sites.google.com/site/dinpuithai/Home/key10/key10f</rdfs:comment>
    </owl:Class>
    


    <!-- http://www.semanticweb.org/ontologies/2022/6/geological_taxonomy#Ustolls -->

    <owl:Class rdf:about="http://www.semanticweb.org/ontologies/2022/6/geological_taxonomy#Ustolls">
        <rdfs:subClassOf rdf:resource="http://www.semanticweb.org/ontologies/2022/6/geological_taxonomy#Mollisols"/>
        <rdfs:comment>Ustolls have an ustic or an aridic Soil Moisture Regime

Resource: https://www.sciencedirect.com/topics/agricultural-and-biological-sciences/mollisol</rdfs:comment>
    </owl:Class>
    


    <!-- http://www.semanticweb.org/ontologies/2022/6/geological_taxonomy#Ustox -->

    <owl:Class rdf:about="http://www.semanticweb.org/ontologies/2022/6/geological_taxonomy#Ustox">
        <rdfs:subClassOf rdf:resource="http://www.semanticweb.org/ontologies/2022/6/geological_taxonomy#Oxisols"/>
        <rdfs:comment>Oxisols that have an ustic or xeric moisture regime

Resource: https://sites.google.com/site/dinpuithai/Home/key10/key10e</rdfs:comment>
    </owl:Class>
    


    <!-- http://www.semanticweb.org/ontologies/2022/6/geological_taxonomy#Ustults -->

    <owl:Class rdf:about="http://www.semanticweb.org/ontologies/2022/6/geological_taxonomy#Ustults">
        <rdfs:subClassOf rdf:resource="http://www.semanticweb.org/ontologies/2022/6/geological_taxonomy#Ultisols"/>
        <rdfs:comment>Ultisols that have an ustic moisture regime

Resource: https://sites.google.com/site/dinpuithai/Home/key10/key10h</rdfs:comment>
    </owl:Class>
    


    <!-- http://www.semanticweb.org/ontologies/2022/6/geological_taxonomy#Vertisols -->

    <owl:Class rdf:about="http://www.semanticweb.org/ontologies/2022/6/geological_taxonomy#Vertisols">
        <rdfs:subClassOf rdf:resource="http://www.semanticweb.org/ontologies/2022/6/geological_taxonomy#Soil"/>
        <rdfs:comment>The central concept of Vertisols is that of soils that have a high content of expanding clay and that have at some time of the year deep wide cracks.

Resource: https://www.nrcs.usda.gov/wps/portal/nrcs/detail/soils/survey/class/maps/?cid=nrcs142p2_053611

Justification: Based on moisture regime and one is based on temperature regime</rdfs:comment>
    </owl:Class>
    


    <!-- http://www.semanticweb.org/ontologies/2022/6/geological_taxonomy#Vitrands -->

    <owl:Class rdf:about="http://www.semanticweb.org/ontologies/2022/6/geological_taxonomy#Vitrands">
        <rdfs:subClassOf rdf:resource="http://www.semanticweb.org/ontologies/2022/6/geological_taxonomy#Andisols"/>
        <rdfs:comment>Andisols that have a 1500 kPa water retention of less than 15 percent on air-dried samples and less than 30 percent on undried samples throughout 60 percent or more of the thickness.
Relatively young Andisols that are coarse-textured and dominated by glass.

Resource: https://sites.google.com/site/dinpuithai/Home/key10/key10d
https://en.wikipedia.org/wiki/Andisol</rdfs:comment>
    </owl:Class>
    


    <!-- http://www.semanticweb.org/ontologies/2022/6/geological_taxonomy#Volcanic_Earthquake -->

    <owl:Class rdf:about="http://www.semanticweb.org/ontologies/2022/6/geological_taxonomy#Volcanic_Earthquake">
        <rdfs:subClassOf rdf:resource="http://www.semanticweb.org/ontologies/2022/6/geological_taxonomy#Earthquake"/>
        <rdfs:comment>Earthquakes induced by rising lava or magma beneath active volcanoes is called volcanic earthquakes.

Resource: https://www.phivolcs.dost.gov.ph/index.php/earthquake/introduction-to-earthquake</rdfs:comment>
    </owl:Class>
    


    <!-- http://www.semanticweb.org/ontologies/2022/6/geological_taxonomy#Wackestone -->

    <owl:Class rdf:about="http://www.semanticweb.org/ontologies/2022/6/geological_taxonomy#Wackestone">
        <rdfs:subClassOf rdf:resource="http://www.semanticweb.org/ontologies/2022/6/geological_taxonomy#Sedimentary_rocks"/>
        <rdfs:comment>A matrix-supported carbonate sedimentary rock.

Resource: https://geology.fandom.com/wiki/List_of_rock_types</rdfs:comment>
    </owl:Class>
    


    <!-- http://www.semanticweb.org/ontologies/2022/6/geological_taxonomy#Weather_conditions -->

    <owl:Class rdf:about="http://www.semanticweb.org/ontologies/2022/6/geological_taxonomy#Weather_conditions">
        <rdfs:subClassOf rdf:resource="http://www.semanticweb.org/ontologies/2022/6/geological_taxonomy#Geological_phenomena"/>
        <rdfs:comment>The atmospheric conditions that comprise the state of the atmosphere in terms of temperature and wind and clouds and precipitation

Resource: https://www.vocabulary.com/dictionary/weather%20condition

Justification: Classified based on the different conditions of the earth’s atmosphere.</rdfs:comment>
    </owl:Class>
    


    <!-- http://www.semanticweb.org/ontologies/2022/6/geological_taxonomy#Websterite -->

    <owl:Class rdf:about="http://www.semanticweb.org/ontologies/2022/6/geological_taxonomy#Websterite">
        <rdfs:subClassOf rdf:resource="http://www.semanticweb.org/ontologies/2022/6/geological_taxonomy#Igneous_rocks"/>
        <rdfs:comment>Websterite is ultramafic igneous rock that consists of roughly equal proportions of orthopyroxene and clinopyroxene. 

Resource: https://en.wikipedia.org/wiki/Websterite</rdfs:comment>
    </owl:Class>
    


    <!-- http://www.semanticweb.org/ontologies/2022/6/geological_taxonomy#Wehrlite -->

    <owl:Class rdf:about="http://www.semanticweb.org/ontologies/2022/6/geological_taxonomy#Wehrlite">
        <rdfs:subClassOf rdf:resource="http://www.semanticweb.org/ontologies/2022/6/geological_taxonomy#Igneous_rocks"/>
        <rdfs:comment>Wehrlite is an ultramafic and ultrabasic rock that is a mixture of olivine and clinopyroxene.

Resource: https://en.wikipedia.org/wiki/Wehrlite</rdfs:comment>
    </owl:Class>
    


    <!-- http://www.semanticweb.org/ontologies/2022/6/geological_taxonomy#Whiteschist -->

    <owl:Class rdf:about="http://www.semanticweb.org/ontologies/2022/6/geological_taxonomy#Whiteschist">
        <rdfs:subClassOf rdf:resource="http://www.semanticweb.org/ontologies/2022/6/geological_taxonomy#Metamorphic_rocks"/>
        <rdfs:comment>A whiteschist is an uncommon metamorphic rock formed at high to ultra-high pressures.

Resource: https://en.wikipedia.org/wiki/Whiteschist</rdfs:comment>
    </owl:Class>
    


    <!-- http://www.semanticweb.org/ontologies/2022/6/geological_taxonomy#Wildfire -->

    <owl:Class rdf:about="http://www.semanticweb.org/ontologies/2022/6/geological_taxonomy#Wildfire">
        <rdfs:subClassOf rdf:resource="http://www.semanticweb.org/ontologies/2022/6/geological_taxonomy#Natural_disaster"/>
        <rdfs:comment>A wildfire, forest fire, bushfire, wildland fire or rural fire is an unplanned, uncontrolled and unpredictable fire in an area of combustible vegetation starting in rural and urban areas.	

Resource: https://en.wikipedia.org/wiki/Wildfire

Justification: Classification based on the type of vegetation that fuels them and intensity of the wildfire</rdfs:comment>
    </owl:Class>
    


    <!-- http://www.semanticweb.org/ontologies/2022/6/geological_taxonomy#Windy -->

    <owl:Class rdf:about="http://www.semanticweb.org/ontologies/2022/6/geological_taxonomy#Windy">
        <rdfs:subClassOf rdf:resource="http://www.semanticweb.org/ontologies/2022/6/geological_taxonomy#Weather_conditions"/>
        <rdfs:comment>Wind can be defined as air under motion. Air moves whenever there’s an imbalance between the pressure in any two locations.

Resource: https://outforia.com/types-of-weather/</rdfs:comment>
    </owl:Class>
    


    <!-- http://www.semanticweb.org/ontologies/2022/6/geological_taxonomy#Xeralfs -->

    <owl:Class rdf:about="http://www.semanticweb.org/ontologies/2022/6/geological_taxonomy#Xeralfs">
        <rdfs:subClassOf rdf:resource="http://www.semanticweb.org/ontologies/2022/6/geological_taxonomy#Alfisols"/>
        <rdfs:comment>Alfisols that have a xeric moisture regime

Resource: https://sites.google.com/site/dinpuithai/Home/taxonomy/j-alfisols</rdfs:comment>
    </owl:Class>
    


    <!-- http://www.semanticweb.org/ontologies/2022/6/geological_taxonomy#Xerands -->

    <owl:Class rdf:about="http://www.semanticweb.org/ontologies/2022/6/geological_taxonomy#Xerands">
        <rdfs:subClassOf rdf:resource="http://www.semanticweb.org/ontologies/2022/6/geological_taxonomy#Andisols"/>
        <rdfs:comment>Andisols that have a xeric moisture regime.

Resource: https://sites.google.com/site/dinpuithai/Home/key10/key10d</rdfs:comment>
    </owl:Class>
    


    <!-- http://www.semanticweb.org/ontologies/2022/6/geological_taxonomy#Xerepts -->

    <owl:Class rdf:about="http://www.semanticweb.org/ontologies/2022/6/geological_taxonomy#Xerepts">
        <rdfs:subClassOf rdf:resource="http://www.semanticweb.org/ontologies/2022/6/geological_taxonomy#Inceptisols"/>
        <rdfs:comment>Inceptisols that have a xeric soil moisture regime.

Resource: https://sites.google.com/site/dinpuithai/Home/key10/key10k</rdfs:comment>
    </owl:Class>
    


    <!-- http://www.semanticweb.org/ontologies/2022/6/geological_taxonomy#Xererts -->

    <owl:Class rdf:about="http://www.semanticweb.org/ontologies/2022/6/geological_taxonomy#Xererts">
        <rdfs:subClassOf rdf:resource="http://www.semanticweb.org/ontologies/2022/6/geological_taxonomy#Vertisols"/>
        <rdfs:comment>They have a thermic, mesic, or frigid soil temperature regime. They show cracks that are open at least 60 consecutive days during the summer, but are closed at least 60 consecutive days during winter.

Resource: https://en.wikipedia.org/wiki/Vertisol</rdfs:comment>
    </owl:Class>
    


    <!-- http://www.semanticweb.org/ontologies/2022/6/geological_taxonomy#Xerolls -->

    <owl:Class rdf:about="http://www.semanticweb.org/ontologies/2022/6/geological_taxonomy#Xerolls">
        <rdfs:subClassOf rdf:resource="http://www.semanticweb.org/ontologies/2022/6/geological_taxonomy#Mollisols"/>
        <rdfs:comment>Xerolls have a xeric Soil Moisture Regime

Resource: https://www.sciencedirect.com/topics/agricultural-and-biological-sciences/mollisol</rdfs:comment>
    </owl:Class>
    


    <!-- http://www.semanticweb.org/ontologies/2022/6/geological_taxonomy#Xerults -->

    <owl:Class rdf:about="http://www.semanticweb.org/ontologies/2022/6/geological_taxonomy#Xerults">
        <rdfs:subClassOf rdf:resource="http://www.semanticweb.org/ontologies/2022/6/geological_taxonomy#Ultisols"/>
        <rdfs:comment>A suborder of the soil order Ultisol, formed in a xeric moisture regime; brownish or reddish soil with a low to moderate organic-carbon content.

Resource: https://encyclopedia2.thefreedictionary.com/Xerult</rdfs:comment>
    </owl:Class>
    


    <!-- http://www.semanticweb.org/ontologies/2022/6/geological_taxonomy#protolith -->

    <owl:Class rdf:about="http://www.semanticweb.org/ontologies/2022/6/geological_taxonomy#protolith">
        <rdfs:subClassOf rdf:resource="http://www.semanticweb.org/ontologies/2022/6/geological_taxonomy#Metamorphic_rocks"/>
        <rdfs:comment>A protolith is the original, unmetamorphosed rock from which a given metamorphic rock is formed.

Resource: https://en.wikipedia.org/wiki/List_of_rock_types</rdfs:comment>
    </owl:Class>
    


    <!-- http://www.semanticweb.org/ontologies/2022/6/geological_taxonomy#ʻAʻā -->

    <owl:Class rdf:about="http://www.semanticweb.org/ontologies/2022/6/geological_taxonomy#ʻAʻā">
        <rdfs:subClassOf rdf:resource="http://www.semanticweb.org/ontologies/2022/6/geological_taxonomy#Basalt"/>
        <rdfs:comment>Basaltic lava with a crumpled appearance

Resource: https://en.wikipedia.org/wiki/%CA%BBA%CA%BB%C4%81</rdfs:comment>
    </owl:Class>
    


    <!-- http://www.semanticweb.org/ontologies/2022/6/geological_taxonomy#D_Double-Prime_(D’’) -->

    <owl:Class rdf:about="http://www.semanticweb.org/ontologies/2022/6/geological_taxonomy#D_Double-Prime_(D’’)">
        <rdfs:subClassOf rdf:resource="http://www.semanticweb.org/ontologies/2022/6/geological_taxonomy#Mantle"/>
        <rdfs:comment>D&quot; is the layer which separates the mantle from the core, a region with anomalous seismic properties.

Resource: https://www.newworldencyclopedia.org/entry/Mantle_(geology)</rdfs:comment>
    </owl:Class>
    


    <!-- http://www.semanticweb.org/ontologies/2022/6/geological_taxonomy#Dolomite_(rock) -->

    <owl:Class rdf:about="http://www.semanticweb.org/ontologies/2022/6/geological_taxonomy#Dolomite_(rock)">
        <rdfs:subClassOf rdf:resource="http://www.semanticweb.org/ontologies/2022/6/geological_taxonomy#Sedimentary_rocks"/>
        <rdfs:comment>Dolomite (also known as dolomite rock, dolostone or dolomitic rock) is a sedimentary carbonate rock that contains a high percentage of the mineral dolomite, CaMg(CO3)2. 

Resource: https://en.wikipedia.org/wiki/Dolomite_(rock)</rdfs:comment>
    </owl:Class>
    


    <!-- http://www.semanticweb.org/ontologies/2022/6/geological_taxonomy#Earth&apos;s_inner_core -->

    <owl:Class rdf:about="http://www.semanticweb.org/ontologies/2022/6/geological_taxonomy#Earth&apos;s_inner_core">
        <rdfs:subClassOf rdf:resource="http://www.semanticweb.org/ontologies/2022/6/geological_taxonomy#Planetary_core"/>
        <rdfs:comment>Earth&apos;s inner core is the innermost geologic layer of planet Earth. It is primarily a solid ball with a radius of about 1,220 km (760 mi). Pressure ranges from about 330 to 360 gigapascals (3,300,000 to 3,600,000 atm)

Resource: https://en.wikipedia.org/wiki/Earth%27s_inner_core</rdfs:comment>
    </owl:Class>
    


    <!-- http://www.semanticweb.org/ontologies/2022/6/geological_taxonomy#Lithosphere–asthenosphere_boundary -->

    <owl:Class rdf:about="http://www.semanticweb.org/ontologies/2022/6/geological_taxonomy#Lithosphere–asthenosphere_boundary">
        <rdfs:subClassOf rdf:resource="http://www.semanticweb.org/ontologies/2022/6/geological_taxonomy#Upper_mantle"/>
        <rdfs:comment>represents a mechanical difference between layers in Earth&apos;s inner structure.

Resource: https://en.wikipedia.org/wiki/Lithosphere%E2%80%93asthenosphere_boundary</rdfs:comment>
    </owl:Class>
    


    <!-- http://www.semanticweb.org/ontologies/2022/6/geological_taxonomy#Nor&apos;easter -->

    <owl:Class rdf:about="http://www.semanticweb.org/ontologies/2022/6/geological_taxonomy#Nor&apos;easter">
        <rdfs:subClassOf rdf:resource="http://www.semanticweb.org/ontologies/2022/6/geological_taxonomy#Extratropical_cyclone"/>
        <rdfs:comment>A synoptic-scale extratropical cyclone in the western North Atlantic Ocean with combination of northeast winds and moisture content of the swirling clouds.

Resource: https://en.wikipedia.org/wiki/Nor%27easter</rdfs:comment>
    </owl:Class>
    


    <!-- http://www.semanticweb.org/ontologies/2022/6/geological_taxonomy#Riverine_(Channel)_Flood -->

    <owl:Class rdf:about="http://www.semanticweb.org/ontologies/2022/6/geological_taxonomy#Riverine_(Channel)_Flood">
        <rdfs:subClassOf rdf:resource="http://www.semanticweb.org/ontologies/2022/6/geological_taxonomy#Flood"/>
        <rdfs:comment>Riverine Flooding is when streams and rivers exceed the capacity of their natural or constructed channels to accommodate water flow and water overflows the banks, spilling out into adjacent low-lying, dry land	

Resource: https://hazards.fema.gov/nri/riverine-flooding</rdfs:comment>
    </owl:Class>
    


    <!-- http://www.semanticweb.org/ontologies/2022/6/geological_taxonomy#Transition_zone_(Earth) -->

    <owl:Class rdf:about="http://www.semanticweb.org/ontologies/2022/6/geological_taxonomy#Transition_zone_(Earth)">
        <rdfs:subClassOf rdf:resource="http://www.semanticweb.org/ontologies/2022/6/geological_taxonomy#Mantle"/>
        <rdfs:comment>The transition zone is part of the Earth&apos;s mantle, and is located between the lower mantle and the upper mantle

Resource: https://en.wikipedia.org/wiki/Transition_zone_(Earth)</rdfs:comment>
    </owl:Class>
    


    <!-- https://en.wikipedia.org/wiki/Atmosphere#Overcast -->

    <owl:Class rdf:about="https://en.wikipedia.org/wiki/Atmosphere#Overcast">
        <rdfs:subClassOf rdf:resource="http://www.semanticweb.org/ontologies/2022/6/geological_taxonomy#Cloudy"/>
        <owl:disjointWith rdf:resource="https://en.wikipedia.org/wiki/Atmosphere#Partially_cloudy"/>
        <rdfs:comment>Overcast weather is when the sky is completely covered by a cloud blanket.

Resource: https://weather.fandom.com/wiki/Types_of_Weather#Overcast</rdfs:comment>
    </owl:Class>
    


    <!-- https://en.wikipedia.org/wiki/Atmosphere#Partially_cloudy -->

    <owl:Class rdf:about="https://en.wikipedia.org/wiki/Atmosphere#Partially_cloudy">
        <rdfs:subClassOf rdf:resource="http://www.semanticweb.org/ontologies/2022/6/geological_taxonomy#Cloudy"/>
        <rdfs:comment>Partially cloudy weather is when some clouds are hovering above the horizon level; however, most of the sky remains clear and there is no precipitation of any kind.

Resource: https://weather.fandom.com/wiki/Types_of_Weather#Partially_cloudy</rdfs:comment>
    </owl:Class>
    


    <!-- 
    ///////////////////////////////////////////////////////////////////////////////////////
    //
    // Individuals
    //
    ///////////////////////////////////////////////////////////////////////////////////////
     -->

    


    <!-- http://www.semanticweb.org/ontologies/2022/6/geological_taxonomy#Actinolite -->

    <owl:NamedIndividual rdf:about="http://www.semanticweb.org/ontologies/2022/6/geological_taxonomy#Actinolite">
        <rdf:type rdf:resource="http://www.semanticweb.org/ontologies/2022/6/geological_taxonomy#Silicates"/>
        <rdfs:comment>Actinolite is an amphibole silicate mineral with the chemical formula Ca2(Mg4.5-2.5Fe2+0.5-2.5)Si8O22(OH)2.

Resource: https://en.wikipedia.org/wiki/Actinolite</rdfs:comment>
    </owl:NamedIndividual>
    


    <!-- http://www.semanticweb.org/ontologies/2022/6/geological_taxonomy#Afghanite -->

    <owl:NamedIndividual rdf:about="http://www.semanticweb.org/ontologies/2022/6/geological_taxonomy#Afghanite">
        <rdf:type rdf:resource="http://www.semanticweb.org/ontologies/2022/6/geological_taxonomy#Silicates"/>
        <rdfs:comment>Afghanite, (Na,K)22Ca10[Si24Al24O96](SO4)6Cl6,[2] is a hydrous sodium, calcium, potassium, sulfate, chloride, carbonate alumino-silicate mineral. Afghanite is a feldspathoid of the cancrinite group and typically occurs with sodalite group minerals.

Resource: https://en.wikipedia.org/wiki/Afghanite</rdfs:comment>
    </owl:NamedIndividual>
    


    <!-- http://www.semanticweb.org/ontologies/2022/6/geological_taxonomy#Alarsite -->

    <owl:NamedIndividual rdf:about="http://www.semanticweb.org/ontologies/2022/6/geological_taxonomy#Alarsite">
        <rdf:type rdf:resource="http://www.semanticweb.org/ontologies/2022/6/geological_taxonomy#Phosphates_Arsenates_Vanadates"/>
        <rdfs:comment>Alarsite (AlAsO4) is an aluminium arsenate mineral with its name derived from its composition: aluminium and arsenate.
Chemical Formula: AlAsO4

Resource: http://webmineral.com/data/Alarsite.shtml#.Yy8RcnZBzIU
https://en.wikipedia.org/wiki/Alarsite</rdfs:comment>
    </owl:NamedIndividual>
    


    <!-- http://www.semanticweb.org/ontologies/2022/6/geological_taxonomy#Albite -->

    <owl:NamedIndividual rdf:about="http://www.semanticweb.org/ontologies/2022/6/geological_taxonomy#Albite">
        <rdf:type rdf:resource="http://www.semanticweb.org/ontologies/2022/6/geological_taxonomy#Silicates"/>
        <rdfs:comment>Albite is a plagioclase feldspar mineral. The pure albite endmember has the formula NaAlSi3O8.

Resource: https://en.wikipedia.org/wiki/Albite</rdfs:comment>
    </owl:NamedIndividual>
    


    <!-- http://www.semanticweb.org/ontologies/2022/6/geological_taxonomy#Alfredstelznerite -->

    <owl:NamedIndividual rdf:about="http://www.semanticweb.org/ontologies/2022/6/geological_taxonomy#Alfredstelznerite">
        <rdf:type rdf:resource="http://www.semanticweb.org/ontologies/2022/6/geological_taxonomy#Borates"/>
        <rdfs:comment>Chemical Formula: Ca4(H2O)4 [B4O4(OH)6]4 {H2O}15

Resource: http://www.webmineral.com/data/Alfredstelznerite.shtml#.Yy8RnnZBzIU</rdfs:comment>
    </owl:NamedIndividual>
    


    <!-- http://www.semanticweb.org/ontologies/2022/6/geological_taxonomy#Algodonite -->

    <owl:NamedIndividual rdf:about="http://www.semanticweb.org/ontologies/2022/6/geological_taxonomy#Algodonite">
        <rdf:type rdf:resource="http://www.semanticweb.org/ontologies/2022/6/geological_taxonomy#Sulfides_and_Sulfosalts"/>
        <rdfs:comment>Algodonite is a copper arsenide mineral. It is a gray white metallic mineral crystallizing in the hexagonal system.
Chemical formula: Cu6As

Resource: https://en.wikipedia.org/wiki/Algodonite</rdfs:comment>
    </owl:NamedIndividual>
    


    <!-- http://www.semanticweb.org/ontologies/2022/6/geological_taxonomy#Almandine -->

    <owl:NamedIndividual rdf:about="http://www.semanticweb.org/ontologies/2022/6/geological_taxonomy#Almandine">
        <rdf:type rdf:resource="http://www.semanticweb.org/ontologies/2022/6/geological_taxonomy#Silicates"/>
        <rdfs:comment>Almandine, also known as almandite, is a species of mineral belonging to the garnet group. The almandine crystal formula is: Fe3Al2(SiO4)3.

Resource: https://en.wikipedia.org/wiki/Almandine</rdfs:comment>
    </owl:NamedIndividual>
    


    <!-- http://www.semanticweb.org/ontologies/2022/6/geological_taxonomy#Amalgam -->

    <owl:NamedIndividual rdf:about="http://www.semanticweb.org/ontologies/2022/6/geological_taxonomy#Amalgam">
        <rdf:type rdf:resource="http://www.semanticweb.org/ontologies/2022/6/geological_taxonomy#Elements"/>
        <rdfs:comment>An amalgam is an alloy of mercury with another metal. It may be a liquid, a soft paste or a solid, depending upon the proportion of mercury.
Chemical Formula: Ag2Hg3

Resource: https://en.wikipedia.org/wiki/Amalgam_(chemistry)
http://webmineral.com/data/Amalgam.shtml#.Yy8SM3ZBzIU</rdfs:comment>
    </owl:NamedIndividual>
    


    <!-- http://www.semanticweb.org/ontologies/2022/6/geological_taxonomy#Amblygonite -->

    <owl:NamedIndividual rdf:about="http://www.semanticweb.org/ontologies/2022/6/geological_taxonomy#Amblygonite">
        <rdf:type rdf:resource="http://www.semanticweb.org/ontologies/2022/6/geological_taxonomy#Phosphates_Arsenates_Vanadates"/>
        <rdfs:comment>Amblygonite, is a fluorophosphate mineral, (Li,Na)AlPO4(F,OH), composed of lithium, sodium, aluminium, phosphate, fluoride and hydroxide.

Resource: https://en.wikipedia.org/wiki/Amblygonite</rdfs:comment>
    </owl:NamedIndividual>
    


    <!-- http://www.semanticweb.org/ontologies/2022/6/geological_taxonomy#Andalusite -->

    <owl:NamedIndividual rdf:about="http://www.semanticweb.org/ontologies/2022/6/geological_taxonomy#Andalusite">
        <rdf:type rdf:resource="http://www.semanticweb.org/ontologies/2022/6/geological_taxonomy#Silicates"/>
        <rdfs:comment>Andalusite is an aluminium nesosilicate mineral with the chemical formula Al2SiO5.

Resource: https://en.wikipedia.org/wiki/Andalusite</rdfs:comment>
    </owl:NamedIndividual>
    


    <!-- http://www.semanticweb.org/ontologies/2022/6/geological_taxonomy#Andradite -->

    <owl:NamedIndividual rdf:about="http://www.semanticweb.org/ontologies/2022/6/geological_taxonomy#Andradite">
        <rdf:type rdf:resource="http://www.semanticweb.org/ontologies/2022/6/geological_taxonomy#Silicates"/>
        <rdfs:comment>Andradite is a mineral species of the garnet group. It is a nesosilicate, with formula Ca3Fe2Si3O12.

Resource: https://en.wikipedia.org/wiki/Andradite</rdfs:comment>
    </owl:NamedIndividual>
    


    <!-- http://www.semanticweb.org/ontologies/2022/6/geological_taxonomy#Anhydrite -->

    <owl:NamedIndividual rdf:about="http://www.semanticweb.org/ontologies/2022/6/geological_taxonomy#Anhydrite">
        <rdf:type rdf:resource="http://www.semanticweb.org/ontologies/2022/6/geological_taxonomy#Sulfates"/>
        <rdfs:comment>Anhydrite, or anhydrous calcium sulfate, is a mineral with the chemical formula CaSO4.

Resource: https://en.wikipedia.org/wiki/Anhydrite</rdfs:comment>
    </owl:NamedIndividual>
    


    <!-- http://www.semanticweb.org/ontologies/2022/6/geological_taxonomy#Anorthite -->

    <owl:NamedIndividual rdf:about="http://www.semanticweb.org/ontologies/2022/6/geological_taxonomy#Anorthite">
        <rdf:type rdf:resource="http://www.semanticweb.org/ontologies/2022/6/geological_taxonomy#Silicates"/>
        <rdfs:comment>Anorthite is the calcium endmember of the plagioclase feldspar mineral series. The chemical formula of pure anorthite is CaAl2Si2O8.

Resource: https://en.wikipedia.org/wiki/Anorthite</rdfs:comment>
    </owl:NamedIndividual>
    


    <!-- http://www.semanticweb.org/ontologies/2022/6/geological_taxonomy#Antigorite -->

    <owl:NamedIndividual rdf:about="http://www.semanticweb.org/ontologies/2022/6/geological_taxonomy#Antigorite">
        <rdf:type rdf:resource="http://www.semanticweb.org/ontologies/2022/6/geological_taxonomy#Silicates"/>
        <rdfs:comment>Antigorite is a lamellated, monoclinic mineral in the phylosilicate serpentine subgroup with the ideal chemical formula of (Mg,Fe2+)3Si2O5(OH)4

Resource: https://en.wikipedia.org/wiki/Antigorite</rdfs:comment>
    </owl:NamedIndividual>
    


    <!-- http://www.semanticweb.org/ontologies/2022/6/geological_taxonomy#Aragonite -->

    <owl:NamedIndividual rdf:about="http://www.semanticweb.org/ontologies/2022/6/geological_taxonomy#Aragonite">
        <rdf:type rdf:resource="http://www.semanticweb.org/ontologies/2022/6/geological_taxonomy#Carbonates"/>
        <rdfs:comment>Aragonite is a carbonate mineral, one of the three most common naturally occurring crystal forms of calcium carbonate, CaCO3

Resource: https://en.wikipedia.org/wiki/Aragonite</rdfs:comment>
    </owl:NamedIndividual>
    


    <!-- http://www.semanticweb.org/ontologies/2022/6/geological_taxonomy#Arcanite -->

    <owl:NamedIndividual rdf:about="http://www.semanticweb.org/ontologies/2022/6/geological_taxonomy#Arcanite">
        <rdf:type rdf:resource="http://www.semanticweb.org/ontologies/2022/6/geological_taxonomy#Sulfates"/>
        <rdfs:comment></rdfs:comment>
        <rdfs:comment>Arcanite is a potassium sulfate mineral with formula: K2SO4.

Resource: https://en.wikipedia.org/wiki/Arcanite</rdfs:comment>
    </owl:NamedIndividual>
    


    <!-- http://www.semanticweb.org/ontologies/2022/6/geological_taxonomy#Atheneite -->

    <owl:NamedIndividual rdf:about="http://www.semanticweb.org/ontologies/2022/6/geological_taxonomy#Atheneite">
        <rdf:type rdf:resource="http://www.semanticweb.org/ontologies/2022/6/geological_taxonomy#Sulfides_and_Sulfosalts"/>
        <rdfs:comment>Atheneite is a rare palladium, mercury arsenide mineral with the chemical formula (Pd,Hg)3 associated with palladium–gold deposits.

Resource: https://en.wikipedia.org/wiki/Atheneite</rdfs:comment>
    </owl:NamedIndividual>
    


    <!-- http://www.semanticweb.org/ontologies/2022/6/geological_taxonomy#Benitoite -->

    <owl:NamedIndividual rdf:about="http://www.semanticweb.org/ontologies/2022/6/geological_taxonomy#Benitoite">
        <rdf:type rdf:resource="http://www.semanticweb.org/ontologies/2022/6/geological_taxonomy#Silicates"/>
        <rdfs:comment>Benitoite is a rare blue barium titanium cyclosilicate.
Chemical Formula: BaTi(Si3O9)

Resource: https://en.wikipedia.org/wiki/Benitoite
https://www.mindat.org/min-624.html</rdfs:comment>
    </owl:NamedIndividual>
    


    <!-- http://www.semanticweb.org/ontologies/2022/6/geological_taxonomy#Berborite -->

    <owl:NamedIndividual rdf:about="http://www.semanticweb.org/ontologies/2022/6/geological_taxonomy#Berborite">
        <rdf:type rdf:resource="http://www.semanticweb.org/ontologies/2022/6/geological_taxonomy#Borates"/>
        <rdfs:comment>Berborite is a beryllium borate mineral with the chemical formula Be2(BO3)(OH,F)·(H2O). It is colorless and leaves a white streak. Its crystals are hexagonal to pyramidal. It is transparent and has vitreous luster.

Resource: https://en.wikipedia.org/wiki/Berborite</rdfs:comment>
    </owl:NamedIndividual>
    


    <!-- http://www.semanticweb.org/ontologies/2022/6/geological_taxonomy#Berlinite -->

    <owl:NamedIndividual rdf:about="http://www.semanticweb.org/ontologies/2022/6/geological_taxonomy#Berlinite">
        <rdf:type rdf:resource="http://www.semanticweb.org/ontologies/2022/6/geological_taxonomy#Phosphates_Arsenates_Vanadates"/>
        <rdfs:comment>Berlinite (aluminium phosphate, chemical formula AlPO4 or Al(PO4))) is a rare high-temperature hydrothermal or metasomatic phosphate mineral.

Resource: https://en.wikipedia.org/wiki/Berlinite</rdfs:comment>
    </owl:NamedIndividual>
    


    <!-- http://www.semanticweb.org/ontologies/2022/6/geological_taxonomy#Beryl -->

    <owl:NamedIndividual rdf:about="http://www.semanticweb.org/ontologies/2022/6/geological_taxonomy#Beryl">
        <rdf:type rdf:resource="http://www.semanticweb.org/ontologies/2022/6/geological_taxonomy#Silicates"/>
        <rdfs:comment>Beryl is a mineral composed of beryllium aluminium silicate with the chemical formula Be3Al2Si6O18.

Resource: https://en.wikipedia.org/wiki/Beryl</rdfs:comment>
    </owl:NamedIndividual>
    


    <!-- http://www.semanticweb.org/ontologies/2022/6/geological_taxonomy#Brazilianite -->

    <owl:NamedIndividual rdf:about="http://www.semanticweb.org/ontologies/2022/6/geological_taxonomy#Brazilianite">
        <rdf:type rdf:resource="http://www.semanticweb.org/ontologies/2022/6/geological_taxonomy#Phosphates_Arsenates_Vanadates"/>
        <rdfs:comment>Brazilianite, whose name derives from its country of origin, Brazil, is a typically yellow-green phosphate mineral, most commonly found in phosphate-rich pegmatites.
Chemical Formula: NaAl3(PO4)2(OH)4

Resource: https://en.wikipedia.org/wiki/Brazilianite
https://www.mindat.org/min-760.html</rdfs:comment>
    </owl:NamedIndividual>
    


    <!-- http://www.semanticweb.org/ontologies/2022/6/geological_taxonomy#Brownmillerite -->

    <owl:NamedIndividual rdf:about="http://www.semanticweb.org/ontologies/2022/6/geological_taxonomy#Brownmillerite">
        <rdf:type rdf:resource="http://www.semanticweb.org/ontologies/2022/6/geological_taxonomy#Oxides"/>
        <rdfs:comment>Brownmillerite is a rare oxide mineral with chemical formula Ca2(Al,Fe)2O5.

Resource: https://en.wikipedia.org/wiki/Brownmillerite</rdfs:comment>
    </owl:NamedIndividual>
    


    <!-- http://www.semanticweb.org/ontologies/2022/6/geological_taxonomy#Cadmium -->

    <owl:NamedIndividual rdf:about="http://www.semanticweb.org/ontologies/2022/6/geological_taxonomy#Cadmium">
        <rdf:type rdf:resource="http://www.semanticweb.org/ontologies/2022/6/geological_taxonomy#Elements"/>
        <rdfs:comment>Cadmium is a chemical element with the symbol Cd and atomic number 48. This soft, silvery-white metal is chemically similar to the two other stable metals in group 12, zinc and mercury.

Resource: https://en.wikipedia.org/wiki/Cadmium</rdfs:comment>
    </owl:NamedIndividual>
    


    <!-- http://www.semanticweb.org/ontologies/2022/6/geological_taxonomy#Calcite -->

    <owl:NamedIndividual rdf:about="http://www.semanticweb.org/ontologies/2022/6/geological_taxonomy#Calcite">
        <rdf:type rdf:resource="http://www.semanticweb.org/ontologies/2022/6/geological_taxonomy#Carbonates"/>
        <rdfs:comment>Calcite, the most common form of natural calcium carbonate (CaCO3), a widely distributed mineral known for the beautiful development and great variety of its crystals.

Resource: https://www.britannica.com/science/calcite</rdfs:comment>
    </owl:NamedIndividual>
    


    <!-- http://www.semanticweb.org/ontologies/2022/6/geological_taxonomy#Caminite -->

    <owl:NamedIndividual rdf:about="http://www.semanticweb.org/ontologies/2022/6/geological_taxonomy#Caminite">
        <rdf:type rdf:resource="http://www.semanticweb.org/ontologies/2022/6/geological_taxonomy#Sulfates"/>
        <rdfs:comment>A tetragonal-ditetragonal dipyramidal mineral containing hydrogen, magnesium, oxygen, and sulfur.
Chemical Formula: Mg7(SO4)5(OH)4•(H2O)

Resource: https://en.wiktionary.org/wiki/caminite
http://webmineral.com/data/Caminite.shtml#.Yy8YXHZBzIU</rdfs:comment>
    </owl:NamedIndividual>
    


    <!-- http://www.semanticweb.org/ontologies/2022/6/geological_taxonomy#Carnallite -->

    <owl:NamedIndividual rdf:about="http://www.semanticweb.org/ontologies/2022/6/geological_taxonomy#Carnallite">
        <rdf:type rdf:resource="http://www.semanticweb.org/ontologies/2022/6/geological_taxonomy#Halides"/>
        <rdfs:comment>Carnallite, a soft, white halide mineral, hydrated potassium and magnesium chloride (KMgCl3·6H2O), that is a source of potassium for fertilizers. 

Resource: https://www.britannica.com/science/carnallite</rdfs:comment>
    </owl:NamedIndividual>
    


    <!-- http://www.semanticweb.org/ontologies/2022/6/geological_taxonomy#Cerussite -->

    <owl:NamedIndividual rdf:about="http://www.semanticweb.org/ontologies/2022/6/geological_taxonomy#Cerussite">
        <rdf:type rdf:resource="http://www.semanticweb.org/ontologies/2022/6/geological_taxonomy#Carbonates"/>
        <rdfs:comment>Cerussite (also known as lead carbonate or white lead ore) is a mineral consisting of lead carbonate (PbCO3), and is an important ore of lead.

Resource: https://en.wikipedia.org/wiki/Cerussite</rdfs:comment>
    </owl:NamedIndividual>
    


    <!-- http://www.semanticweb.org/ontologies/2022/6/geological_taxonomy#Chalcocite -->

    <owl:NamedIndividual rdf:about="http://www.semanticweb.org/ontologies/2022/6/geological_taxonomy#Chalcocite">
        <rdf:type rdf:resource="http://www.semanticweb.org/ontologies/2022/6/geological_taxonomy#Sulfides_and_Sulfosalts"/>
        <rdfs:comment>Chalcocite, copper(I) sulfide (Cu2S), is an important copper ore mineral. It is opaque and dark gray to black, with a metallic luster.

Resource: https://en.wikipedia.org/wiki/Chalcocite</rdfs:comment>
    </owl:NamedIndividual>
    


    <!-- http://www.semanticweb.org/ontologies/2022/6/geological_taxonomy#Charoite -->

    <owl:NamedIndividual rdf:about="http://www.semanticweb.org/ontologies/2022/6/geological_taxonomy#Charoite">
        <rdf:type rdf:resource="http://www.semanticweb.org/ontologies/2022/6/geological_taxonomy#Silicates"/>
        <rdfs:comment>Charoite K(Ca,Na)2Si4O10(OH,F)•H2O is a rare silicate mineral, first described in 1978

Resource: https://en.wikipedia.org/wiki/Charoite</rdfs:comment>
    </owl:NamedIndividual>
    


    <!-- http://www.semanticweb.org/ontologies/2022/6/geological_taxonomy#Chondrodite -->

    <owl:NamedIndividual rdf:about="http://www.semanticweb.org/ontologies/2022/6/geological_taxonomy#Chondrodite">
        <rdf:type rdf:resource="http://www.semanticweb.org/ontologies/2022/6/geological_taxonomy#Silicates"/>
        <rdfs:comment>Chondrodite is a nesosilicate mineral with formula (Mg,Fe)5(SiO4)2(F,OH,O)2.

Resource: https://en.wikipedia.org/wiki/Chondrodite</rdfs:comment>
    </owl:NamedIndividual>
    


    <!-- http://www.semanticweb.org/ontologies/2022/6/geological_taxonomy#Chromium-dravite -->

    <owl:NamedIndividual rdf:about="http://www.semanticweb.org/ontologies/2022/6/geological_taxonomy#Chromium-dravite">
        <rdf:type rdf:resource="http://www.semanticweb.org/ontologies/2022/6/geological_taxonomy#Silicates"/>
        <rdfs:comment>Chemical Formula: NaMg3Cr3+6(Si6O18)(BO3)3(OH)3(OH)

Resource: https://www.mindat.org/min-1031.html</rdfs:comment>
    </owl:NamedIndividual>
    


    <!-- http://www.semanticweb.org/ontologies/2022/6/geological_taxonomy#Chrysoberyl -->

    <owl:NamedIndividual rdf:about="http://www.semanticweb.org/ontologies/2022/6/geological_taxonomy#Chrysoberyl">
        <rdf:type rdf:resource="http://www.semanticweb.org/ontologies/2022/6/geological_taxonomy#Oxides"/>
        <rdfs:comment>The mineral or gemstone chrysoberyl is an aluminate of beryllium with the formula BeAl2O4.

Resource: https://en.wikipedia.org/wiki/Chrysoberyl</rdfs:comment>
    </owl:NamedIndividual>
    


    <!-- http://www.semanticweb.org/ontologies/2022/6/geological_taxonomy#Clinohumite -->

    <owl:NamedIndividual rdf:about="http://www.semanticweb.org/ontologies/2022/6/geological_taxonomy#Clinohumite">
        <rdf:type rdf:resource="http://www.semanticweb.org/ontologies/2022/6/geological_taxonomy#Silicates"/>
        <rdfs:comment>Clinohumite is an uncommon member of the humite group, a magnesium silicate according to the chemical formula (Mg, Fe)9(SiO4)4(F,OH)2. 

Resource: https://en.wikipedia.org/wiki/Clinohumite</rdfs:comment>
    </owl:NamedIndividual>
    


    <!-- http://www.semanticweb.org/ontologies/2022/6/geological_taxonomy#Clinozoisite -->

    <owl:NamedIndividual rdf:about="http://www.semanticweb.org/ontologies/2022/6/geological_taxonomy#Clinozoisite">
        <rdf:type rdf:resource="http://www.semanticweb.org/ontologies/2022/6/geological_taxonomy#Silicates"/>
        <rdfs:comment>Clinozoisite is a complex calcium aluminium sorosilicate mineral with formula: Ca2Al3(Si2O7)(SiO4)O(OH).

Resource: https://en.wikipedia.org/wiki/Clinozoisite</rdfs:comment>
    </owl:NamedIndividual>
    


    <!-- http://www.semanticweb.org/ontologies/2022/6/geological_taxonomy#Coccinite -->

    <owl:NamedIndividual rdf:about="http://www.semanticweb.org/ontologies/2022/6/geological_taxonomy#Coccinite">
        <rdf:type rdf:resource="http://www.semanticweb.org/ontologies/2022/6/geological_taxonomy#Halides"/>
        <rdfs:comment>Coccinite is a rare mercury iodide mineral with chemical formula of HgI2, mercury(II) iodide.[5][6] It was first discovered in Casas Viejas, Mexico

Resource: https://en.wikipedia.org/wiki/Coccinite</rdfs:comment>
    </owl:NamedIndividual>
    


    <!-- http://www.semanticweb.org/ontologies/2022/6/geological_taxonomy#Copper -->

    <owl:NamedIndividual rdf:about="http://www.semanticweb.org/ontologies/2022/6/geological_taxonomy#Copper">
        <rdf:type rdf:resource="http://www.semanticweb.org/ontologies/2022/6/geological_taxonomy#Elements"/>
        <rdfs:comment>Copper is a chemical element with the symbol Cu (from Latin: cuprum) and atomic number 29. It is a soft, malleable, and ductile metal with very high thermal and electrical conductivity.

Resource: https://en.wikipedia.org/wiki/Copper</rdfs:comment>
    </owl:NamedIndividual>
    


    <!-- http://www.semanticweb.org/ontologies/2022/6/geological_taxonomy#Cordierite -->

    <owl:NamedIndividual rdf:about="http://www.semanticweb.org/ontologies/2022/6/geological_taxonomy#Cordierite">
        <rdf:type rdf:resource="http://www.semanticweb.org/ontologies/2022/6/geological_taxonomy#Silicates"/>
        <rdfs:comment>Cordierite (mineralogy) is a magnesium iron aluminium cyclosilicate.
Chemical Formula: (Mg,Fe)2Al4Si5O18

Resource: https://en.wikipedia.org/wiki/Cordierite</rdfs:comment>
    </owl:NamedIndividual>
    


    <!-- http://www.semanticweb.org/ontologies/2022/6/geological_taxonomy#Corundum -->

    <owl:NamedIndividual rdf:about="http://www.semanticweb.org/ontologies/2022/6/geological_taxonomy#Corundum">
        <rdf:type rdf:resource="http://www.semanticweb.org/ontologies/2022/6/geological_taxonomy#Oxides"/>
        <rdfs:comment>Corundum is a crystalline form of aluminium oxide (Al2O3) typically containing traces of iron, titanium, vanadium and chromium.

Resource: https://en.wikipedia.org/wiki/Corundum</rdfs:comment>
    </owl:NamedIndividual>
    


    <!-- http://www.semanticweb.org/ontologies/2022/6/geological_taxonomy#Crednerite -->

    <owl:NamedIndividual rdf:about="http://www.semanticweb.org/ontologies/2022/6/geological_taxonomy#Crednerite">
        <rdf:type rdf:resource="http://www.semanticweb.org/ontologies/2022/6/geological_taxonomy#Oxides"/>
        <rdfs:comment>A dark grey mineral that is a mixed oxide of copper and manganese.
Chemical Formula: CuMnO2

Resource: https://en.wiktionary.org/wiki/crednerite
http://webmineral.com/data/Crednerite.shtml#.Yy8Z4HZBzIU</rdfs:comment>
    </owl:NamedIndividual>
    


    <!-- http://www.semanticweb.org/ontologies/2022/6/geological_taxonomy#Cuprite -->

    <owl:NamedIndividual rdf:about="http://www.semanticweb.org/ontologies/2022/6/geological_taxonomy#Cuprite">
        <rdf:type rdf:resource="http://www.semanticweb.org/ontologies/2022/6/geological_taxonomy#Oxides"/>
        <rdfs:comment>Cuprite is an oxide mineral composed of copper(I) oxide Cu2O, and is a minor ore of copper.

Resource: https://en.wikipedia.org/wiki/Cuprite</rdfs:comment>
    </owl:NamedIndividual>
    


    <!-- http://www.semanticweb.org/ontologies/2022/6/geological_taxonomy#Danburite -->

    <owl:NamedIndividual rdf:about="http://www.semanticweb.org/ontologies/2022/6/geological_taxonomy#Danburite">
        <rdf:type rdf:resource="http://www.semanticweb.org/ontologies/2022/6/geological_taxonomy#Silicates"/>
        <rdfs:comment>Danburite is a calcium boron silicate mineral with a chemical formula of CaB2(SiO4)2.

Resource: https://en.wikipedia.org/wiki/Danburite</rdfs:comment>
    </owl:NamedIndividual>
    


    <!-- http://www.semanticweb.org/ontologies/2022/6/geological_taxonomy#Dashkovaite -->

    <owl:NamedIndividual rdf:about="http://www.semanticweb.org/ontologies/2022/6/geological_taxonomy#Dashkovaite">
        <rdf:type rdf:resource="http://www.semanticweb.org/ontologies/2022/6/geological_taxonomy#Organic_compounds"/>
        <rdfs:comment>A monoclinic-prismatic white mineral containing carbon, hydrogen, magnesium, and oxygen.
Chemical Formula: Mg(HCOO)2•2(H2O)

Resource: https://en.wiktionary.org/wiki/dashkovaite
http://webmineral.com/data/Dashkovaite.shtml#.Yy8aZnZBzIU</rdfs:comment>
    </owl:NamedIndividual>
    


    <!-- http://www.semanticweb.org/ontologies/2022/6/geological_taxonomy#Datolite -->

    <owl:NamedIndividual rdf:about="http://www.semanticweb.org/ontologies/2022/6/geological_taxonomy#Datolite">
        <rdf:type rdf:resource="http://www.semanticweb.org/ontologies/2022/6/geological_taxonomy#Silicates"/>
        <rdfs:comment>Datolite is a calcium boron hydroxide nesosilicate, CaBSiO4(OH).

Resource: https://en.wikipedia.org/wiki/Datolite</rdfs:comment>
    </owl:NamedIndividual>
    


    <!-- http://www.semanticweb.org/ontologies/2022/6/geological_taxonomy#Diamond -->

    <owl:NamedIndividual rdf:about="http://www.semanticweb.org/ontologies/2022/6/geological_taxonomy#Diamond">
        <rdf:type rdf:resource="http://www.semanticweb.org/ontologies/2022/6/geological_taxonomy#Elements"/>
        <rdfs:comment>Diamond is a solid form of the element carbon with its atoms arranged in a crystal structure called diamond cubic.
Chemical Formula: C

Resource: https://en.wikipedia.org/wiki/Diamond
https://www.mindat.org/min-1282.html</rdfs:comment>
    </owl:NamedIndividual>
    


    <!-- http://www.semanticweb.org/ontologies/2022/6/geological_taxonomy#Diaspore -->

    <owl:NamedIndividual rdf:about="http://www.semanticweb.org/ontologies/2022/6/geological_taxonomy#Diaspore">
        <rdf:type rdf:resource="http://www.semanticweb.org/ontologies/2022/6/geological_taxonomy#Oxides"/>
        <rdfs:comment>Diaspore, also known as diasporite, empholite, kayserite, or tanatarite, is an aluminium oxide hydroxide mineral, α-AlO(OH)

Resource: https://en.wikipedia.org/wiki/Diaspore</rdfs:comment>
    </owl:NamedIndividual>
    


    <!-- http://www.semanticweb.org/ontologies/2022/6/geological_taxonomy#Diopside -->

    <owl:NamedIndividual rdf:about="http://www.semanticweb.org/ontologies/2022/6/geological_taxonomy#Diopside">
        <rdf:type rdf:resource="http://www.semanticweb.org/ontologies/2022/6/geological_taxonomy#Silicates"/>
        <rdfs:comment>Diopside is a monoclinic pyroxene mineral with composition MgCaSi2O6.

Resource: https://en.wikipedia.org/wiki/Diopside</rdfs:comment>
    </owl:NamedIndividual>
    


    <!-- http://www.semanticweb.org/ontologies/2022/6/geological_taxonomy#Djurleite -->

    <owl:NamedIndividual rdf:about="http://www.semanticweb.org/ontologies/2022/6/geological_taxonomy#Djurleite">
        <rdf:type rdf:resource="http://www.semanticweb.org/ontologies/2022/6/geological_taxonomy#Sulfides_and_Sulfosalts"/>
        <rdfs:comment>Djurleite is a copper sulfide mineral of secondary origin with formula Cu31S16 that crystallizes with monoclinic-prismatic symmetry.

Resource: https://en.wikipedia.org/wiki/Djurleite</rdfs:comment>
    </owl:NamedIndividual>
    


    <!-- http://www.semanticweb.org/ontologies/2022/6/geological_taxonomy#Dolomite -->

    <owl:NamedIndividual rdf:about="http://www.semanticweb.org/ontologies/2022/6/geological_taxonomy#Dolomite">
        <rdf:type rdf:resource="http://www.semanticweb.org/ontologies/2022/6/geological_taxonomy#Carbonates"/>
    </owl:NamedIndividual>
    


    <!-- http://www.semanticweb.org/ontologies/2022/6/geological_taxonomy#Domeykite -->

    <owl:NamedIndividual rdf:about="http://www.semanticweb.org/ontologies/2022/6/geological_taxonomy#Domeykite">
        <rdf:type rdf:resource="http://www.semanticweb.org/ontologies/2022/6/geological_taxonomy#Sulfides_and_Sulfosalts"/>
        <rdfs:comment>Domeykite is a copper arsenide mineral, Cu3As. It crystallizes in the isometric system, although crystals are very rare. 

Resource: https://en.wikipedia.org/wiki/Domeykite</rdfs:comment>
    </owl:NamedIndividual>
    


    <!-- http://www.semanticweb.org/ontologies/2022/6/geological_taxonomy#Dravite -->

    <owl:NamedIndividual rdf:about="http://www.semanticweb.org/ontologies/2022/6/geological_taxonomy#Dravite">
        <rdf:type rdf:resource="http://www.semanticweb.org/ontologies/2022/6/geological_taxonomy#Silicates"/>
        <rdfs:comment>Dravite is best known as the &quot;Brown Tourmaline&quot;. It is a relatively common form of Tourmaline, and often forms in crude uninteresting formation.
Chemical Formula: NaMg3Al6(BO3)3Si6O18(OH)3F

Resource: https://www.minerals.net/mineral/dravite.aspx</rdfs:comment>
    </owl:NamedIndividual>
    


    <!-- http://www.semanticweb.org/ontologies/2022/6/geological_taxonomy#Earlandite -->

    <owl:NamedIndividual rdf:about="http://www.semanticweb.org/ontologies/2022/6/geological_taxonomy#Earlandite">
        <rdf:type rdf:resource="http://www.semanticweb.org/ontologies/2022/6/geological_taxonomy#Organic_compounds"/>
        <rdfs:comment>Earlandite, [Ca3(C6H5O7)2(H2O)2]·2H2O, is the mineral form of calcium citrate tetrahydrate. It was first reported in 1936.

Resource: https://en.wikipedia.org/wiki/Earlandite</rdfs:comment>
    </owl:NamedIndividual>
    


    <!-- http://www.semanticweb.org/ontologies/2022/6/geological_taxonomy#Eitelite -->

    <owl:NamedIndividual rdf:about="http://www.semanticweb.org/ontologies/2022/6/geological_taxonomy#Eitelite">
        <rdf:type rdf:resource="http://www.semanticweb.org/ontologies/2022/6/geological_taxonomy#Carbonates"/>
        <rdfs:comment>Chemical Formula: Na2Mg(CO3)2

Resource: http://webmineral.com/data/Eitelite.shtml#.Yy8bFHZBzIU</rdfs:comment>
    </owl:NamedIndividual>
    


    <!-- http://www.semanticweb.org/ontologies/2022/6/geological_taxonomy#Elbaite -->

    <owl:NamedIndividual rdf:about="http://www.semanticweb.org/ontologies/2022/6/geological_taxonomy#Elbaite">
        <rdf:type rdf:resource="http://www.semanticweb.org/ontologies/2022/6/geological_taxonomy#Silicates"/>
        <rdfs:comment>Elbaite, a sodium, lithium, aluminium boro-silicate, with the chemical composition Na(Li1.5Al1.5)Al6Si6O18(BO3)3(OH)4,[4] is a mineral species belonging to the six-member ring cyclosilicate tourmaline group.

Resource: https://en.wikipedia.org/wiki/Elbaite</rdfs:comment>
    </owl:NamedIndividual>
    


    <!-- http://www.semanticweb.org/ontologies/2022/6/geological_taxonomy#Enstatite -->

    <owl:NamedIndividual rdf:about="http://www.semanticweb.org/ontologies/2022/6/geological_taxonomy#Enstatite">
        <rdf:type rdf:resource="http://www.semanticweb.org/ontologies/2022/6/geological_taxonomy#Silicates"/>
        <rdfs:comment>Enstatite is a mineral; the magnesium endmember of the pyroxene silicate mineral series enstatite (MgSiO3) – ferrosilite (FeSiO3).

Resource: https://en.wikipedia.org/wiki/Enstatite</rdfs:comment>
    </owl:NamedIndividual>
    


    <!-- http://www.semanticweb.org/ontologies/2022/6/geological_taxonomy#Epidote -->

    <owl:NamedIndividual rdf:about="http://www.semanticweb.org/ontologies/2022/6/geological_taxonomy#Epidote">
        <rdf:type rdf:resource="http://www.semanticweb.org/ontologies/2022/6/geological_taxonomy#Silicates"/>
        <rdfs:comment>Epidote is a calcium aluminium iron sorosilicate mineral.
Chemical Formula: {Ca2}{Al2Fe3+}(Si2O7)(SiO4)O(OH)

Resource: https://en.wikipedia.org/wiki/Epidote
https://www.mindat.org/min-1389.html</rdfs:comment>
    </owl:NamedIndividual>
    


    <!-- http://www.semanticweb.org/ontologies/2022/6/geological_taxonomy#Euclase -->

    <owl:NamedIndividual rdf:about="http://www.semanticweb.org/ontologies/2022/6/geological_taxonomy#Euclase">
        <rdf:type rdf:resource="http://www.semanticweb.org/ontologies/2022/6/geological_taxonomy#Silicates"/>
        <rdfs:comment>Euclase is a beryllium aluminium hydroxide silicate mineral (BeAlSiO4(OH)). It crystallizes in the monoclinic crystal system and is typically massive to fibrous as well as in slender prismatic crystals.

Resource: https://en.wikipedia.org/wiki/Euclase</rdfs:comment>
    </owl:NamedIndividual>
    


    <!-- http://www.semanticweb.org/ontologies/2022/6/geological_taxonomy#Eucryptite -->

    <owl:NamedIndividual rdf:about="http://www.semanticweb.org/ontologies/2022/6/geological_taxonomy#Eucryptite">
        <rdf:type rdf:resource="http://www.semanticweb.org/ontologies/2022/6/geological_taxonomy#Silicates"/>
        <rdfs:comment>Eucryptite is a lithium bearing aluminium silicate mineral with formula LiAlSiO4. It crystallizes in the trigonal - rhombohedral crystal system.

Resource: https://en.wikipedia.org/wiki/Eucryptite</rdfs:comment>
    </owl:NamedIndividual>
    


    <!-- http://www.semanticweb.org/ontologies/2022/6/geological_taxonomy#Farringtonite -->

    <owl:NamedIndividual rdf:about="http://www.semanticweb.org/ontologies/2022/6/geological_taxonomy#Farringtonite">
        <rdf:type rdf:resource="http://www.semanticweb.org/ontologies/2022/6/geological_taxonomy#Phosphates_Arsenates_Vanadates"/>
        <rdfs:comment>Chemical Formula: Mg3(PO4)2

Resource: https://www.webmineral.com/data/Farringtonite.shtml</rdfs:comment>
    </owl:NamedIndividual>
    


    <!-- http://www.semanticweb.org/ontologies/2022/6/geological_taxonomy#Ferrisicklerite -->

    <owl:NamedIndividual rdf:about="http://www.semanticweb.org/ontologies/2022/6/geological_taxonomy#Ferrisicklerite">
        <rdf:type rdf:resource="http://www.semanticweb.org/ontologies/2022/6/geological_taxonomy#Phosphates_Arsenates_Vanadates"/>
        <rdfs:comment>An orthorhombic-dipyramidal mineral containing iron, lithium, manganese, oxygen, and phosphorus.
Chemical Formula: Li(Fe+++,Mn++)PO4

Resource: https://en.wiktionary.org/wiki/ferrisicklerite
http://www.webmineral.com/data/Ferrisicklerite.shtml#.Yy8btXZBzIU</rdfs:comment>
    </owl:NamedIndividual>
    


    <!-- http://www.semanticweb.org/ontologies/2022/6/geological_taxonomy#Ferro-actinolite -->

    <owl:NamedIndividual rdf:about="http://www.semanticweb.org/ontologies/2022/6/geological_taxonomy#Ferro-actinolite">
        <rdf:type rdf:resource="http://www.semanticweb.org/ontologies/2022/6/geological_taxonomy#Silicates"/>
        <rdfs:comment>Ferro-actinolite is the ferrous iron-rich endmember of the actinolite-tremolite continuous solid solution series of the double chain calcareous amphibole group of inosilicate minerals.
Chemical Formula: Ca2Fe2+5(Si8O22)OH2

Resource: https://en.wikipedia.org/wiki/Ferro-actinolite
https://www.mindat.org/min-1505.html</rdfs:comment>
    </owl:NamedIndividual>
    


    <!-- http://www.semanticweb.org/ontologies/2022/6/geological_taxonomy#Fluorapatite -->

    <owl:NamedIndividual rdf:about="http://www.semanticweb.org/ontologies/2022/6/geological_taxonomy#Fluorapatite">
        <rdf:type rdf:resource="http://www.semanticweb.org/ontologies/2022/6/geological_taxonomy#Phosphates_Arsenates_Vanadates"/>
        <rdfs:comment>Fluorapatite, is a phosphate mineral with the formula Ca5(PO4)3F (calcium fluorophosphate). Fluorapatite is a hard crystalline solid.

Resource: https://en.wikipedia.org/wiki/Fluorapatite</rdfs:comment>
    </owl:NamedIndividual>
    


    <!-- http://www.semanticweb.org/ontologies/2022/6/geological_taxonomy#Fluorite -->

    <owl:NamedIndividual rdf:about="http://www.semanticweb.org/ontologies/2022/6/geological_taxonomy#Fluorite">
        <rdf:type rdf:resource="http://www.semanticweb.org/ontologies/2022/6/geological_taxonomy#Halides"/>
        <rdfs:comment>Fluorite (also called fluorspar) is the mineral form of calcium fluoride, CaF2.

Resource: https://en.wikipedia.org/wiki/Fluorite</rdfs:comment>
    </owl:NamedIndividual>
    


    <!-- http://www.semanticweb.org/ontologies/2022/6/geological_taxonomy#Formicaite -->

    <owl:NamedIndividual rdf:about="http://www.semanticweb.org/ontologies/2022/6/geological_taxonomy#Formicaite">
        <rdf:type rdf:resource="http://www.semanticweb.org/ontologies/2022/6/geological_taxonomy#Organic_compounds"/>
        <rdfs:comment>A tetragonal-trapezohedral mineral containing calcium, carbon, hydrogen, and oxygen.
Chemical Formula: Ca(HCOO)2

Resource: https://en.wiktionary.org/wiki/formicaite
http://www.webmineral.com/data/Formicaite.shtml#.Yy8b5HZBzIU</rdfs:comment>
    </owl:NamedIndividual>
    


    <!-- http://www.semanticweb.org/ontologies/2022/6/geological_taxonomy#Forsterite -->

    <owl:NamedIndividual rdf:about="http://www.semanticweb.org/ontologies/2022/6/geological_taxonomy#Forsterite">
        <rdf:type rdf:resource="http://www.semanticweb.org/ontologies/2022/6/geological_taxonomy#Silicates"/>
        <rdfs:comment>Chemical Formula: Mg2SiO4

Resource: https://www.mindat.org/min-1584.html</rdfs:comment>
    </owl:NamedIndividual>
    


    <!-- http://www.semanticweb.org/ontologies/2022/6/geological_taxonomy#Friedelite -->

    <owl:NamedIndividual rdf:about="http://www.semanticweb.org/ontologies/2022/6/geological_taxonomy#Friedelite">
        <rdf:type rdf:resource="http://www.semanticweb.org/ontologies/2022/6/geological_taxonomy#Silicates"/>
        <rdfs:comment>Friedelite is a mineral in the pyrosmalite group.
Chemical Formula: Mn2+8Si6O15(OH,Cl)10

Resource: https://en.wikipedia.org/wiki/Friedelite
https://www.mindat.org/min-1609.html</rdfs:comment>
    </owl:NamedIndividual>
    


    <!-- http://www.semanticweb.org/ontologies/2022/6/geological_taxonomy#Gaspeite -->

    <owl:NamedIndividual rdf:about="http://www.semanticweb.org/ontologies/2022/6/geological_taxonomy#Gaspeite">
        <rdf:type rdf:resource="http://www.semanticweb.org/ontologies/2022/6/geological_taxonomy#Carbonates"/>
        <rdfs:comment>Gaspéite, a very rare nickel carbonate mineral, with the formula (Ni,Fe,Mg)CO3, is named for the place it was first described, in the Gaspé Peninsula, Québec, Canada.

Resource: https://en.wikipedia.org/wiki/Gasp%C3%A9ite</rdfs:comment>
    </owl:NamedIndividual>
    


    <!-- http://www.semanticweb.org/ontologies/2022/6/geological_taxonomy#Grandidierite -->

    <owl:NamedIndividual rdf:about="http://www.semanticweb.org/ontologies/2022/6/geological_taxonomy#Grandidierite">
        <rdf:type rdf:resource="http://www.semanticweb.org/ontologies/2022/6/geological_taxonomy#Silicates"/>
        <rdfs:comment>Grandidierite is a rare mineral that was first discovered in 1902 in southern Madagascar.
Chemical Formula: (Mg,Fe2+)(Al,Fe3+)3(SiO4)(BO3)O2

Resource: https://en.wikipedia.org/wiki/Grandidierite
https://www.mindat.org/min-1737.html</rdfs:comment>
    </owl:NamedIndividual>
    


    <!-- http://www.semanticweb.org/ontologies/2022/6/geological_taxonomy#Gregoryite -->

    <owl:NamedIndividual rdf:about="http://www.semanticweb.org/ontologies/2022/6/geological_taxonomy#Gregoryite">
        <rdf:type rdf:resource="http://www.semanticweb.org/ontologies/2022/6/geological_taxonomy#Carbonates"/>
        <rdfs:comment>Gregoryite is an anhydrous carbonate mineral that is rich in potassium and sodium[5] with the chemical formula (Na2,K2,Ca)CO3.[

Resource: https://en.wikipedia.org/wiki/Gregoryite</rdfs:comment>
    </owl:NamedIndividual>
    


    <!-- http://www.semanticweb.org/ontologies/2022/6/geological_taxonomy#Grossular -->

    <owl:NamedIndividual rdf:about="http://www.semanticweb.org/ontologies/2022/6/geological_taxonomy#Grossular">
        <rdf:type rdf:resource="http://www.semanticweb.org/ontologies/2022/6/geological_taxonomy#Silicates"/>
        <rdfs:comment>Grossular is a calcium-aluminium species of the garnet group of minerals. It has the chemical formula of Ca3Al2(SiO4)3

Resource: https://en.wikipedia.org/wiki/Grossular</rdfs:comment>
    </owl:NamedIndividual>
    


    <!-- http://www.semanticweb.org/ontologies/2022/6/geological_taxonomy#Hambergite -->

    <owl:NamedIndividual rdf:about="http://www.semanticweb.org/ontologies/2022/6/geological_taxonomy#Hambergite">
        <rdf:type rdf:resource="http://www.semanticweb.org/ontologies/2022/6/geological_taxonomy#Borates"/>
        <rdfs:comment>Hambergite (Be2BO3OH) is a beryllium borate mineral named after Swedish explorer and mineralogist Axel Hamberg (1863–1933). The mineral occurs as white or colorless orthorhombic crystals.

Resource: https://en.wikipedia.org/wiki/Hambergite</rdfs:comment>
    </owl:NamedIndividual>
    


    <!-- http://www.semanticweb.org/ontologies/2022/6/geological_taxonomy#Hauckite -->

    <owl:NamedIndividual rdf:about="http://www.semanticweb.org/ontologies/2022/6/geological_taxonomy#Hauckite">
        <rdf:type rdf:resource="http://www.semanticweb.org/ontologies/2022/6/geological_taxonomy#Sulfates"/>
        <rdfs:comment>Chemical Formula: Fe3+3(Mg,Mn2+)24Zn18(SO4)4(CO3)2(OH)81

Resource: https://www.mindat.org/min-1830.html</rdfs:comment>
    </owl:NamedIndividual>
    


    <!-- http://www.semanticweb.org/ontologies/2022/6/geological_taxonomy#Haüyne -->

    <owl:NamedIndividual rdf:about="http://www.semanticweb.org/ontologies/2022/6/geological_taxonomy#Haüyne">
        <rdf:type rdf:resource="http://www.semanticweb.org/ontologies/2022/6/geological_taxonomy#Silicates"/>
        <rdfs:comment>Hauyne or haüyne, also called hauynite or haüynite, is a tectosilicate sulfate mineral with endmember formula Na3Ca(Si3Al3)O12(SO4).

Resource: https://en.wikipedia.org/wiki/Hauyne</rdfs:comment>
    </owl:NamedIndividual>
    


    <!-- http://www.semanticweb.org/ontologies/2022/6/geological_taxonomy#Hematite -->

    <owl:NamedIndividual rdf:about="http://www.semanticweb.org/ontologies/2022/6/geological_taxonomy#Hematite">
        <rdf:type rdf:resource="http://www.semanticweb.org/ontologies/2022/6/geological_taxonomy#Oxides"/>
        <rdfs:comment>Hematite, also spelled as haematite, is a common iron oxide compound with the formula, Fe2O3.

Resource: https://en.wikipedia.org/wiki/Hematite</rdfs:comment>
    </owl:NamedIndividual>
    


    <!-- http://www.semanticweb.org/ontologies/2022/6/geological_taxonomy#Hemimorphite -->

    <owl:NamedIndividual rdf:about="http://www.semanticweb.org/ontologies/2022/6/geological_taxonomy#Hemimorphite">
        <rdf:type rdf:resource="http://www.semanticweb.org/ontologies/2022/6/geological_taxonomy#Silicates"/>
        <rdfs:comment>Hemimorphite is the chemical compound Zn4(Si2O7)(OH)2·H2O, a component of mineral calamine.

Resource: https://en.wikipedia.org/wiki/Hemimorphite</rdfs:comment>
    </owl:NamedIndividual>
    


    <!-- http://www.semanticweb.org/ontologies/2022/6/geological_taxonomy#Herderite -->

    <owl:NamedIndividual rdf:about="http://www.semanticweb.org/ontologies/2022/6/geological_taxonomy#Herderite">
        <rdf:type rdf:resource="http://www.semanticweb.org/ontologies/2022/6/geological_taxonomy#Phosphates_Arsenates_Vanadates"/>
        <rdfs:comment>Herderite is a phosphate mineral belonging to the apatite, phosphate group, with formula CaBe(PO4)(F,OH).

Resource: https://en.wikipedia.org/wiki/Herderite</rdfs:comment>
    </owl:NamedIndividual>
    


    <!-- http://www.semanticweb.org/ontologies/2022/6/geological_taxonomy#Howardevansite -->

    <owl:NamedIndividual rdf:about="http://www.semanticweb.org/ontologies/2022/6/geological_taxonomy#Howardevansite">
        <rdf:type rdf:resource="http://www.semanticweb.org/ontologies/2022/6/geological_taxonomy#Phosphates_Arsenates_Vanadates"/>
        <rdfs:comment>A triclinic-pinacoidal black mineral containing copper, iron, oxygen, sodium, and vanadium.
Chemical Formula: NaCuFe2(VO4)3

Resource: https://en.wiktionary.org/wiki/howardevansite
https://www.mindat.org/min-1934.html</rdfs:comment>
    </owl:NamedIndividual>
    


    <!-- http://www.semanticweb.org/ontologies/2022/6/geological_taxonomy#Howlite -->

    <owl:NamedIndividual rdf:about="http://www.semanticweb.org/ontologies/2022/6/geological_taxonomy#Howlite">
        <rdf:type rdf:resource="http://www.semanticweb.org/ontologies/2022/6/geological_taxonomy#Borates"/>
        <rdfs:comment>Howlite, a calcium borosilicate hydroxide (Ca2B5SiO9(OH)5), is a borate mineral found in evaporite deposits.

Resource: https://en.wikipedia.org/wiki/Howlite</rdfs:comment>
    </owl:NamedIndividual>
    


    <!-- http://www.semanticweb.org/ontologies/2022/6/geological_taxonomy#Humboldtine -->

    <owl:NamedIndividual rdf:about="http://www.semanticweb.org/ontologies/2022/6/geological_taxonomy#Humboldtine">
        <rdf:type rdf:resource="http://www.semanticweb.org/ontologies/2022/6/geological_taxonomy#Organic_compounds"/>
        <rdfs:comment>Humboldtine is a rarely occurring mineral from the mineral class of &quot;organic compounds&quot; with the chemical composition FeC2O4•2H2O and is therefore a water-containing iron(II) oxalate or the iron salt of oxalic acid.

Resource: https://en.wikipedia.org/wiki/Humboldtine</rdfs:comment>
    </owl:NamedIndividual>
    


    <!-- http://www.semanticweb.org/ontologies/2022/6/geological_taxonomy#Hydrohalite -->

    <owl:NamedIndividual rdf:about="http://www.semanticweb.org/ontologies/2022/6/geological_taxonomy#Hydrohalite">
        <rdf:type rdf:resource="http://www.semanticweb.org/ontologies/2022/6/geological_taxonomy#Halides"/>
        <rdfs:comment>Hydrohalite is a mineral that occurs in saturated halite brines at cold temperatures (below 0.1 °C). It was first described in 1847 in Dürrnberg, Austria. It exists in cold weather.

Resource: https://en.wikipedia.org/wiki/Hydrohalite</rdfs:comment>
    </owl:NamedIndividual>
    


    <!-- http://www.semanticweb.org/ontologies/2022/6/geological_taxonomy#IMA2008-029 -->

    <owl:NamedIndividual rdf:about="http://www.semanticweb.org/ontologies/2022/6/geological_taxonomy#IMA2008-029">
        <rdf:type rdf:resource="http://www.semanticweb.org/ontologies/2022/6/geological_taxonomy#Sulfates"/>
        <rdfs:comment>Chemical Formula: (NH4)3Fe(SO4)3

Resource: https://www.mindat.org/min-39464.html</rdfs:comment>
    </owl:NamedIndividual>
    


    <!-- http://www.semanticweb.org/ontologies/2022/6/geological_taxonomy#IMA2008-054 -->

    <owl:NamedIndividual rdf:about="http://www.semanticweb.org/ontologies/2022/6/geological_taxonomy#IMA2008-054">
        <rdf:type rdf:resource="http://www.semanticweb.org/ontologies/2022/6/geological_taxonomy#Phosphates_Arsenates_Vanadates"/>
        <rdfs:comment>Chemical Formula: NaCaMn2(PO4)[PO3(OH)]2

Resource: http://webmineral.com/data/IMA2008-054.shtml#.Yy8d1XZBzIU</rdfs:comment>
    </owl:NamedIndividual>
    


    <!-- http://www.semanticweb.org/ontologies/2022/6/geological_taxonomy#Ice -->

    <owl:NamedIndividual rdf:about="http://www.semanticweb.org/ontologies/2022/6/geological_taxonomy#Ice">
        <rdf:type rdf:resource="http://www.semanticweb.org/ontologies/2022/6/geological_taxonomy#Oxides"/>
        <rdfs:comment>Ice is water frozen into a solid state, typically forming at or below temperatures of 0 degrees Celsius or 32 °F 
Chemical Formula: H2O

Resource: https://en.wikipedia.org/wiki/Ice
https://www.mindat.org/min-2001.html</rdfs:comment>
    </owl:NamedIndividual>
    


    <!-- http://www.semanticweb.org/ontologies/2022/6/geological_taxonomy#Indium -->

    <owl:NamedIndividual rdf:about="http://www.semanticweb.org/ontologies/2022/6/geological_taxonomy#Indium">
        <rdf:type rdf:resource="http://www.semanticweb.org/ontologies/2022/6/geological_taxonomy#Elements"/>
        <rdfs:comment>Indium is a chemical element with the symbol In and atomic number 49. Indium is the softest metal that is not an alkali metal.

Resource: https://en.wikipedia.org/wiki/Indium</rdfs:comment>
    </owl:NamedIndividual>
    


    <!-- http://www.semanticweb.org/ontologies/2022/6/geological_taxonomy#Ivanyukite-Cu -->

    <owl:NamedIndividual rdf:about="http://www.semanticweb.org/ontologies/2022/6/geological_taxonomy#Ivanyukite-Cu">
        <rdf:type rdf:resource="http://www.semanticweb.org/ontologies/2022/6/geological_taxonomy#Silicates"/>
        <rdfs:comment>Chemical Formula: C uTi4(SiO4)3(OH)2O2 · 7H2O

Resource: https://www.mindat.org/min-32620.html</rdfs:comment>
    </owl:NamedIndividual>
    


    <!-- http://www.semanticweb.org/ontologies/2022/6/geological_taxonomy#Ivanyukite-Na -->

    <owl:NamedIndividual rdf:about="http://www.semanticweb.org/ontologies/2022/6/geological_taxonomy#Ivanyukite-Na">
        <rdf:type rdf:resource="http://www.semanticweb.org/ontologies/2022/6/geological_taxonomy#Silicates"/>
        <rdfs:comment>Chemical Formula: Na2Ti4(SiO4)3(OH)2O2 · 6H2O

Resource: https://www.mindat.org/min-32618.html</rdfs:comment>
    </owl:NamedIndividual>
    


    <!-- http://www.semanticweb.org/ontologies/2022/6/geological_taxonomy#Jadeite -->

    <owl:NamedIndividual rdf:about="http://www.semanticweb.org/ontologies/2022/6/geological_taxonomy#Jadeite">
        <rdf:type rdf:resource="http://www.semanticweb.org/ontologies/2022/6/geological_taxonomy#Silicates"/>
        <rdfs:comment>Jadeite is a pyroxene mineral with composition NaAlSi2O6. It is hard (Mohs hardness of about 6.5 to 7.0), very tough, and dense, with a specific gravity of about 3.4.

Resource: https://en.wikipedia.org/wiki/Jadeite</rdfs:comment>
    </owl:NamedIndividual>
    


    <!-- http://www.semanticweb.org/ontologies/2022/6/geological_taxonomy#Jeremejevite -->

    <owl:NamedIndividual rdf:about="http://www.semanticweb.org/ontologies/2022/6/geological_taxonomy#Jeremejevite">
        <rdf:type rdf:resource="http://www.semanticweb.org/ontologies/2022/6/geological_taxonomy#Borates"/>
        <rdfs:comment>Jeremejevite is an aluminium borate mineral with variable fluoride and hydroxide ions. Its chemical formula is Al6B5O15(F,OH)3.

Resource: https://en.wikipedia.org/wiki/Jeremejevite</rdfs:comment>
    </owl:NamedIndividual>
    


    <!-- http://www.semanticweb.org/ontologies/2022/6/geological_taxonomy#Johachidolite -->

    <owl:NamedIndividual rdf:about="http://www.semanticweb.org/ontologies/2022/6/geological_taxonomy#Johachidolite">
        <rdf:type rdf:resource="http://www.semanticweb.org/ontologies/2022/6/geological_taxonomy#Borates"/>
        <rdfs:comment>An orthorhombic-dipyramidal mineral containing aluminum, boron, calcium, and oxygen.
Chemical Formula: CaAlB3O7

Resource: https://en.wiktionary.org/wiki/johachidolite
https://www.mindat.org/min-2101.html</rdfs:comment>
    </owl:NamedIndividual>
    


    <!-- http://www.semanticweb.org/ontologies/2022/6/geological_taxonomy#Julienite -->

    <owl:NamedIndividual rdf:about="http://www.semanticweb.org/ontologies/2022/6/geological_taxonomy#Julienite">
        <rdf:type rdf:resource="http://www.semanticweb.org/ontologies/2022/6/geological_taxonomy#Organic_compounds"/>
        <rdfs:comment>Chemical Formula: Na2[Co(SCN)4] · 8H2O

Resource: https://www.mindat.org/min-2121.html</rdfs:comment>
    </owl:NamedIndividual>
    


    <!-- http://www.semanticweb.org/ontologies/2022/6/geological_taxonomy#Kafehydrocyanite -->

    <owl:NamedIndividual rdf:about="http://www.semanticweb.org/ontologies/2022/6/geological_taxonomy#Kafehydrocyanite">
        <rdf:type rdf:resource="http://www.semanticweb.org/ontologies/2022/6/geological_taxonomy#Organic_compounds"/>
        <rdfs:comment>Chemical Formula: K4[Fe(CN)6] · H2O

Resource: https://www.mindat.org/min-2130.html</rdfs:comment>
    </owl:NamedIndividual>
    


    <!-- http://www.semanticweb.org/ontologies/2022/6/geological_taxonomy#Kornerupine -->

    <owl:NamedIndividual rdf:about="http://www.semanticweb.org/ontologies/2022/6/geological_taxonomy#Kornerupine">
        <rdf:type rdf:resource="http://www.semanticweb.org/ontologies/2022/6/geological_taxonomy#Silicates"/>
        <rdfs:comment>Kornerupine (also called Prismatine) is a rare boro-silicate mineral with the chemical formula (Mg,Fe2+)4(Al,Fe3+)6(SiO4,BO4)5(O,OH)2. It crystallizes in the orthorhombic - dipyramidal crystal system as brown, green, yellow to colorless slender tourmaline like prisms or in massive fibrous forms. 

Resource: https://en.wikipedia.org/wiki/Kornerupine</rdfs:comment>
    </owl:NamedIndividual>
    


    <!-- http://www.semanticweb.org/ontologies/2022/6/geological_taxonomy#Kyanite -->

    <owl:NamedIndividual rdf:about="http://www.semanticweb.org/ontologies/2022/6/geological_taxonomy#Kyanite">
        <rdf:type rdf:resource="http://www.semanticweb.org/ontologies/2022/6/geological_taxonomy#Silicates"/>
        <rdfs:comment>Kyanite, also spelled cyanite, also called disthene, silicate mineral that is formed during the regional metamorphism of clay-rich sediments.
Chemical Formula: Al2(SiO4)

Resource: https://www.britannica.com/science/kyanite
https://www.mindat.org/min-2303.html</rdfs:comment>
    </owl:NamedIndividual>
    


    <!-- http://www.semanticweb.org/ontologies/2022/6/geological_taxonomy#Larsenite -->

    <owl:NamedIndividual rdf:about="http://www.semanticweb.org/ontologies/2022/6/geological_taxonomy#Larsenite">
        <rdf:type rdf:resource="http://www.semanticweb.org/ontologies/2022/6/geological_taxonomy#Silicates"/>
        <rdfs:comment>A nesosilicate mineral.
Chemical Formula: PbZnSiO4

Resource: https://www.wikidata.org/wiki/Q3827220
https://www.mindat.org/min-2335.html</rdfs:comment>
    </owl:NamedIndividual>
    


    <!-- http://www.semanticweb.org/ontologies/2022/6/geological_taxonomy#Lazulite -->

    <owl:NamedIndividual rdf:about="http://www.semanticweb.org/ontologies/2022/6/geological_taxonomy#Lazulite">
        <rdf:type rdf:resource="http://www.semanticweb.org/ontologies/2022/6/geological_taxonomy#Phosphates_Arsenates_Vanadates"/>
        <rdfs:comment>Lazulite ((Mg,Fe2+)Al2(PO4)2(OH)2)[3] is a blue, phosphate mineral containing magnesium, iron, and aluminium phosphate.

Resource: https://en.wikipedia.org/wiki/Lazulite</rdfs:comment>
    </owl:NamedIndividual>
    


    <!-- http://www.semanticweb.org/ontologies/2022/6/geological_taxonomy#Lead -->

    <owl:NamedIndividual rdf:about="http://www.semanticweb.org/ontologies/2022/6/geological_taxonomy#Lead">
        <rdf:type rdf:resource="http://www.semanticweb.org/ontologies/2022/6/geological_taxonomy#Elements"/>
        <rdfs:comment>Lead is a soft, malleable, ductile and dense metallic element.
Chemical Formula: Pb

Resource: https://www.nrcan.gc.ca/our-natural-resources/minerals-mining/minerals-metals-facts/lead-facts/20518
https://www.mindat.org/min-2358.html</rdfs:comment>
    </owl:NamedIndividual>
    


    <!-- http://www.semanticweb.org/ontologies/2022/6/geological_taxonomy#Leucite -->

    <owl:NamedIndividual rdf:about="http://www.semanticweb.org/ontologies/2022/6/geological_taxonomy#Leucite">
        <rdf:type rdf:resource="http://www.semanticweb.org/ontologies/2022/6/geological_taxonomy#Silicates"/>
        <rdfs:comment>Leucite is a rock-forming mineral of the feldspathoid group, silica-undersaturated and composed of potassium and aluminium tectosilicate KAlSi2O6.

Resource: https://en.wikipedia.org/wiki/Leucite</rdfs:comment>
    </owl:NamedIndividual>
    


    <!-- http://www.semanticweb.org/ontologies/2022/6/geological_taxonomy#Lindbergite -->

    <owl:NamedIndividual rdf:about="http://www.semanticweb.org/ontologies/2022/6/geological_taxonomy#Lindbergite">
        <rdf:type rdf:resource="http://www.semanticweb.org/ontologies/2022/6/geological_taxonomy#Organic_compounds"/>
        <rdfs:comment>A monoclinic-prismatic mineral containing aluminum, carbon, hydrogen, manganese, oxygen, and sodium.
Chemical Formula: Mn2+(C2O4) · 2H2O

Resource: https://en.wiktionary.org/wiki/lindbergite
https://www.mindat.org/min-26578.html</rdfs:comment>
    </owl:NamedIndividual>
    


    <!-- http://www.semanticweb.org/ontologies/2022/6/geological_taxonomy#Lizardite -->

    <owl:NamedIndividual rdf:about="http://www.semanticweb.org/ontologies/2022/6/geological_taxonomy#Lizardite">
        <rdf:type rdf:resource="http://www.semanticweb.org/ontologies/2022/6/geological_taxonomy#Silicates"/>
        <rdfs:comment>Lizardite is a mineral from the serpentine group with formula Mg3(Si2O5)(OH)4, and the most common type of mineral in the group. It is also a member of the kaolinite-serpentine group.

Resource: https://en.wikipedia.org/wiki/Lizardite</rdfs:comment>
    </owl:NamedIndividual>
    


    <!-- http://www.semanticweb.org/ontologies/2022/6/geological_taxonomy#Magnesite -->

    <owl:NamedIndividual rdf:about="http://www.semanticweb.org/ontologies/2022/6/geological_taxonomy#Magnesite">
        <rdf:type rdf:resource="http://www.semanticweb.org/ontologies/2022/6/geological_taxonomy#Carbonates"/>
        <rdfs:comment>Magnesite is a mineral with the chemical formula MgCO
3 (magnesium carbonate). Iron, manganese, cobalt, and nickel may occur as admixtures, but only in small amounts.

Resource: https://en.wikipedia.org/wiki/Magnesite</rdfs:comment>
    </owl:NamedIndividual>
    


    <!-- http://www.semanticweb.org/ontologies/2022/6/geological_taxonomy#Malachite -->

    <owl:NamedIndividual rdf:about="http://www.semanticweb.org/ontologies/2022/6/geological_taxonomy#Malachite">
        <rdf:type rdf:resource="http://www.semanticweb.org/ontologies/2022/6/geological_taxonomy#Carbonates"/>
        <rdfs:comment>Malachite is a copper carbonate hydroxide mineral, with the formula Cu2CO3(OH)2. This opaque, green-banded mineral crystallizes in the monoclinic crystal system, and most often forms botryoidal, fibrous, or stalagmitic masses, in fractures and deep, underground spaces, where the water table and hydrothermal fluids provide the means for chemical precipitation. Individual crystals are rare, but occur as slender to acicular prisms.

Resource: https://en.wikipedia.org/wiki/Malachite</rdfs:comment>
    </owl:NamedIndividual>
    


    <!-- http://www.semanticweb.org/ontologies/2022/6/geological_taxonomy#Manganostibite -->

    <owl:NamedIndividual rdf:about="http://www.semanticweb.org/ontologies/2022/6/geological_taxonomy#Manganostibite">
        <rdf:type rdf:resource="http://www.semanticweb.org/ontologies/2022/6/geological_taxonomy#Oxides"/>
        <rdfs:comment>Chemical Formula: (Mn,Fe)7SbAsO12

Resource: https://www.mindat.org/min-2528.html</rdfs:comment>
    </owl:NamedIndividual>
    


    <!-- http://www.semanticweb.org/ontologies/2022/6/geological_taxonomy#Marialite -->

    <owl:NamedIndividual rdf:about="http://www.semanticweb.org/ontologies/2022/6/geological_taxonomy#Marialite">
        <rdf:type rdf:resource="http://www.semanticweb.org/ontologies/2022/6/geological_taxonomy#Silicates"/>
        <rdfs:comment>Marialite is a silicate mineral with a chemical formula of Na4Al3Si9O24Cl

Resource: https://en.wikipedia.org/wiki/Marialite</rdfs:comment>
    </owl:NamedIndividual>
    


    <!-- http://www.semanticweb.org/ontologies/2022/6/geological_taxonomy#Mascagnite -->

    <owl:NamedIndividual rdf:about="http://www.semanticweb.org/ontologies/2022/6/geological_taxonomy#Mascagnite">
        <rdf:type rdf:resource="http://www.semanticweb.org/ontologies/2022/6/geological_taxonomy#Sulfates"/>
        <rdfs:comment>Mascagnite is a rare ammonium sulfate mineral (NH4)2SO4.

Resource: https://en.wikipedia.org/wiki/Mascagnite</rdfs:comment>
    </owl:NamedIndividual>
    


    <!-- http://www.semanticweb.org/ontologies/2022/6/geological_taxonomy#Maucherite -->

    <owl:NamedIndividual rdf:about="http://www.semanticweb.org/ontologies/2022/6/geological_taxonomy#Maucherite">
        <rdf:type rdf:resource="http://www.semanticweb.org/ontologies/2022/6/geological_taxonomy#Sulfides_and_Sulfosalts"/>
        <rdfs:comment>Maucherite is a grey to reddish silver white nickel arsenide mineral. It crystallizes in the tetragonal crystal system. 
Chemical Formula: Ni11As8

Resource: https://en.wikipedia.org/wiki/Maucherite
https://www.mindat.org/min-2599.html</rdfs:comment>
    </owl:NamedIndividual>
    


    <!-- http://www.semanticweb.org/ontologies/2022/6/geological_taxonomy#Mellite -->

    <owl:NamedIndividual rdf:about="http://www.semanticweb.org/ontologies/2022/6/geological_taxonomy#Mellite">
        <rdf:type rdf:resource="http://www.semanticweb.org/ontologies/2022/6/geological_taxonomy#Organic_compounds"/>
        <rdfs:comment>Mellite, also called honeystone, is an unusual mineral being also an organic chemical. It is chemically identified as an aluminium salt of mellitic acid, and specifically as aluminium benzene hexacarboxylate hydrate, with the chemical formula Al2C6(COO)6·16H2O.

Resource: https://en.wikipedia.org/wiki/Mellite</rdfs:comment>
    </owl:NamedIndividual>
    


    <!-- http://www.semanticweb.org/ontologies/2022/6/geological_taxonomy#Mercury -->

    <owl:NamedIndividual rdf:about="http://www.semanticweb.org/ontologies/2022/6/geological_taxonomy#Mercury">
        <rdf:type rdf:resource="http://www.semanticweb.org/ontologies/2022/6/geological_taxonomy#Elements"/>
        <rdfs:comment>Mercury is a chemical element with the symbol Hg and atomic number 80. It is also known as quicksilver.

Resource: https://en.wikipedia.org/wiki/Mercury_(element)</rdfs:comment>
    </owl:NamedIndividual>
    


    <!-- http://www.semanticweb.org/ontologies/2022/6/geological_taxonomy#Microcline -->

    <owl:NamedIndividual rdf:about="http://www.semanticweb.org/ontologies/2022/6/geological_taxonomy#Microcline">
        <rdf:type rdf:resource="http://www.semanticweb.org/ontologies/2022/6/geological_taxonomy#Silicates"/>
        <rdfs:comment>Microcline (KAlSi3O8) is an important igneous rock-forming tectosilicate mineral. It is a potassium-rich alkali feldspar.

Resource: https://en.wikipedia.org/wiki/Microcline</rdfs:comment>
    </owl:NamedIndividual>
    


    <!-- http://www.semanticweb.org/ontologies/2022/6/geological_taxonomy#Mikasaite -->

    <owl:NamedIndividual rdf:about="http://www.semanticweb.org/ontologies/2022/6/geological_taxonomy#Mikasaite">
        <rdf:type rdf:resource="http://www.semanticweb.org/ontologies/2022/6/geological_taxonomy#Sulfates"/>
        <rdfs:comment>A trigonal-rhombohedral mineral containing iron, oxygen, and sulfur.
Chemical Formula: Fe2(SO4)3

Resource: https://en.wiktionary.org/wiki/mikasaite
https://www.mindat.org/min-2709.html</rdfs:comment>
    </owl:NamedIndividual>
    


    <!-- http://www.semanticweb.org/ontologies/2022/6/geological_taxonomy#Millosevichite -->

    <owl:NamedIndividual rdf:about="http://www.semanticweb.org/ontologies/2022/6/geological_taxonomy#Millosevichite">
        <rdf:type rdf:resource="http://www.semanticweb.org/ontologies/2022/6/geological_taxonomy#Sulfates"/>
        <rdfs:comment>Millosevichite is a rare sulfate mineral with the chemical formula Al2(SO4)3.

Resource: https://en.wikipedia.org/wiki/Millosevichite</rdfs:comment>
    </owl:NamedIndividual>
    


    <!-- http://www.semanticweb.org/ontologies/2022/6/geological_taxonomy#Molysite -->

    <owl:NamedIndividual rdf:about="http://www.semanticweb.org/ontologies/2022/6/geological_taxonomy#Molysite">
        <rdf:type rdf:resource="http://www.semanticweb.org/ontologies/2022/6/geological_taxonomy#Halides"/>
        <rdfs:comment>A trigonal-rhombohedral mineral containing chlorine and iron.
Chemical Formula: FeCl3

Resource: https://en.wiktionary.org/wiki/molysite
https://www.mindat.org/min-2749.html</rdfs:comment>
    </owl:NamedIndividual>
    


    <!-- http://www.semanticweb.org/ontologies/2022/6/geological_taxonomy#Montebrasite -->

    <owl:NamedIndividual rdf:about="http://www.semanticweb.org/ontologies/2022/6/geological_taxonomy#Montebrasite">
        <rdf:type rdf:resource="http://www.semanticweb.org/ontologies/2022/6/geological_taxonomy#Phosphates_Arsenates_Vanadates"/>
        <rdfs:comment>Chemical Formula: LiAl(PO4)(OH)

Resource: https://www.mindat.org/min-2763.html</rdfs:comment>
    </owl:NamedIndividual>
    


    <!-- http://www.semanticweb.org/ontologies/2022/6/geological_taxonomy#Nahpoite -->

    <owl:NamedIndividual rdf:about="http://www.semanticweb.org/ontologies/2022/6/geological_taxonomy#Nahpoite">
        <rdf:type rdf:resource="http://www.semanticweb.org/ontologies/2022/6/geological_taxonomy#Phosphates_Arsenates_Vanadates"/>
        <rdfs:comment>A monoclinic white mineral containing hydrogen, oxygen, phosphorus, and sodium.
Chemical Formula: Na2(PO3OH)

Resource: https://en.wiktionary.org/wiki/nahpoite
https://www.mindat.org/min-2832.html</rdfs:comment>
    </owl:NamedIndividual>
    


    <!-- http://www.semanticweb.org/ontologies/2022/6/geological_taxonomy#Nantokite -->

    <owl:NamedIndividual rdf:about="http://www.semanticweb.org/ontologies/2022/6/geological_taxonomy#Nantokite">
        <rdf:type rdf:resource="http://www.semanticweb.org/ontologies/2022/6/geological_taxonomy#Halides"/>
        <rdfs:comment>An isometric-hextetrahedral mineral containing chlorine and copper.
Chemical Formula: CuCl

Resource: https://en.wiktionary.org/wiki/nantokite
https://www.mindat.org/min-2840.html</rdfs:comment>
    </owl:NamedIndividual>
    


    <!-- http://www.semanticweb.org/ontologies/2022/6/geological_taxonomy#Natrolite -->

    <owl:NamedIndividual rdf:about="http://www.semanticweb.org/ontologies/2022/6/geological_taxonomy#Natrolite">
        <rdf:type rdf:resource="http://www.semanticweb.org/ontologies/2022/6/geological_taxonomy#Silicates"/>
        <rdfs:comment>Natrolite is a tectosilicate mineral species belonging to the zeolite group. It is a hydrated sodium and aluminium silicate with the formula Na2Al2Si3O10 · 2H2O.

Resource: https://en.wikipedia.org/wiki/Natrolite</rdfs:comment>
    </owl:NamedIndividual>
    


    <!-- http://www.semanticweb.org/ontologies/2022/6/geological_taxonomy#Nordenskioldine -->

    <owl:NamedIndividual rdf:about="http://www.semanticweb.org/ontologies/2022/6/geological_taxonomy#Nordenskioldine">
        <rdf:type rdf:resource="http://www.semanticweb.org/ontologies/2022/6/geological_taxonomy#Borates"/>
        <rdfs:comment>Nordenskioldine is a fairly rare tin-borate and is found in less than 15 localities worldwide. It typically occurs in alkaline pegmatites, (Arø Island, Norway); in a metasomatized marble (Arandis, Namibia); and in skarns deposits (Xianghualing mine, China &amp; this occurence, the MW claim). 
Formula: CaSn4+[BO3]2

Resource: https://www.dakotamatrix.com/products/14984/nordenskioldine
https://www.mindat.org/min-2926.html</rdfs:comment>
    </owl:NamedIndividual>
    


    <!-- http://www.semanticweb.org/ontologies/2022/6/geological_taxonomy#Nyerereite -->

    <owl:NamedIndividual rdf:about="http://www.semanticweb.org/ontologies/2022/6/geological_taxonomy#Nyerereite">
        <rdf:type rdf:resource="http://www.semanticweb.org/ontologies/2022/6/geological_taxonomy#Carbonates"/>
        <rdfs:comment>Nyerereite is a very rare sodium calcium carbonate mineral with formula Na2Ca(CO3)2. It forms colorless, platey pseudohexagonal orthorhombic crystals that are typically twinned.

Resource: https://en.wikipedia.org/wiki/Nyerereite</rdfs:comment>
    </owl:NamedIndividual>
    


    <!-- http://www.semanticweb.org/ontologies/2022/6/geological_taxonomy#Opal -->

    <owl:NamedIndividual rdf:about="http://www.semanticweb.org/ontologies/2022/6/geological_taxonomy#Opal">
        <rdf:type rdf:resource="http://www.semanticweb.org/ontologies/2022/6/geological_taxonomy#Oxides"/>
        <rdfs:comment>The opal is a fairly white rock mineral.
Chemical Formula: SiO2 · nH2O

Resource: https://simple.wikipedia.org/wiki/Opal
https://www.mindat.org/min-3004.html</rdfs:comment>
    </owl:NamedIndividual>
    


    <!-- http://www.semanticweb.org/ontologies/2022/6/geological_taxonomy#Orcelite -->

    <owl:NamedIndividual rdf:about="http://www.semanticweb.org/ontologies/2022/6/geological_taxonomy#Orcelite">
        <rdf:type rdf:resource="http://www.semanticweb.org/ontologies/2022/6/geological_taxonomy#Sulfides_and_Sulfosalts"/>
        <rdfs:comment>A hexagonal-dihexagonal pyramidal orange white mineral containing arsenic and nickel.
Formula:Ni5-xAs2, x ~ 0.25

Resource: https://en.wiktionary.org/wiki/orcelite
https://www.mindat.org/min-3012.html</rdfs:comment>
    </owl:NamedIndividual>
    


    <!-- http://www.semanticweb.org/ontologies/2022/6/geological_taxonomy#Orthoclase -->

    <owl:NamedIndividual rdf:about="http://www.semanticweb.org/ontologies/2022/6/geological_taxonomy#Orthoclase">
        <rdf:type rdf:resource="http://www.semanticweb.org/ontologies/2022/6/geological_taxonomy#Silicates"/>
        <rdfs:comment>Orthoclase, or orthoclase feldspar (endmember formula KAlSi3O8), is an important tectosilicate mineral which forms igneous rock.

Resource: https://en.wikipedia.org/wiki/Orthoclase</rdfs:comment>
    </owl:NamedIndividual>
    


    <!-- http://www.semanticweb.org/ontologies/2022/6/geological_taxonomy#Panichiite -->

    <owl:NamedIndividual rdf:about="http://www.semanticweb.org/ontologies/2022/6/geological_taxonomy#Panichiite">
        <rdf:type rdf:resource="http://www.semanticweb.org/ontologies/2022/6/geological_taxonomy#Halides"/>
        <rdfs:comment>Chemical Formula:(NH4)2SnCl6

Resource: https://www.mindat.org/min-35969.html</rdfs:comment>
    </owl:NamedIndividual>
    


    <!-- http://www.semanticweb.org/ontologies/2022/6/geological_taxonomy#Pargasite -->

    <owl:NamedIndividual rdf:about="http://www.semanticweb.org/ontologies/2022/6/geological_taxonomy#Pargasite">
        <rdf:type rdf:resource="http://www.semanticweb.org/ontologies/2022/6/geological_taxonomy#Silicates"/>
        <rdfs:comment>Pargasite is a complex inosilicate mineral of the amphibole group with formula NaCa2(Mg4Al)(Si6Al2)O22(OH)2.

Resource: https://en.wikipedia.org/wiki/Pargasite</rdfs:comment>
    </owl:NamedIndividual>
    


    <!-- http://www.semanticweb.org/ontologies/2022/6/geological_taxonomy#Pectolite -->

    <owl:NamedIndividual rdf:about="http://www.semanticweb.org/ontologies/2022/6/geological_taxonomy#Pectolite">
        <rdf:type rdf:resource="http://www.semanticweb.org/ontologies/2022/6/geological_taxonomy#Silicates"/>
        <rdfs:comment>Pectolite is a white to gray mineral, NaCa2Si3O8(OH), sodium calcium hydroxide inosilicate. It crystallizes in the triclinic system typically occurring in radiated or fibrous crystalline masses.

Resource: https://en.wikipedia.org/wiki/Pectolite</rdfs:comment>
    </owl:NamedIndividual>
    


    <!-- http://www.semanticweb.org/ontologies/2022/6/geological_taxonomy#Petalite -->

    <owl:NamedIndividual rdf:about="http://www.semanticweb.org/ontologies/2022/6/geological_taxonomy#Petalite">
        <rdf:type rdf:resource="http://www.semanticweb.org/ontologies/2022/6/geological_taxonomy#Silicates"/>
        <rdfs:comment>Petalite, also known as castorite, is a lithium aluminium phyllosilicate mineral LiAlSi4O10, crystallizing in the monoclinic system.

Resource: https://en.wikipedia.org/wiki/Petalite</rdfs:comment>
    </owl:NamedIndividual>
    


    <!-- http://www.semanticweb.org/ontologies/2022/6/geological_taxonomy#Phenakite -->

    <owl:NamedIndividual rdf:about="http://www.semanticweb.org/ontologies/2022/6/geological_taxonomy#Phenakite">
        <rdf:type rdf:resource="http://www.semanticweb.org/ontologies/2022/6/geological_taxonomy#Silicates"/>
        <rdfs:comment>Phenakite or phenacite is a fairly rare nesosilicate mineral consisting of beryllium orthosilicate, Be2SiO4. Occasionally used as a gemstone.

Resource: https://en.wikipedia.org/wiki/Phenakite</rdfs:comment>
    </owl:NamedIndividual>
    


    <!-- http://www.semanticweb.org/ontologies/2022/6/geological_taxonomy#Phosphosiderite -->

    <owl:NamedIndividual rdf:about="http://www.semanticweb.org/ontologies/2022/6/geological_taxonomy#Phosphosiderite">
        <rdf:type rdf:resource="http://www.semanticweb.org/ontologies/2022/6/geological_taxonomy#Phosphates_Arsenates_Vanadates"/>
        <rdfs:comment>Phosphosiderite is a rare mineral named for its main components, phosphate and iron.
Chemical Formula: FePO4 · 2H2O

Resource: https://en.wikipedia.org/wiki/Phosphosiderite
https://www.mindat.org/min-3187.html</rdfs:comment>
    </owl:NamedIndividual>
    


    <!-- http://www.semanticweb.org/ontologies/2022/6/geological_taxonomy#Pollucite -->

    <owl:NamedIndividual rdf:about="http://www.semanticweb.org/ontologies/2022/6/geological_taxonomy#Pollucite">
        <rdf:type rdf:resource="http://www.semanticweb.org/ontologies/2022/6/geological_taxonomy#Silicates"/>
        <rdfs:comment>Pollucite is a zeolite mineral with the formula (Cs,Na)2Al2Si4O12·2H2O with iron, calcium, rubidium and potassium as common substituting elements.

Resource: https://en.wikipedia.org/wiki/Pollucite</rdfs:comment>
    </owl:NamedIndividual>
    


    <!-- http://www.semanticweb.org/ontologies/2022/6/geological_taxonomy#Prehnite -->

    <owl:NamedIndividual rdf:about="http://www.semanticweb.org/ontologies/2022/6/geological_taxonomy#Prehnite">
        <rdf:type rdf:resource="http://www.semanticweb.org/ontologies/2022/6/geological_taxonomy#Silicates"/>
        <rdfs:comment>Prehnite is an inosilicate of calcium and aluminium with the formula: Ca2Al(AlSi3O10)(OH)2.

Resource: https://en.wikipedia.org/wiki/Prehnite</rdfs:comment>
    </owl:NamedIndividual>
    


    <!-- http://www.semanticweb.org/ontologies/2022/6/geological_taxonomy#Pyrope -->

    <owl:NamedIndividual rdf:about="http://www.semanticweb.org/ontologies/2022/6/geological_taxonomy#Pyrope">
        <rdf:type rdf:resource="http://www.semanticweb.org/ontologies/2022/6/geological_taxonomy#Silicates"/>
        <rdfs:comment>The mineral pyrope is a member of the garnet group. Pyrope is the only member of the garnet family to always display red colouration in natural samples
Chemical Formula: Mg3Al2(SiO4)3

Resource: https://en.wikipedia.org/wiki/Pyrope
https://www.mindat.org/min-3321.html</rdfs:comment>
    </owl:NamedIndividual>
    


    <!-- http://www.semanticweb.org/ontologies/2022/6/geological_taxonomy#Quartz -->

    <owl:NamedIndividual rdf:about="http://www.semanticweb.org/ontologies/2022/6/geological_taxonomy#Quartz">
        <rdf:type rdf:resource="http://www.semanticweb.org/ontologies/2022/6/geological_taxonomy#Oxides"/>
        <rdfs:comment>Quartz is a hard, crystalline mineral composed of silica (silicon dioxide). 
Chemical Formula: SiO2

Resource: https://en.wikipedia.org/wiki/Quartz</rdfs:comment>
    </owl:NamedIndividual>
    


    <!-- http://www.semanticweb.org/ontologies/2022/6/geological_taxonomy#Rhodochrosite -->

    <owl:NamedIndividual rdf:about="http://www.semanticweb.org/ontologies/2022/6/geological_taxonomy#Rhodochrosite">
        <rdf:type rdf:resource="http://www.semanticweb.org/ontologies/2022/6/geological_taxonomy#Carbonates"/>
        <rdfs:comment>Rhodochrosite is a manganese carbonate mineral with chemical composition MnCO3. 

Resource: https://en.wikipedia.org/wiki/Rhodochrosite</rdfs:comment>
    </owl:NamedIndividual>
    


    <!-- http://www.semanticweb.org/ontologies/2022/6/geological_taxonomy#Rhodonite -->

    <owl:NamedIndividual rdf:about="http://www.semanticweb.org/ontologies/2022/6/geological_taxonomy#Rhodonite">
        <rdf:type rdf:resource="http://www.semanticweb.org/ontologies/2022/6/geological_taxonomy#Silicates"/>
        <rdfs:comment>Rhodonite, silicate mineral that occurs as rounded crystals, masses, or grains in various manganese ores, often with rhodochrosite.
Chemical Formula: CaMn3Mn[Si5O15]

Resource: https://www.britannica.com/science/rhodonite
https://www.mindat.org/min-3407.html</rdfs:comment>
    </owl:NamedIndividual>
    


    <!-- http://www.semanticweb.org/ontologies/2022/6/geological_taxonomy#Rutile -->

    <owl:NamedIndividual rdf:about="http://www.semanticweb.org/ontologies/2022/6/geological_taxonomy#Rutile">
        <rdf:type rdf:resource="http://www.semanticweb.org/ontologies/2022/6/geological_taxonomy#Oxides"/>
        <rdfs:comment>Rutile is an oxide mineral composed of titanium dioxide (TiO2).

Resource: https://en.wikipedia.org/wiki/Rutile</rdfs:comment>
    </owl:NamedIndividual>
    


    <!-- http://www.semanticweb.org/ontologies/2022/6/geological_taxonomy#Sanidine -->

    <owl:NamedIndividual rdf:about="http://www.semanticweb.org/ontologies/2022/6/geological_taxonomy#Sanidine">
        <rdf:type rdf:resource="http://www.semanticweb.org/ontologies/2022/6/geological_taxonomy#Silicates"/>
        <rdfs:comment>Sanidine is the high temperature form of potassium feldspar with a general formula K(AlSi3O8).[2] Sanidine is found most typically in felsic volcanic rocks such as obsidian, rhyolite and trachyte. 

Resource: https://en.wikipedia.org/wiki/Sanidine</rdfs:comment>
    </owl:NamedIndividual>
    


    <!-- http://www.semanticweb.org/ontologies/2022/6/geological_taxonomy#Sapphirine -->

    <owl:NamedIndividual rdf:about="http://www.semanticweb.org/ontologies/2022/6/geological_taxonomy#Sapphirine">
        <rdf:type rdf:resource="http://www.semanticweb.org/ontologies/2022/6/geological_taxonomy#Silicates"/>
        <rdfs:comment>Sapphirine is a rare mineral, a silicate of magnesium and aluminium with the chemical formula (Mg,Al)8(Al,Si)6O20

Resource: https://en.wikipedia.org/wiki/Sapphirine</rdfs:comment>
    </owl:NamedIndividual>
    


    <!-- http://www.semanticweb.org/ontologies/2022/6/geological_taxonomy#Sassolite -->

    <owl:NamedIndividual rdf:about="http://www.semanticweb.org/ontologies/2022/6/geological_taxonomy#Sassolite">
        <rdf:type rdf:resource="http://www.semanticweb.org/ontologies/2022/6/geological_taxonomy#Borates"/>
        <rdfs:comment>Sassolite is a borate mineral, specifically the mineral form of boric acid. It is usually white to gray, and colourless in transmitted light.
Chemical Formula: H3BO3

Resource: https://en.wikipedia.org/wiki/Sassolite
https://www.mindat.org/min-3540.html</rdfs:comment>
    </owl:NamedIndividual>
    


    <!-- http://www.semanticweb.org/ontologies/2022/6/geological_taxonomy#Scheelite -->

    <owl:NamedIndividual rdf:about="http://www.semanticweb.org/ontologies/2022/6/geological_taxonomy#Scheelite">
        <rdf:type rdf:resource="http://www.semanticweb.org/ontologies/2022/6/geological_taxonomy#Sulfates"/>
        <rdfs:comment>Scheelite is a calcium tungstate mineral with the chemical formula CaWO4. It is an important ore of tungsten (wolfram).

Resource: https://en.wikipedia.org/wiki/Scheelite</rdfs:comment>
    </owl:NamedIndividual>
    


    <!-- http://www.semanticweb.org/ontologies/2022/6/geological_taxonomy#Schorl -->

    <owl:NamedIndividual rdf:about="http://www.semanticweb.org/ontologies/2022/6/geological_taxonomy#Schorl">
        <rdf:type rdf:resource="http://www.semanticweb.org/ontologies/2022/6/geological_taxonomy#Silicates"/>
        <rdfs:comment>Chemical Formula:NaFe2+3Al6(Si6O18)(BO3)3(OH)3(OH)

Resource: https://www.mindat.org/min-3578.html</rdfs:comment>
    </owl:NamedIndividual>
    


    <!-- http://www.semanticweb.org/ontologies/2022/6/geological_taxonomy#Scolecite -->

    <owl:NamedIndividual rdf:about="http://www.semanticweb.org/ontologies/2022/6/geological_taxonomy#Scolecite">
        <rdf:type rdf:resource="http://www.semanticweb.org/ontologies/2022/6/geological_taxonomy#Silicates"/>
        <rdfs:comment>Scolecite is a tectosilicate mineral belonging to the zeolite group; it is a hydrated calcium silicate, CaAl2Si3O10·3H2O.

Resource: https://en.wikipedia.org/wiki/Scolecite</rdfs:comment>
    </owl:NamedIndividual>
    


    <!-- http://www.semanticweb.org/ontologies/2022/6/geological_taxonomy#Serendibite -->

    <owl:NamedIndividual rdf:about="http://www.semanticweb.org/ontologies/2022/6/geological_taxonomy#Serendibite">
        <rdf:type rdf:resource="http://www.semanticweb.org/ontologies/2022/6/geological_taxonomy#Silicates"/>
        <rdfs:comment>Serendibite is an extremely rare silicate mineral that was first discovered in 1902 in Sri Lanka
Chemical Formula: Ca4[Mg6Al6]O4[Si6B3Al3O36]

Resource: https://en.wikipedia.org/wiki/Serendibite
https://www.mindat.org/min-3623.html</rdfs:comment>
    </owl:NamedIndividual>
    


    <!-- http://www.semanticweb.org/ontologies/2022/6/geological_taxonomy#Sillimanite -->

    <owl:NamedIndividual rdf:about="http://www.semanticweb.org/ontologies/2022/6/geological_taxonomy#Sillimanite">
        <rdf:type rdf:resource="http://www.semanticweb.org/ontologies/2022/6/geological_taxonomy#Silicates"/>
        <rdfs:comment>Sillimanite is an aluminosilicate mineral with the chemical formula Al2SiO5.

Resource: https://en.wikipedia.org/wiki/Sillimanite</rdfs:comment>
    </owl:NamedIndividual>
    


    <!-- http://www.semanticweb.org/ontologies/2022/6/geological_taxonomy#Sinhalite -->

    <owl:NamedIndividual rdf:about="http://www.semanticweb.org/ontologies/2022/6/geological_taxonomy#Sinhalite">
        <rdf:type rdf:resource="http://www.semanticweb.org/ontologies/2022/6/geological_taxonomy#Borates"/>
        <rdfs:comment>Sinhalite is a borate mineral with formula MgAl(BO4). 
Sinhalite was first found in Sri Lanka (Ceylon) in 1952, and was named from Sinhala - the Sanskrit name for Sri Lanka.

Resource: https://en.wikipedia.org/wiki/Sinhalite</rdfs:comment>
    </owl:NamedIndividual>
    


    <!-- http://www.semanticweb.org/ontologies/2022/6/geological_taxonomy#Smithsonite -->

    <owl:NamedIndividual rdf:about="http://www.semanticweb.org/ontologies/2022/6/geological_taxonomy#Smithsonite">
        <rdf:type rdf:resource="http://www.semanticweb.org/ontologies/2022/6/geological_taxonomy#Carbonates"/>
        <rdfs:comment>Smithsonite, also known as zinc spar, is the mineral form of zinc carbonate (ZnCO3).

Resource: https://en.wikipedia.org/wiki/Smithsonite</rdfs:comment>
    </owl:NamedIndividual>
    


    <!-- http://www.semanticweb.org/ontologies/2022/6/geological_taxonomy#Sodalite -->

    <owl:NamedIndividual rdf:about="http://www.semanticweb.org/ontologies/2022/6/geological_taxonomy#Sodalite">
        <rdf:type rdf:resource="http://www.semanticweb.org/ontologies/2022/6/geological_taxonomy#Silicates"/>
        <rdfs:comment>Sodalite is a tectosilicate mineral with the formula Na8(Al6Si6O24)Cl2, with royal blue varieties widely used as an ornamental gemstone. 

Resource: https://en.wikipedia.org/wiki/Sodalite</rdfs:comment>
    </owl:NamedIndividual>
    


    <!-- http://www.semanticweb.org/ontologies/2022/6/geological_taxonomy#Spessartine -->

    <owl:NamedIndividual rdf:about="http://www.semanticweb.org/ontologies/2022/6/geological_taxonomy#Spessartine">
        <rdf:type rdf:resource="http://www.semanticweb.org/ontologies/2022/6/geological_taxonomy#Silicates"/>
        <rdfs:comment>Spessartine is a nesosilicate, manganese aluminium garnet species, Mn2+3Al2(SiO4)3. This mineral is sometimes mistakenly referred to as spessartite.

Resource: https://en.wikipedia.org/wiki/Spessartine</rdfs:comment>
    </owl:NamedIndividual>
    


    <!-- http://www.semanticweb.org/ontologies/2022/6/geological_taxonomy#Sphalerite -->

    <owl:NamedIndividual rdf:about="http://www.semanticweb.org/ontologies/2022/6/geological_taxonomy#Sphalerite">
        <rdf:type rdf:resource="http://www.semanticweb.org/ontologies/2022/6/geological_taxonomy#Sulfides_and_Sulfosalts"/>
        <rdfs:comment>Sphalerite (sometimes spelled sphaelerite) is a sulfide mineral with the chemical formula (Zn,Fe)S. It is the most important ore of zinc.

Resource: https://en.wikipedia.org/wiki/Sphalerite</rdfs:comment>
    </owl:NamedIndividual>
    


    <!-- http://www.semanticweb.org/ontologies/2022/6/geological_taxonomy#Spinel -->

    <owl:NamedIndividual rdf:about="http://www.semanticweb.org/ontologies/2022/6/geological_taxonomy#Spinel">
        <rdf:type rdf:resource="http://www.semanticweb.org/ontologies/2022/6/geological_taxonomy#Oxides"/>
        <rdfs:comment>Spinel is the magnesium/aluminium member of the larger spinel group of minerals. It has the formula MgAl2O4 in the cubic crystal system.

Resource: https://en.wikipedia.org/wiki/Spinel</rdfs:comment>
    </owl:NamedIndividual>
    


    <!-- http://www.semanticweb.org/ontologies/2022/6/geological_taxonomy#Spodumene -->

    <owl:NamedIndividual rdf:about="http://www.semanticweb.org/ontologies/2022/6/geological_taxonomy#Spodumene">
        <rdf:type rdf:resource="http://www.semanticweb.org/ontologies/2022/6/geological_taxonomy#Silicates"/>
        <rdfs:comment>Spodumene is a pyroxene mineral consisting of lithium aluminium inosilicate, LiAl(SiO3)2, and is a source of lithium.

Resource: https://en.wikipedia.org/wiki/Spodumene</rdfs:comment>
    </owl:NamedIndividual>
    


    <!-- http://www.semanticweb.org/ontologies/2022/6/geological_taxonomy#Sugilite -->

    <owl:NamedIndividual rdf:about="http://www.semanticweb.org/ontologies/2022/6/geological_taxonomy#Sugilite">
        <rdf:type rdf:resource="http://www.semanticweb.org/ontologies/2022/6/geological_taxonomy#Silicates"/>
        <rdfs:comment>Sugilite is a relatively rare pink to purple cyclosilicate mineral with the complex chemical formula KNa2(Fe, Mn, Al)2Li3Si12O30. 

Resource: https://en.wikipedia.org/wiki/Sugilite</rdfs:comment>
    </owl:NamedIndividual>
    


    <!-- http://www.semanticweb.org/ontologies/2022/6/geological_taxonomy#Svenekite -->

    <owl:NamedIndividual rdf:about="http://www.semanticweb.org/ontologies/2022/6/geological_taxonomy#Svenekite">
        <rdf:type rdf:resource="http://www.semanticweb.org/ontologies/2022/6/geological_taxonomy#Phosphates_Arsenates_Vanadates"/>
        <rdfs:comment>Chemical Formula: Ca(H2AsO4)2

Resource: https://www.mindat.org/min-7076.html</rdfs:comment>
    </owl:NamedIndividual>
    


    <!-- http://www.semanticweb.org/ontologies/2022/6/geological_taxonomy#Swedenborgite -->

    <owl:NamedIndividual rdf:about="http://www.semanticweb.org/ontologies/2022/6/geological_taxonomy#Swedenborgite">
        <rdf:type rdf:resource="http://www.semanticweb.org/ontologies/2022/6/geological_taxonomy#Oxides"/>
        <rdfs:comment>A hexagonal-dihexagonal pyramidal mineral containing antimony, beryllium, oxygen, and sodium.
Formula:NaBe4Sb5+O7

Resource: https://en.wiktionary.org/wiki/swedenborgite
https://www.mindat.org/min-3845.html</rdfs:comment>
    </owl:NamedIndividual>
    


    <!-- http://www.semanticweb.org/ontologies/2022/6/geological_taxonomy#Tenorite -->

    <owl:NamedIndividual rdf:about="http://www.semanticweb.org/ontologies/2022/6/geological_taxonomy#Tenorite">
        <rdf:type rdf:resource="http://www.semanticweb.org/ontologies/2022/6/geological_taxonomy#Oxides"/>
        <rdfs:comment>Tenorite is a copper oxide mineral with the chemical formula CuO.

Resource: https://en.wikipedia.org/wiki/Tenorite</rdfs:comment>
    </owl:NamedIndividual>
    


    <!-- http://www.semanticweb.org/ontologies/2022/6/geological_taxonomy#Tin -->

    <owl:NamedIndividual rdf:about="http://www.semanticweb.org/ontologies/2022/6/geological_taxonomy#Tin">
        <rdf:type rdf:resource="http://www.semanticweb.org/ontologies/2022/6/geological_taxonomy#Elements"/>
        <rdfs:comment>Tin is a chemical element with the symbol Sn (from Latin: stannum) and atomic number 50. Tin is a silvery-coloured metal.

Resource: https://en.wikipedia.org/wiki/Tin</rdfs:comment>
    </owl:NamedIndividual>
    


    <!-- http://www.semanticweb.org/ontologies/2022/6/geological_taxonomy#Titanite -->

    <owl:NamedIndividual rdf:about="http://www.semanticweb.org/ontologies/2022/6/geological_taxonomy#Titanite">
        <rdf:type rdf:resource="http://www.semanticweb.org/ontologies/2022/6/geological_taxonomy#Silicates"/>
        <rdfs:comment>Titanite, or sphene (from the Greek sphenos (σφηνώ), meaning wedge[5]), is a calcium titanium nesosilicate mineral, CaTiSiO5.

Resource: https://en.wikipedia.org/wiki/Titanite</rdfs:comment>
    </owl:NamedIndividual>
    


    <!-- http://www.semanticweb.org/ontologies/2022/6/geological_taxonomy#Tolbachite -->

    <owl:NamedIndividual rdf:about="http://www.semanticweb.org/ontologies/2022/6/geological_taxonomy#Tolbachite">
        <rdf:type rdf:resource="http://www.semanticweb.org/ontologies/2022/6/geological_taxonomy#Halides"/>
        <rdfs:comment>A monoclinic-prismatic mineral containing chlorine and copper.
Formula: CuCl2

Resource: https://en.wiktionary.org/wiki/tolbachite
https://www.mindat.org/min-3990.html</rdfs:comment>
    </owl:NamedIndividual>
    


    <!-- http://www.semanticweb.org/ontologies/2022/6/geological_taxonomy#Topaz -->

    <owl:NamedIndividual rdf:about="http://www.semanticweb.org/ontologies/2022/6/geological_taxonomy#Topaz">
        <rdf:type rdf:resource="http://www.semanticweb.org/ontologies/2022/6/geological_taxonomy#Silicates"/>
        <rdfs:comment>Topaz is a silicate mineral of aluminium and fluorine with the chemical formula Al2SiO4(F,OH)2.

Resource: https://en.wikipedia.org/wiki/Topaz</rdfs:comment>
    </owl:NamedIndividual>
    


    <!-- http://www.semanticweb.org/ontologies/2022/6/geological_taxonomy#Trimerite -->

    <owl:NamedIndividual rdf:about="http://www.semanticweb.org/ontologies/2022/6/geological_taxonomy#Trimerite">
        <rdf:type rdf:resource="http://www.semanticweb.org/ontologies/2022/6/geological_taxonomy#Silicates"/>
        <rdfs:comment>A monoclinic-prismatic mineral containing beryllium, calcium, manganese, oxygen, and silicon.
Formula:CaMn2+2Be3(SiO4)3

Resource: https://en.wiktionary.org/wiki/trimerite
https://www.mindat.org/min-4018.html</rdfs:comment>
    </owl:NamedIndividual>
    


    <!-- http://www.semanticweb.org/ontologies/2022/6/geological_taxonomy#Triplite -->

    <owl:NamedIndividual rdf:about="http://www.semanticweb.org/ontologies/2022/6/geological_taxonomy#Triplite">
        <rdf:type rdf:resource="http://www.semanticweb.org/ontologies/2022/6/geological_taxonomy#Phosphates_Arsenates_Vanadates"/>
        <rdfs:comment>Triplite is a rare phosphate mineral with formula: (Mn, Fe)2PO4(F, OH). It occurs in phosphate-rich granitic pegmatites typically as irregular brown opaque masses.

Resource: https://en.wikipedia.org/wiki/Triplite</rdfs:comment>
    </owl:NamedIndividual>
    


    <!-- http://www.semanticweb.org/ontologies/2022/6/geological_taxonomy#Turquoise -->

    <owl:NamedIndividual rdf:about="http://www.semanticweb.org/ontologies/2022/6/geological_taxonomy#Turquoise">
        <rdf:type rdf:resource="http://www.semanticweb.org/ontologies/2022/6/geological_taxonomy#Phosphates_Arsenates_Vanadates"/>
        <rdfs:comment>Turquoise is an opaque, blue-to-green mineral that is a hydrated phosphate of copper and aluminium, with the chemical formula CuAl6(PO4)4(OH)8·4H2O.

Resource: https://en.wikipedia.org/wiki/Turquoise</rdfs:comment>
    </owl:NamedIndividual>
    


    <!-- http://www.semanticweb.org/ontologies/2022/6/geological_taxonomy#Uvite -->

    <owl:NamedIndividual rdf:about="http://www.semanticweb.org/ontologies/2022/6/geological_taxonomy#Uvite">
        <rdf:type rdf:resource="http://www.semanticweb.org/ontologies/2022/6/geological_taxonomy#Silicates"/>
        <rdfs:comment>Formula:CaMg3(Al5Mg)(Si6O18)(BO3)3(OH)3(OH)

Resource: https://www.mindat.org/min-54355.html</rdfs:comment>
    </owl:NamedIndividual>
    


    <!-- http://www.semanticweb.org/ontologies/2022/6/geological_taxonomy#Vanthoffite -->

    <owl:NamedIndividual rdf:about="http://www.semanticweb.org/ontologies/2022/6/geological_taxonomy#Vanthoffite">
        <rdf:type rdf:resource="http://www.semanticweb.org/ontologies/2022/6/geological_taxonomy#Sulfates"/>
        <rdfs:comment>A monoclinic-prismatic colorless mineral containing magnesium, oxygen, sodium, and sulfur. 
Formula:Na6Mg(SO4)4

Resource: https://en.wiktionary.org/wiki/vanthoffite
https://www.mindat.org/min-4151.html</rdfs:comment>
    </owl:NamedIndividual>
    


    <!-- http://www.semanticweb.org/ontologies/2022/6/geological_taxonomy#Variscite -->

    <owl:NamedIndividual rdf:about="http://www.semanticweb.org/ontologies/2022/6/geological_taxonomy#Variscite">
        <rdf:type rdf:resource="http://www.semanticweb.org/ontologies/2022/6/geological_taxonomy#Phosphates_Arsenates_Vanadates"/>
        <rdfs:comment>Variscite is a hydrated aluminium phosphate mineral (AlPO4 · 2 H2O). It is a relatively rare phosphate mineral.

Resource: https://en.wikipedia.org/wiki/Variscite</rdfs:comment>
    </owl:NamedIndividual>
    


    <!-- http://www.semanticweb.org/ontologies/2022/6/geological_taxonomy#Vesuvianite -->

    <owl:NamedIndividual rdf:about="http://www.semanticweb.org/ontologies/2022/6/geological_taxonomy#Vesuvianite">
        <rdf:type rdf:resource="http://www.semanticweb.org/ontologies/2022/6/geological_taxonomy#Silicates"/>
        <rdfs:comment>Vesuvianite, also known as idocrase, is a green, brown, yellow, or blue silicate mineral.
Chemical Formula: Ca19Fe3+Al4(Al6Mg2)(◻4)◻[Si2O7]4[(SiO4)10]O(OH)9

Resource: https://en.wikipedia.org/wiki/Vesuvianite
https://www.mindat.org/min-4223.html</rdfs:comment>
    </owl:NamedIndividual>
    


    <!-- http://www.semanticweb.org/ontologies/2022/6/geological_taxonomy#Vincentite -->

    <owl:NamedIndividual rdf:about="http://www.semanticweb.org/ontologies/2022/6/geological_taxonomy#Vincentite">
        <rdf:type rdf:resource="http://www.semanticweb.org/ontologies/2022/6/geological_taxonomy#Sulfides_and_Sulfosalts"/>
        <rdfs:comment>A monoclinic gray mineral containing antimony, arsenic, palladium, platinum, and tellurium.
Formula:Pd3As

Resource: https://en.wiktionary.org/wiki/vincentite
https://www.mindat.org/min-4184.html</rdfs:comment>
    </owl:NamedIndividual>
    


    <!-- http://www.semanticweb.org/ontologies/2022/6/geological_taxonomy#Vlasovite -->

    <owl:NamedIndividual rdf:about="http://www.semanticweb.org/ontologies/2022/6/geological_taxonomy#Vlasovite">
        <rdf:type rdf:resource="http://www.semanticweb.org/ontologies/2022/6/geological_taxonomy#Silicates"/>
        <rdfs:comment>Vlasovite is a rare inosilicate (chain silicate) mineral with sodium and zirconium, with the chemical formula Na2ZrSi4O11. It was discovered in 1961 

Resource: https://en.wikipedia.org/wiki/Vlasovite</rdfs:comment>
    </owl:NamedIndividual>
    


    <!-- http://www.semanticweb.org/ontologies/2022/6/geological_taxonomy#Väyrynenite -->

    <owl:NamedIndividual rdf:about="http://www.semanticweb.org/ontologies/2022/6/geological_taxonomy#Väyrynenite">
        <rdf:type rdf:resource="http://www.semanticweb.org/ontologies/2022/6/geological_taxonomy#Phosphates_Arsenates_Vanadates"/>
        <rdfs:comment>Väyrynenite is a rare phosphate mineral with formula MnBe(PO4)(OH,F).

Resource: https://en.wikipedia.org/wiki/V%C3%A4yrynenite</rdfs:comment>
    </owl:NamedIndividual>
    


    <!-- http://www.semanticweb.org/ontologies/2022/6/geological_taxonomy#Zabuyelite -->

    <owl:NamedIndividual rdf:about="http://www.semanticweb.org/ontologies/2022/6/geological_taxonomy#Zabuyelite">
        <rdf:type rdf:resource="http://www.semanticweb.org/ontologies/2022/6/geological_taxonomy#Carbonates"/>
        <rdfs:comment>Zabuyelite is the natural mineral form of lithium carbonate, with a formula Li2CO3. 

Resource: https://en.wikipedia.org/wiki/Zabuyelite</rdfs:comment>
    </owl:NamedIndividual>
    


    <!-- http://www.semanticweb.org/ontologies/2022/6/geological_taxonomy#Zharchikhite -->

    <owl:NamedIndividual rdf:about="http://www.semanticweb.org/ontologies/2022/6/geological_taxonomy#Zharchikhite">
        <rdf:type rdf:resource="http://www.semanticweb.org/ontologies/2022/6/geological_taxonomy#Halides"/>
        <rdfs:comment>Zharchikhite is a halide mineral, a hydroxyl fluoride of aluminium; formula AlF(OH)2. It forms colourless, transparent crystals.

Resource: https://en.wikipedia.org/wiki/Zharchikhite</rdfs:comment>
    </owl:NamedIndividual>
    


    <!-- http://www.semanticweb.org/ontologies/2022/6/geological_taxonomy#Zinc -->

    <owl:NamedIndividual rdf:about="http://www.semanticweb.org/ontologies/2022/6/geological_taxonomy#Zinc">
        <rdf:type rdf:resource="http://www.semanticweb.org/ontologies/2022/6/geological_taxonomy#Elements"/>
        <rdfs:comment>Zinc is a chemical element with the symbol Zn and atomic number 30.

Resource: https://en.wikipedia.org/wiki/Zinc</rdfs:comment>
    </owl:NamedIndividual>
    


    <!-- http://www.semanticweb.org/ontologies/2022/6/geological_taxonomy#Zircon -->

    <owl:NamedIndividual rdf:about="http://www.semanticweb.org/ontologies/2022/6/geological_taxonomy#Zircon">
        <rdf:type rdf:resource="http://www.semanticweb.org/ontologies/2022/6/geological_taxonomy#Silicates"/>
        <rdfs:comment>Zircon is a mineral belonging to the group of nesosilicates and is a source of the metal zirconium. Its chemical name is zirconium(IV) silicate, and its corresponding chemical formula is ZrSiO4.

Resource: https://en.wikipedia.org/wiki/Zircon</rdfs:comment>
    </owl:NamedIndividual>
    


    <!-- http://www.semanticweb.org/ontologies/2022/6/geological_taxonomy#Zoisite -->

    <owl:NamedIndividual rdf:about="http://www.semanticweb.org/ontologies/2022/6/geological_taxonomy#Zoisite">
        <rdf:type rdf:resource="http://www.semanticweb.org/ontologies/2022/6/geological_taxonomy#Silicates"/>
        <rdfs:comment>Zoisite, first known as saualpite, after its type locality, is a calcium aluminium hydroxy sorosilicate belonging to the epidote group of minerals. Its chemical formula is Ca2Al3(SiO4)(Si2O7)O(OH).

Resource:  https://en.wikipedia.org/wiki/Zoisite</rdfs:comment>
    </owl:NamedIndividual>
    


    <!-- http://www.semanticweb.org/ontologies/2022/6/geological_taxonomy#Axinite-(Fe) -->

    <owl:NamedIndividual rdf:about="http://www.semanticweb.org/ontologies/2022/6/geological_taxonomy#Axinite-(Fe)">
        <rdf:type rdf:resource="http://www.semanticweb.org/ontologies/2022/6/geological_taxonomy#Silicates"/>
        <rdfs:comment>Axinite-(Fe) or ferroaxinite, Ca2Fe2+Al2BOSi4O15(OH) iron rich, clove-brown, brown, plum-blue, pearl-gray

Resource: https://en.wikipedia.org/wiki/Axinite</rdfs:comment>
    </owl:NamedIndividual>
    


    <!-- http://www.semanticweb.org/ontologies/2022/6/geological_taxonomy#Axinite-(Mg) -->

    <owl:NamedIndividual rdf:about="http://www.semanticweb.org/ontologies/2022/6/geological_taxonomy#Axinite-(Mg)">
        <rdf:type rdf:resource="http://www.semanticweb.org/ontologies/2022/6/geological_taxonomy#Silicates"/>
        <rdfs:comment>Axinite-(Mg) is a borosilicate mineral of aluminum, calcium and magnesium of the axinite group, with magnesium as the dominant cation in the place of the structure that can also be occupied by iron and manganese.
Chemical Formula: Ca2MgAl2BSi4O15OH

Resource: https://en.wikipedia.org/wiki/Axinite-(Mg)
https://www.mindat.org/min-2490.html</rdfs:comment>
    </owl:NamedIndividual>
    


    <!-- http://www.semanticweb.org/ontologies/2022/6/geological_taxonomy#Bastnäsite-(Ce) -->

    <owl:NamedIndividual rdf:about="http://www.semanticweb.org/ontologies/2022/6/geological_taxonomy#Bastnäsite-(Ce)">
        <rdf:type rdf:resource="http://www.semanticweb.org/ontologies/2022/6/geological_taxonomy#Carbonates"/>
        <rdfs:comment>Chemical Formula: Ce(CO3)F

Resource: https://www.mindat.org/min-560.html</rdfs:comment>
    </owl:NamedIndividual>
    


    <!-- http://www.semanticweb.org/ontologies/2022/6/geological_taxonomy#Gadolinite-(Y) -->

    <owl:NamedIndividual rdf:about="http://www.semanticweb.org/ontologies/2022/6/geological_taxonomy#Gadolinite-(Y)">
        <rdf:type rdf:resource="http://www.semanticweb.org/ontologies/2022/6/geological_taxonomy#Silicates"/>
        <rdfs:comment>Chemical Formula: Y2Fe2+Be2Si2O10

Resource: https://www.mindat.org/min-1628.html</rdfs:comment>
    </owl:NamedIndividual>
    


    <!-- http://www.semanticweb.org/ontologies/2022/6/geological_taxonomy#Remondite-(Ce) -->

    <owl:NamedIndividual rdf:about="http://www.semanticweb.org/ontologies/2022/6/geological_taxonomy#Remondite-(Ce)">
        <rdf:type rdf:resource="http://www.semanticweb.org/ontologies/2022/6/geological_taxonomy#Carbonates"/>
        <rdfs:comment>Chemical Formula: Na3(Ca,Ce,La,Na,Sr)3(CO3)5 
The mineral is named in honor of Dr. Guy Rémond, a physicist for the Bureau de Recherches Géologiques et Minières in Orléans, France.
Found only in Cameroon, Canada, and purportedly Russia, Remondite occurs at its Cameroon locality in nepheline syenite, and as its Canadian locality “associated with an intrusive alkalic gabbro-syenite complex.”

Resource: https://www.dakotamatrix.com/mineralpedia/7351/remondite-ce</rdfs:comment>
    </owl:NamedIndividual>
    


    <!-- http://www.semanticweb.org/ontologies/2022/6/geological_taxonomy#Sahamalite-(Ce) -->

    <owl:NamedIndividual rdf:about="http://www.semanticweb.org/ontologies/2022/6/geological_taxonomy#Sahamalite-(Ce)">
        <rdf:type rdf:resource="http://www.semanticweb.org/ontologies/2022/6/geological_taxonomy#Carbonates"/>
        <rdfs:comment>Chemical Formula: (Mg,Fe++)Ce2(CO3)4

Resource: http://www.webmineral.com/data/Sahamalite-(Ce).shtml#.Yy70-HZBzIU</rdfs:comment>
    </owl:NamedIndividual>
    


    <!-- 
    ///////////////////////////////////////////////////////////////////////////////////////
    //
    // Annotations
    //
    ///////////////////////////////////////////////////////////////////////////////////////
     -->

    <rdf:Description rdf:about="http://www.semanticweb.org/ontologies/2022/6/geological_taxonomy#Dolomite">
        <rdfs:comment>Dolomite (also known as dolomite rock, dolostone or dolomitic rock) is a sedimentary carbonate rock that contains a high percentage of the mineral dolomite, CaMg(CO3)2. 

Resource: https://en.wikipedia.org/wiki/Dolomite_(rock)</rdfs:comment>
    </rdf:Description>
    


    <!-- 
    ///////////////////////////////////////////////////////////////////////////////////////
    //
    // General axioms
    //
    ///////////////////////////////////////////////////////////////////////////////////////
     -->

    <rdf:Description>
        <rdf:type rdf:resource="http://www.w3.org/2002/07/owl#AllDisjointClasses"/>
        <owl:members rdf:parseType="Collection">
            <rdf:Description rdf:about="http://www.semanticweb.org/ontologies/2022/6/geological_taxonomy#Abnormally_Dry"/>
            <rdf:Description rdf:about="http://www.semanticweb.org/ontologies/2022/6/geological_taxonomy#Exceptional_Drought"/>
            <rdf:Description rdf:about="http://www.semanticweb.org/ontologies/2022/6/geological_taxonomy#Extreme_Drought"/>
            <rdf:Description rdf:about="http://www.semanticweb.org/ontologies/2022/6/geological_taxonomy#Moderate_Drought"/>
            <rdf:Description rdf:about="http://www.semanticweb.org/ontologies/2022/6/geological_taxonomy#Severe_Drought"/>
        </owl:members>
    </rdf:Description>
    <rdf:Description>
        <rdf:type rdf:resource="http://www.w3.org/2002/07/owl#AllDisjointClasses"/>
        <owl:members rdf:parseType="Collection">
            <rdf:Description rdf:about="http://www.semanticweb.org/ontologies/2022/6/geological_taxonomy#Adakite"/>
            <rdf:Description rdf:about="http://www.semanticweb.org/ontologies/2022/6/geological_taxonomy#Hawaiite"/>
            <rdf:Description rdf:about="http://www.semanticweb.org/ontologies/2022/6/geological_taxonomy#Pāhoehoe"/>
            <rdf:Description rdf:about="http://www.semanticweb.org/ontologies/2022/6/geological_taxonomy#ʻAʻā"/>
        </owl:members>
    </rdf:Description>
    <rdf:Description>
        <rdf:type rdf:resource="http://www.w3.org/2002/07/owl#AllDisjointClasses"/>
        <owl:members rdf:parseType="Collection">
            <rdf:Description rdf:about="http://www.semanticweb.org/ontologies/2022/6/geological_taxonomy#Albolls"/>
            <rdf:Description rdf:about="http://www.semanticweb.org/ontologies/2022/6/geological_taxonomy#Aquolls"/>
            <rdf:Description rdf:about="http://www.semanticweb.org/ontologies/2022/6/geological_taxonomy#Cryolls"/>
            <rdf:Description rdf:about="http://www.semanticweb.org/ontologies/2022/6/geological_taxonomy#Gelolls"/>
            <rdf:Description rdf:about="http://www.semanticweb.org/ontologies/2022/6/geological_taxonomy#Rendolls"/>
            <rdf:Description rdf:about="http://www.semanticweb.org/ontologies/2022/6/geological_taxonomy#Udolls"/>
            <rdf:Description rdf:about="http://www.semanticweb.org/ontologies/2022/6/geological_taxonomy#Ustolls"/>
            <rdf:Description rdf:about="http://www.semanticweb.org/ontologies/2022/6/geological_taxonomy#Xerolls"/>
        </owl:members>
    </rdf:Description>
    <rdf:Description>
        <rdf:type rdf:resource="http://www.w3.org/2002/07/owl#AllDisjointClasses"/>
        <owl:members rdf:parseType="Collection">
            <rdf:Description rdf:about="http://www.semanticweb.org/ontologies/2022/6/geological_taxonomy#Alfisols"/>
            <rdf:Description rdf:about="http://www.semanticweb.org/ontologies/2022/6/geological_taxonomy#Andisols"/>
            <rdf:Description rdf:about="http://www.semanticweb.org/ontologies/2022/6/geological_taxonomy#Aridisols"/>
            <rdf:Description rdf:about="http://www.semanticweb.org/ontologies/2022/6/geological_taxonomy#Entisols"/>
            <rdf:Description rdf:about="http://www.semanticweb.org/ontologies/2022/6/geological_taxonomy#Gelisols"/>
            <rdf:Description rdf:about="http://www.semanticweb.org/ontologies/2022/6/geological_taxonomy#Histosols"/>
            <rdf:Description rdf:about="http://www.semanticweb.org/ontologies/2022/6/geological_taxonomy#Inceptisols"/>
            <rdf:Description rdf:about="http://www.semanticweb.org/ontologies/2022/6/geological_taxonomy#Mollisols"/>
            <rdf:Description rdf:about="http://www.semanticweb.org/ontologies/2022/6/geological_taxonomy#Oxisols"/>
            <rdf:Description rdf:about="http://www.semanticweb.org/ontologies/2022/6/geological_taxonomy#Spodosols"/>
            <rdf:Description rdf:about="http://www.semanticweb.org/ontologies/2022/6/geological_taxonomy#Ultisols"/>
            <rdf:Description rdf:about="http://www.semanticweb.org/ontologies/2022/6/geological_taxonomy#Vertisols"/>
        </owl:members>
    </rdf:Description>
    <rdf:Description>
        <rdf:type rdf:resource="http://www.w3.org/2002/07/owl#AllDisjointClasses"/>
        <owl:members rdf:parseType="Collection">
            <rdf:Description rdf:about="http://www.semanticweb.org/ontologies/2022/6/geological_taxonomy#Alkali_feldspar_granite"/>
            <rdf:Description rdf:about="http://www.semanticweb.org/ontologies/2022/6/geological_taxonomy#Andesite"/>
            <rdf:Description rdf:about="http://www.semanticweb.org/ontologies/2022/6/geological_taxonomy#Anorthosite"/>
            <rdf:Description rdf:about="http://www.semanticweb.org/ontologies/2022/6/geological_taxonomy#Aplite"/>
            <rdf:Description rdf:about="http://www.semanticweb.org/ontologies/2022/6/geological_taxonomy#Basalt"/>
            <rdf:Description rdf:about="http://www.semanticweb.org/ontologies/2022/6/geological_taxonomy#Basanite"/>
            <rdf:Description rdf:about="http://www.semanticweb.org/ontologies/2022/6/geological_taxonomy#Blairmorite"/>
            <rdf:Description rdf:about="http://www.semanticweb.org/ontologies/2022/6/geological_taxonomy#Boninite"/>
            <rdf:Description rdf:about="http://www.semanticweb.org/ontologies/2022/6/geological_taxonomy#Carbonatite"/>
            <rdf:Description rdf:about="http://www.semanticweb.org/ontologies/2022/6/geological_taxonomy#Charnockite"/>
            <rdf:Description rdf:about="http://www.semanticweb.org/ontologies/2022/6/geological_taxonomy#Dacite"/>
            <rdf:Description rdf:about="http://www.semanticweb.org/ontologies/2022/6/geological_taxonomy#Diabase"/>
            <rdf:Description rdf:about="http://www.semanticweb.org/ontologies/2022/6/geological_taxonomy#Diorite"/>
            <rdf:Description rdf:about="http://www.semanticweb.org/ontologies/2022/6/geological_taxonomy#Dunite"/>
            <rdf:Description rdf:about="http://www.semanticweb.org/ontologies/2022/6/geological_taxonomy#Essexite"/>
            <rdf:Description rdf:about="http://www.semanticweb.org/ontologies/2022/6/geological_taxonomy#Foidolite"/>
            <rdf:Description rdf:about="http://www.semanticweb.org/ontologies/2022/6/geological_taxonomy#Foyaite"/>
            <rdf:Description rdf:about="http://www.semanticweb.org/ontologies/2022/6/geological_taxonomy#Gabbro"/>
            <rdf:Description rdf:about="http://www.semanticweb.org/ontologies/2022/6/geological_taxonomy#Granite"/>
            <rdf:Description rdf:about="http://www.semanticweb.org/ontologies/2022/6/geological_taxonomy#Granodiorite"/>
            <rdf:Description rdf:about="http://www.semanticweb.org/ontologies/2022/6/geological_taxonomy#Granophyre"/>
            <rdf:Description rdf:about="http://www.semanticweb.org/ontologies/2022/6/geological_taxonomy#Harzburgite"/>
            <rdf:Description rdf:about="http://www.semanticweb.org/ontologies/2022/6/geological_taxonomy#Hornblendite"/>
            <rdf:Description rdf:about="http://www.semanticweb.org/ontologies/2022/6/geological_taxonomy#Hyaloclastite"/>
            <rdf:Description rdf:about="http://www.semanticweb.org/ontologies/2022/6/geological_taxonomy#Icelandite"/>
            <rdf:Description rdf:about="http://www.semanticweb.org/ontologies/2022/6/geological_taxonomy#Ignimbrite"/>
            <rdf:Description rdf:about="http://www.semanticweb.org/ontologies/2022/6/geological_taxonomy#Ijolite"/>
            <rdf:Description rdf:about="http://www.semanticweb.org/ontologies/2022/6/geological_taxonomy#Kimberlite"/>
            <rdf:Description rdf:about="http://www.semanticweb.org/ontologies/2022/6/geological_taxonomy#Komatiite"/>
            <rdf:Description rdf:about="http://www.semanticweb.org/ontologies/2022/6/geological_taxonomy#Lamproite"/>
            <rdf:Description rdf:about="http://www.semanticweb.org/ontologies/2022/6/geological_taxonomy#Lamprophyre"/>
            <rdf:Description rdf:about="http://www.semanticweb.org/ontologies/2022/6/geological_taxonomy#Latite"/>
            <rdf:Description rdf:about="http://www.semanticweb.org/ontologies/2022/6/geological_taxonomy#Lherzolite"/>
            <rdf:Description rdf:about="http://www.semanticweb.org/ontologies/2022/6/geological_taxonomy#Limburgite"/>
            <rdf:Description rdf:about="http://www.semanticweb.org/ontologies/2022/6/geological_taxonomy#Monzogranite"/>
            <rdf:Description rdf:about="http://www.semanticweb.org/ontologies/2022/6/geological_taxonomy#Monzonite"/>
            <rdf:Description rdf:about="http://www.semanticweb.org/ontologies/2022/6/geological_taxonomy#Nepheline_syenite"/>
            <rdf:Description rdf:about="http://www.semanticweb.org/ontologies/2022/6/geological_taxonomy#Nephelinite"/>
            <rdf:Description rdf:about="http://www.semanticweb.org/ontologies/2022/6/geological_taxonomy#Norite"/>
            <rdf:Description rdf:about="http://www.semanticweb.org/ontologies/2022/6/geological_taxonomy#Obsidian"/>
            <rdf:Description rdf:about="http://www.semanticweb.org/ontologies/2022/6/geological_taxonomy#Pegmatite"/>
            <rdf:Description rdf:about="http://www.semanticweb.org/ontologies/2022/6/geological_taxonomy#Peridotite"/>
            <rdf:Description rdf:about="http://www.semanticweb.org/ontologies/2022/6/geological_taxonomy#Phonolite"/>
            <rdf:Description rdf:about="http://www.semanticweb.org/ontologies/2022/6/geological_taxonomy#Phonotephrite"/>
            <rdf:Description rdf:about="http://www.semanticweb.org/ontologies/2022/6/geological_taxonomy#Picrite"/>
            <rdf:Description rdf:about="http://www.semanticweb.org/ontologies/2022/6/geological_taxonomy#Porphyry"/>
            <rdf:Description rdf:about="http://www.semanticweb.org/ontologies/2022/6/geological_taxonomy#Pumice"/>
            <rdf:Description rdf:about="http://www.semanticweb.org/ontologies/2022/6/geological_taxonomy#Pyroxenite"/>
            <rdf:Description rdf:about="http://www.semanticweb.org/ontologies/2022/6/geological_taxonomy#Quartz_diorite"/>
            <rdf:Description rdf:about="http://www.semanticweb.org/ontologies/2022/6/geological_taxonomy#Quartz_monzonite"/>
            <rdf:Description rdf:about="http://www.semanticweb.org/ontologies/2022/6/geological_taxonomy#Quartzolite"/>
            <rdf:Description rdf:about="http://www.semanticweb.org/ontologies/2022/6/geological_taxonomy#Rapakivi"/>
            <rdf:Description rdf:about="http://www.semanticweb.org/ontologies/2022/6/geological_taxonomy#Rhomb-porphyry"/>
            <rdf:Description rdf:about="http://www.semanticweb.org/ontologies/2022/6/geological_taxonomy#Rhyodacite"/>
            <rdf:Description rdf:about="http://www.semanticweb.org/ontologies/2022/6/geological_taxonomy#Rhyolite"/>
            <rdf:Description rdf:about="http://www.semanticweb.org/ontologies/2022/6/geological_taxonomy#Scoria"/>
            <rdf:Description rdf:about="http://www.semanticweb.org/ontologies/2022/6/geological_taxonomy#Shonkinite"/>
            <rdf:Description rdf:about="http://www.semanticweb.org/ontologies/2022/6/geological_taxonomy#Sovite"/>
            <rdf:Description rdf:about="http://www.semanticweb.org/ontologies/2022/6/geological_taxonomy#Syenite"/>
            <rdf:Description rdf:about="http://www.semanticweb.org/ontologies/2022/6/geological_taxonomy#Sövite"/>
            <rdf:Description rdf:about="http://www.semanticweb.org/ontologies/2022/6/geological_taxonomy#Tachylyte"/>
            <rdf:Description rdf:about="http://www.semanticweb.org/ontologies/2022/6/geological_taxonomy#Tephriphonolite"/>
            <rdf:Description rdf:about="http://www.semanticweb.org/ontologies/2022/6/geological_taxonomy#Tephrite"/>
            <rdf:Description rdf:about="http://www.semanticweb.org/ontologies/2022/6/geological_taxonomy#Tonalite"/>
            <rdf:Description rdf:about="http://www.semanticweb.org/ontologies/2022/6/geological_taxonomy#Trachyandesite"/>
            <rdf:Description rdf:about="http://www.semanticweb.org/ontologies/2022/6/geological_taxonomy#Trachybasalt"/>
            <rdf:Description rdf:about="http://www.semanticweb.org/ontologies/2022/6/geological_taxonomy#Trachyte"/>
            <rdf:Description rdf:about="http://www.semanticweb.org/ontologies/2022/6/geological_taxonomy#Troctolite"/>
            <rdf:Description rdf:about="http://www.semanticweb.org/ontologies/2022/6/geological_taxonomy#Trondhjemite"/>
            <rdf:Description rdf:about="http://www.semanticweb.org/ontologies/2022/6/geological_taxonomy#Tuff"/>
            <rdf:Description rdf:about="http://www.semanticweb.org/ontologies/2022/6/geological_taxonomy#Websterite"/>
            <rdf:Description rdf:about="http://www.semanticweb.org/ontologies/2022/6/geological_taxonomy#Wehrlite"/>
        </owl:members>
    </rdf:Description>
    <rdf:Description>
        <rdf:type rdf:resource="http://www.w3.org/2002/07/owl#AllDisjointClasses"/>
        <owl:members rdf:parseType="Collection">
            <rdf:Description rdf:about="http://www.semanticweb.org/ontologies/2022/6/geological_taxonomy#Amphibolite"/>
            <rdf:Description rdf:about="http://www.semanticweb.org/ontologies/2022/6/geological_taxonomy#Anthracite"/>
            <rdf:Description rdf:about="http://www.semanticweb.org/ontologies/2022/6/geological_taxonomy#Blueschist"/>
            <rdf:Description rdf:about="http://www.semanticweb.org/ontologies/2022/6/geological_taxonomy#Cataclasite"/>
            <rdf:Description rdf:about="http://www.semanticweb.org/ontologies/2022/6/geological_taxonomy#Eclogite"/>
            <rdf:Description rdf:about="http://www.semanticweb.org/ontologies/2022/6/geological_taxonomy#Epidosite"/>
            <rdf:Description rdf:about="http://www.semanticweb.org/ontologies/2022/6/geological_taxonomy#Fenite"/>
            <rdf:Description rdf:about="http://www.semanticweb.org/ontologies/2022/6/geological_taxonomy#Gneiss"/>
            <rdf:Description rdf:about="http://www.semanticweb.org/ontologies/2022/6/geological_taxonomy#Gossan"/>
            <rdf:Description rdf:about="http://www.semanticweb.org/ontologies/2022/6/geological_taxonomy#Granulite"/>
            <rdf:Description rdf:about="http://www.semanticweb.org/ontologies/2022/6/geological_taxonomy#Greenschist"/>
            <rdf:Description rdf:about="http://www.semanticweb.org/ontologies/2022/6/geological_taxonomy#Greisen"/>
            <rdf:Description rdf:about="http://www.semanticweb.org/ontologies/2022/6/geological_taxonomy#Hornfels"/>
            <rdf:Description rdf:about="http://www.semanticweb.org/ontologies/2022/6/geological_taxonomy#Litchfieldite"/>
            <rdf:Description rdf:about="http://www.semanticweb.org/ontologies/2022/6/geological_taxonomy#Marble"/>
            <rdf:Description rdf:about="http://www.semanticweb.org/ontologies/2022/6/geological_taxonomy#Metapelite"/>
            <rdf:Description rdf:about="http://www.semanticweb.org/ontologies/2022/6/geological_taxonomy#Metapsammite"/>
            <rdf:Description rdf:about="http://www.semanticweb.org/ontologies/2022/6/geological_taxonomy#Migmatite"/>
            <rdf:Description rdf:about="http://www.semanticweb.org/ontologies/2022/6/geological_taxonomy#Mylonite"/>
            <rdf:Description rdf:about="http://www.semanticweb.org/ontologies/2022/6/geological_taxonomy#Phyllite"/>
            <rdf:Description rdf:about="http://www.semanticweb.org/ontologies/2022/6/geological_taxonomy#Pseudotachylite"/>
            <rdf:Description rdf:about="http://www.semanticweb.org/ontologies/2022/6/geological_taxonomy#Quartzite"/>
            <rdf:Description rdf:about="http://www.semanticweb.org/ontologies/2022/6/geological_taxonomy#Schist"/>
            <rdf:Description rdf:about="http://www.semanticweb.org/ontologies/2022/6/geological_taxonomy#Serpentinite"/>
            <rdf:Description rdf:about="http://www.semanticweb.org/ontologies/2022/6/geological_taxonomy#Shungite"/>
            <rdf:Description rdf:about="http://www.semanticweb.org/ontologies/2022/6/geological_taxonomy#Skarn"/>
            <rdf:Description rdf:about="http://www.semanticweb.org/ontologies/2022/6/geological_taxonomy#Slate"/>
            <rdf:Description rdf:about="http://www.semanticweb.org/ontologies/2022/6/geological_taxonomy#Suevite"/>
            <rdf:Description rdf:about="http://www.semanticweb.org/ontologies/2022/6/geological_taxonomy#Talc_carbonate"/>
            <rdf:Description rdf:about="http://www.semanticweb.org/ontologies/2022/6/geological_taxonomy#Tectonite"/>
            <rdf:Description rdf:about="http://www.semanticweb.org/ontologies/2022/6/geological_taxonomy#Whiteschist"/>
            <rdf:Description rdf:about="http://www.semanticweb.org/ontologies/2022/6/geological_taxonomy#protolith"/>
        </owl:members>
    </rdf:Description>
    <rdf:Description>
        <rdf:type rdf:resource="http://www.w3.org/2002/07/owl#AllDisjointClasses"/>
        <owl:members rdf:parseType="Collection">
            <rdf:Description rdf:about="http://www.semanticweb.org/ontologies/2022/6/geological_taxonomy#Anthrepts"/>
            <rdf:Description rdf:about="http://www.semanticweb.org/ontologies/2022/6/geological_taxonomy#Aquepts"/>
            <rdf:Description rdf:about="http://www.semanticweb.org/ontologies/2022/6/geological_taxonomy#Cryepts"/>
            <rdf:Description rdf:about="http://www.semanticweb.org/ontologies/2022/6/geological_taxonomy#Gelepts"/>
            <rdf:Description rdf:about="http://www.semanticweb.org/ontologies/2022/6/geological_taxonomy#Udepts"/>
            <rdf:Description rdf:about="http://www.semanticweb.org/ontologies/2022/6/geological_taxonomy#Ustepts"/>
            <rdf:Description rdf:about="http://www.semanticweb.org/ontologies/2022/6/geological_taxonomy#Xerepts"/>
        </owl:members>
    </rdf:Description>
    <rdf:Description>
        <rdf:type rdf:resource="http://www.w3.org/2002/07/owl#AllDisjointClasses"/>
        <owl:members rdf:parseType="Collection">
            <rdf:Description rdf:about="http://www.semanticweb.org/ontologies/2022/6/geological_taxonomy#Aqualfs"/>
            <rdf:Description rdf:about="http://www.semanticweb.org/ontologies/2022/6/geological_taxonomy#Cryalfs"/>
            <rdf:Description rdf:about="http://www.semanticweb.org/ontologies/2022/6/geological_taxonomy#Udalfs"/>
            <rdf:Description rdf:about="http://www.semanticweb.org/ontologies/2022/6/geological_taxonomy#Ustalfs"/>
            <rdf:Description rdf:about="http://www.semanticweb.org/ontologies/2022/6/geological_taxonomy#Xeralfs"/>
        </owl:members>
    </rdf:Description>
    <rdf:Description>
        <rdf:type rdf:resource="http://www.w3.org/2002/07/owl#AllDisjointClasses"/>
        <owl:members rdf:parseType="Collection">
            <rdf:Description rdf:about="http://www.semanticweb.org/ontologies/2022/6/geological_taxonomy#Aquands"/>
            <rdf:Description rdf:about="http://www.semanticweb.org/ontologies/2022/6/geological_taxonomy#Cryands"/>
            <rdf:Description rdf:about="http://www.semanticweb.org/ontologies/2022/6/geological_taxonomy#Gelands"/>
            <rdf:Description rdf:about="http://www.semanticweb.org/ontologies/2022/6/geological_taxonomy#Torrands"/>
            <rdf:Description rdf:about="http://www.semanticweb.org/ontologies/2022/6/geological_taxonomy#Udands"/>
            <rdf:Description rdf:about="http://www.semanticweb.org/ontologies/2022/6/geological_taxonomy#Ustands"/>
            <rdf:Description rdf:about="http://www.semanticweb.org/ontologies/2022/6/geological_taxonomy#Vitrands"/>
            <rdf:Description rdf:about="http://www.semanticweb.org/ontologies/2022/6/geological_taxonomy#Xerands"/>
        </owl:members>
    </rdf:Description>
    <rdf:Description>
        <rdf:type rdf:resource="http://www.w3.org/2002/07/owl#AllDisjointClasses"/>
        <owl:members rdf:parseType="Collection">
            <rdf:Description rdf:about="http://www.semanticweb.org/ontologies/2022/6/geological_taxonomy#Aquents"/>
            <rdf:Description rdf:about="http://www.semanticweb.org/ontologies/2022/6/geological_taxonomy#Arents"/>
            <rdf:Description rdf:about="http://www.semanticweb.org/ontologies/2022/6/geological_taxonomy#Fluvents"/>
            <rdf:Description rdf:about="http://www.semanticweb.org/ontologies/2022/6/geological_taxonomy#Orthents"/>
            <rdf:Description rdf:about="http://www.semanticweb.org/ontologies/2022/6/geological_taxonomy#Psamments"/>
        </owl:members>
    </rdf:Description>
    <rdf:Description>
        <rdf:type rdf:resource="http://www.w3.org/2002/07/owl#AllDisjointClasses"/>
        <owl:members rdf:parseType="Collection">
            <rdf:Description rdf:about="http://www.semanticweb.org/ontologies/2022/6/geological_taxonomy#Aquerts"/>
            <rdf:Description rdf:about="http://www.semanticweb.org/ontologies/2022/6/geological_taxonomy#Cryerts"/>
            <rdf:Description rdf:about="http://www.semanticweb.org/ontologies/2022/6/geological_taxonomy#Torrerts"/>
            <rdf:Description rdf:about="http://www.semanticweb.org/ontologies/2022/6/geological_taxonomy#Uderts"/>
            <rdf:Description rdf:about="http://www.semanticweb.org/ontologies/2022/6/geological_taxonomy#Usterts"/>
            <rdf:Description rdf:about="http://www.semanticweb.org/ontologies/2022/6/geological_taxonomy#Xererts"/>
        </owl:members>
    </rdf:Description>
    <rdf:Description>
        <rdf:type rdf:resource="http://www.w3.org/2002/07/owl#AllDisjointClasses"/>
        <owl:members rdf:parseType="Collection">
            <rdf:Description rdf:about="http://www.semanticweb.org/ontologies/2022/6/geological_taxonomy#Aquods"/>
            <rdf:Description rdf:about="http://www.semanticweb.org/ontologies/2022/6/geological_taxonomy#Cryods"/>
            <rdf:Description rdf:about="http://www.semanticweb.org/ontologies/2022/6/geological_taxonomy#Gelods"/>
            <rdf:Description rdf:about="http://www.semanticweb.org/ontologies/2022/6/geological_taxonomy#Humods"/>
            <rdf:Description rdf:about="http://www.semanticweb.org/ontologies/2022/6/geological_taxonomy#Orthods"/>
        </owl:members>
    </rdf:Description>
    <rdf:Description>
        <rdf:type rdf:resource="http://www.w3.org/2002/07/owl#AllDisjointClasses"/>
        <owl:members rdf:parseType="Collection">
            <rdf:Description rdf:about="http://www.semanticweb.org/ontologies/2022/6/geological_taxonomy#Aquox"/>
            <rdf:Description rdf:about="http://www.semanticweb.org/ontologies/2022/6/geological_taxonomy#Perox"/>
            <rdf:Description rdf:about="http://www.semanticweb.org/ontologies/2022/6/geological_taxonomy#Torrox"/>
            <rdf:Description rdf:about="http://www.semanticweb.org/ontologies/2022/6/geological_taxonomy#Udox"/>
            <rdf:Description rdf:about="http://www.semanticweb.org/ontologies/2022/6/geological_taxonomy#Ustox"/>
        </owl:members>
    </rdf:Description>
    <rdf:Description>
        <rdf:type rdf:resource="http://www.w3.org/2002/07/owl#AllDisjointClasses"/>
        <owl:members rdf:parseType="Collection">
            <rdf:Description rdf:about="http://www.semanticweb.org/ontologies/2022/6/geological_taxonomy#Aquults"/>
            <rdf:Description rdf:about="http://www.semanticweb.org/ontologies/2022/6/geological_taxonomy#Humults"/>
            <rdf:Description rdf:about="http://www.semanticweb.org/ontologies/2022/6/geological_taxonomy#Udults"/>
            <rdf:Description rdf:about="http://www.semanticweb.org/ontologies/2022/6/geological_taxonomy#Ustults"/>
            <rdf:Description rdf:about="http://www.semanticweb.org/ontologies/2022/6/geological_taxonomy#Xerults"/>
        </owl:members>
    </rdf:Description>
    <rdf:Description>
        <rdf:type rdf:resource="http://www.w3.org/2002/07/owl#AllDisjointClasses"/>
        <owl:members rdf:parseType="Collection">
            <rdf:Description rdf:about="http://www.semanticweb.org/ontologies/2022/6/geological_taxonomy#Areal"/>
            <rdf:Description rdf:about="http://www.semanticweb.org/ontologies/2022/6/geological_taxonomy#Coastal_Flood"/>
            <rdf:Description rdf:about="http://www.semanticweb.org/ontologies/2022/6/geological_taxonomy#Flash_flood"/>
            <rdf:Description rdf:about="http://www.semanticweb.org/ontologies/2022/6/geological_taxonomy#Riverine_(Channel)_Flood"/>
        </owl:members>
    </rdf:Description>
    <rdf:Description>
        <rdf:type rdf:resource="http://www.w3.org/2002/07/owl#AllDisjointClasses"/>
        <owl:members rdf:parseType="Collection">
            <rdf:Description rdf:about="http://www.semanticweb.org/ontologies/2022/6/geological_taxonomy#Argids"/>
            <rdf:Description rdf:about="http://www.semanticweb.org/ontologies/2022/6/geological_taxonomy#Calcids"/>
            <rdf:Description rdf:about="http://www.semanticweb.org/ontologies/2022/6/geological_taxonomy#Cambids"/>
            <rdf:Description rdf:about="http://www.semanticweb.org/ontologies/2022/6/geological_taxonomy#Cryids"/>
            <rdf:Description rdf:about="http://www.semanticweb.org/ontologies/2022/6/geological_taxonomy#Durids"/>
            <rdf:Description rdf:about="http://www.semanticweb.org/ontologies/2022/6/geological_taxonomy#Gypsids"/>
            <rdf:Description rdf:about="http://www.semanticweb.org/ontologies/2022/6/geological_taxonomy#Salids"/>
        </owl:members>
    </rdf:Description>
    <rdf:Description>
        <rdf:type rdf:resource="http://www.w3.org/2002/07/owl#AllDisjointClasses"/>
        <owl:members rdf:parseType="Collection">
            <rdf:Description rdf:about="http://www.semanticweb.org/ontologies/2022/6/geological_taxonomy#Argillite"/>
            <rdf:Description rdf:about="http://www.semanticweb.org/ontologies/2022/6/geological_taxonomy#Arkose"/>
            <rdf:Description rdf:about="http://www.semanticweb.org/ontologies/2022/6/geological_taxonomy#Banded_iron_formation"/>
            <rdf:Description rdf:about="http://www.semanticweb.org/ontologies/2022/6/geological_taxonomy#Bauxite"/>
            <rdf:Description rdf:about="http://www.semanticweb.org/ontologies/2022/6/geological_taxonomy#Bog_iron"/>
            <rdf:Description rdf:about="http://www.semanticweb.org/ontologies/2022/6/geological_taxonomy#Breccia"/>
            <rdf:Description rdf:about="http://www.semanticweb.org/ontologies/2022/6/geological_taxonomy#Calcarenite"/>
            <rdf:Description rdf:about="http://www.semanticweb.org/ontologies/2022/6/geological_taxonomy#Chalk"/>
            <rdf:Description rdf:about="http://www.semanticweb.org/ontologies/2022/6/geological_taxonomy#Chert"/>
            <rdf:Description rdf:about="http://www.semanticweb.org/ontologies/2022/6/geological_taxonomy#Claystone"/>
            <rdf:Description rdf:about="http://www.semanticweb.org/ontologies/2022/6/geological_taxonomy#Coal"/>
            <rdf:Description rdf:about="http://www.semanticweb.org/ontologies/2022/6/geological_taxonomy#Conglomerate"/>
            <rdf:Description rdf:about="http://www.semanticweb.org/ontologies/2022/6/geological_taxonomy#Coquina"/>
            <rdf:Description rdf:about="http://www.semanticweb.org/ontologies/2022/6/geological_taxonomy#Diatomite"/>
            <rdf:Description rdf:about="http://www.semanticweb.org/ontologies/2022/6/geological_taxonomy#Dolomite"/>
            <rdf:Description rdf:about="http://www.semanticweb.org/ontologies/2022/6/geological_taxonomy#Evaporite"/>
            <rdf:Description rdf:about="http://www.semanticweb.org/ontologies/2022/6/geological_taxonomy#Flint"/>
            <rdf:Description rdf:about="http://www.semanticweb.org/ontologies/2022/6/geological_taxonomy#Geyserite"/>
            <rdf:Description rdf:about="http://www.semanticweb.org/ontologies/2022/6/geological_taxonomy#Graywacke"/>
            <rdf:Description rdf:about="http://www.semanticweb.org/ontologies/2022/6/geological_taxonomy#Greywacke"/>
            <rdf:Description rdf:about="http://www.semanticweb.org/ontologies/2022/6/geological_taxonomy#Gritstone"/>
            <rdf:Description rdf:about="http://www.semanticweb.org/ontologies/2022/6/geological_taxonomy#Gypsum"/>
            <rdf:Description rdf:about="http://www.semanticweb.org/ontologies/2022/6/geological_taxonomy#Itacolumite"/>
            <rdf:Description rdf:about="http://www.semanticweb.org/ontologies/2022/6/geological_taxonomy#Jaspillite"/>
            <rdf:Description rdf:about="http://www.semanticweb.org/ontologies/2022/6/geological_taxonomy#Laterite"/>
            <rdf:Description rdf:about="http://www.semanticweb.org/ontologies/2022/6/geological_taxonomy#Lignite"/>
            <rdf:Description rdf:about="http://www.semanticweb.org/ontologies/2022/6/geological_taxonomy#Limestone"/>
            <rdf:Description rdf:about="http://www.semanticweb.org/ontologies/2022/6/geological_taxonomy#Marl"/>
            <rdf:Description rdf:about="http://www.semanticweb.org/ontologies/2022/6/geological_taxonomy#Mudstone"/>
            <rdf:Description rdf:about="http://www.semanticweb.org/ontologies/2022/6/geological_taxonomy#Oil_shale"/>
            <rdf:Description rdf:about="http://www.semanticweb.org/ontologies/2022/6/geological_taxonomy#Oolite"/>
            <rdf:Description rdf:about="http://www.semanticweb.org/ontologies/2022/6/geological_taxonomy#Phosphorite"/>
            <rdf:Description rdf:about="http://www.semanticweb.org/ontologies/2022/6/geological_taxonomy#Rock_Gypsum-"/>
            <rdf:Description rdf:about="http://www.semanticweb.org/ontologies/2022/6/geological_taxonomy#Sandstone"/>
            <rdf:Description rdf:about="http://www.semanticweb.org/ontologies/2022/6/geological_taxonomy#Shale"/>
            <rdf:Description rdf:about="http://www.semanticweb.org/ontologies/2022/6/geological_taxonomy#Siltstone"/>
            <rdf:Description rdf:about="http://www.semanticweb.org/ontologies/2022/6/geological_taxonomy#Sylvinite"/>
            <rdf:Description rdf:about="http://www.semanticweb.org/ontologies/2022/6/geological_taxonomy#Tillite"/>
            <rdf:Description rdf:about="http://www.semanticweb.org/ontologies/2022/6/geological_taxonomy#Travertine"/>
            <rdf:Description rdf:about="http://www.semanticweb.org/ontologies/2022/6/geological_taxonomy#Tufa"/>
            <rdf:Description rdf:about="http://www.semanticweb.org/ontologies/2022/6/geological_taxonomy#Turbidite"/>
            <rdf:Description rdf:about="http://www.semanticweb.org/ontologies/2022/6/geological_taxonomy#Umber"/>
            <rdf:Description rdf:about="http://www.semanticweb.org/ontologies/2022/6/geological_taxonomy#Wackestone"/>
            <rdf:Description rdf:about="http://www.semanticweb.org/ontologies/2022/6/geological_taxonomy#Dolomite_(rock)"/>
        </owl:members>
    </rdf:Description>
    <rdf:Description>
        <rdf:type rdf:resource="http://www.w3.org/2002/07/owl#AllDisjointClasses"/>
        <owl:members rdf:parseType="Collection">
            <rdf:Description rdf:about="http://www.semanticweb.org/ontologies/2022/6/geological_taxonomy#Asthenosphere"/>
            <rdf:Description rdf:about="http://www.semanticweb.org/ontologies/2022/6/geological_taxonomy#Lithosphere"/>
            <rdf:Description rdf:about="http://www.semanticweb.org/ontologies/2022/6/geological_taxonomy#Lithosphere–asthenosphere_boundary"/>
        </owl:members>
    </rdf:Description>
    <rdf:Description>
        <rdf:type rdf:resource="http://www.w3.org/2002/07/owl#AllDisjointClasses"/>
        <owl:members rdf:parseType="Collection">
            <rdf:Description rdf:about="http://www.semanticweb.org/ontologies/2022/6/geological_taxonomy#Basaltic_trachyandesite"/>
            <rdf:Description rdf:about="http://www.semanticweb.org/ontologies/2022/6/geological_taxonomy#Benmoreite"/>
            <rdf:Description rdf:about="http://www.semanticweb.org/ontologies/2022/6/geological_taxonomy#Mugearite"/>
            <rdf:Description rdf:about="http://www.semanticweb.org/ontologies/2022/6/geological_taxonomy#Shoshonite"/>
        </owl:members>
    </rdf:Description>
    <rdf:Description>
        <rdf:type rdf:resource="http://www.w3.org/2002/07/owl#AllDisjointClasses"/>
        <owl:members rdf:parseType="Collection">
            <rdf:Description rdf:about="http://www.semanticweb.org/ontologies/2022/6/geological_taxonomy#Borates"/>
            <rdf:Description rdf:about="http://www.semanticweb.org/ontologies/2022/6/geological_taxonomy#Carbonates"/>
            <rdf:Description rdf:about="http://www.semanticweb.org/ontologies/2022/6/geological_taxonomy#Elements"/>
            <rdf:Description rdf:about="http://www.semanticweb.org/ontologies/2022/6/geological_taxonomy#Halides"/>
            <rdf:Description rdf:about="http://www.semanticweb.org/ontologies/2022/6/geological_taxonomy#Organic_compounds"/>
            <rdf:Description rdf:about="http://www.semanticweb.org/ontologies/2022/6/geological_taxonomy#Oxides"/>
            <rdf:Description rdf:about="http://www.semanticweb.org/ontologies/2022/6/geological_taxonomy#Phosphates_Arsenates_Vanadates"/>
            <rdf:Description rdf:about="http://www.semanticweb.org/ontologies/2022/6/geological_taxonomy#Silicates"/>
            <rdf:Description rdf:about="http://www.semanticweb.org/ontologies/2022/6/geological_taxonomy#Sulfates"/>
            <rdf:Description rdf:about="http://www.semanticweb.org/ontologies/2022/6/geological_taxonomy#Sulfides_and_Sulfosalts"/>
        </owl:members>
    </rdf:Description>
    <rdf:Description>
        <rdf:type rdf:resource="http://www.w3.org/2002/07/owl#AllDisjointClasses"/>
        <owl:members rdf:parseType="Collection">
            <rdf:Description rdf:about="http://www.semanticweb.org/ontologies/2022/6/geological_taxonomy#Breaching_of_a_barrier"/>
            <rdf:Description rdf:about="http://www.semanticweb.org/ontologies/2022/6/geological_taxonomy#Direct_flooding"/>
            <rdf:Description rdf:about="http://www.semanticweb.org/ontologies/2022/6/geological_taxonomy#Overtopping_of_a_barrier"/>
        </owl:members>
    </rdf:Description>
    <rdf:Description>
        <rdf:type rdf:resource="http://www.w3.org/2002/07/owl#AllDisjointClasses"/>
        <owl:members rdf:parseType="Collection">
            <rdf:Description rdf:about="http://www.semanticweb.org/ontologies/2022/6/geological_taxonomy#Cloudy"/>
            <rdf:Description rdf:about="http://www.semanticweb.org/ontologies/2022/6/geological_taxonomy#Fog"/>
            <rdf:Description rdf:about="http://www.semanticweb.org/ontologies/2022/6/geological_taxonomy#Rain"/>
            <rdf:Description rdf:about="http://www.semanticweb.org/ontologies/2022/6/geological_taxonomy#Snow"/>
            <rdf:Description rdf:about="http://www.semanticweb.org/ontologies/2022/6/geological_taxonomy#Stormy"/>
            <rdf:Description rdf:about="http://www.semanticweb.org/ontologies/2022/6/geological_taxonomy#Sunny"/>
            <rdf:Description rdf:about="http://www.semanticweb.org/ontologies/2022/6/geological_taxonomy#Windy"/>
        </owl:members>
    </rdf:Description>
    <rdf:Description>
        <rdf:type rdf:resource="http://www.w3.org/2002/07/owl#AllDisjointClasses"/>
        <owl:members rdf:parseType="Collection">
            <rdf:Description rdf:about="http://www.semanticweb.org/ontologies/2022/6/geological_taxonomy#Collapse_Earthquake"/>
            <rdf:Description rdf:about="http://www.semanticweb.org/ontologies/2022/6/geological_taxonomy#Explosion_Earthquake"/>
            <rdf:Description rdf:about="http://www.semanticweb.org/ontologies/2022/6/geological_taxonomy#Tectonic_Earthquake"/>
            <rdf:Description rdf:about="http://www.semanticweb.org/ontologies/2022/6/geological_taxonomy#Volcanic_Earthquake"/>
        </owl:members>
    </rdf:Description>
    <rdf:Description>
        <rdf:type rdf:resource="http://www.w3.org/2002/07/owl#AllDisjointClasses"/>
        <owl:members rdf:parseType="Collection">
            <rdf:Description rdf:about="http://www.semanticweb.org/ontologies/2022/6/geological_taxonomy#Continuous_creep"/>
            <rdf:Description rdf:about="http://www.semanticweb.org/ontologies/2022/6/geological_taxonomy#Progressive_creep"/>
            <rdf:Description rdf:about="http://www.semanticweb.org/ontologies/2022/6/geological_taxonomy#Seasonal_creep"/>
        </owl:members>
    </rdf:Description>
    <rdf:Description>
        <rdf:type rdf:resource="http://www.w3.org/2002/07/owl#AllDisjointClasses"/>
        <owl:members rdf:parseType="Collection">
            <rdf:Description rdf:about="http://www.semanticweb.org/ontologies/2022/6/geological_taxonomy#Crown_Fire"/>
            <rdf:Description rdf:about="http://www.semanticweb.org/ontologies/2022/6/geological_taxonomy#Ground_Fire"/>
            <rdf:Description rdf:about="http://www.semanticweb.org/ontologies/2022/6/geological_taxonomy#Surface_Fire"/>
        </owl:members>
    </rdf:Description>
    <rdf:Description>
        <rdf:type rdf:resource="http://www.w3.org/2002/07/owl#AllDisjointClasses"/>
        <owl:members rdf:parseType="Collection">
            <rdf:Description rdf:about="http://www.semanticweb.org/ontologies/2022/6/geological_taxonomy#Crust"/>
            <rdf:Description rdf:about="http://www.semanticweb.org/ontologies/2022/6/geological_taxonomy#Mantle"/>
            <rdf:Description rdf:about="http://www.semanticweb.org/ontologies/2022/6/geological_taxonomy#Planetary_core"/>
        </owl:members>
    </rdf:Description>
    <rdf:Description>
        <rdf:type rdf:resource="http://www.w3.org/2002/07/owl#AllDisjointClasses"/>
        <owl:members rdf:parseType="Collection">
            <rdf:Description rdf:about="http://www.semanticweb.org/ontologies/2022/6/geological_taxonomy#Cyclone"/>
            <rdf:Description rdf:about="http://www.semanticweb.org/ontologies/2022/6/geological_taxonomy#Drought"/>
            <rdf:Description rdf:about="http://www.semanticweb.org/ontologies/2022/6/geological_taxonomy#Earthquake"/>
            <rdf:Description rdf:about="http://www.semanticweb.org/ontologies/2022/6/geological_taxonomy#Extreme_Temperature"/>
            <rdf:Description rdf:about="http://www.semanticweb.org/ontologies/2022/6/geological_taxonomy#Flood"/>
            <rdf:Description rdf:about="http://www.semanticweb.org/ontologies/2022/6/geological_taxonomy#Landslide"/>
            <rdf:Description rdf:about="http://www.semanticweb.org/ontologies/2022/6/geological_taxonomy#Limnic_Eruption"/>
            <rdf:Description rdf:about="http://www.semanticweb.org/ontologies/2022/6/geological_taxonomy#Tsunami"/>
            <rdf:Description rdf:about="http://www.semanticweb.org/ontologies/2022/6/geological_taxonomy#Wildfire"/>
        </owl:members>
    </rdf:Description>
    <rdf:Description>
        <rdf:type rdf:resource="http://www.w3.org/2002/07/owl#AllDisjointClasses"/>
        <owl:members rdf:parseType="Collection">
            <rdf:Description rdf:about="http://www.semanticweb.org/ontologies/2022/6/geological_taxonomy#Fall"/>
            <rdf:Description rdf:about="http://www.semanticweb.org/ontologies/2022/6/geological_taxonomy#Flow"/>
            <rdf:Description rdf:about="http://www.semanticweb.org/ontologies/2022/6/geological_taxonomy#Slide"/>
            <rdf:Description rdf:about="http://www.semanticweb.org/ontologies/2022/6/geological_taxonomy#Subsidence"/>
            <rdf:Description rdf:about="http://www.semanticweb.org/ontologies/2022/6/geological_taxonomy#Topple"/>
        </owl:members>
    </rdf:Description>
    <rdf:Description>
        <rdf:type rdf:resource="http://www.w3.org/2002/07/owl#AllDisjointClasses"/>
        <owl:members rdf:parseType="Collection">
            <rdf:Description rdf:about="http://www.semanticweb.org/ontologies/2022/6/geological_taxonomy#Fibrists"/>
            <rdf:Description rdf:about="http://www.semanticweb.org/ontologies/2022/6/geological_taxonomy#Folists"/>
            <rdf:Description rdf:about="http://www.semanticweb.org/ontologies/2022/6/geological_taxonomy#Hemists"/>
            <rdf:Description rdf:about="http://www.semanticweb.org/ontologies/2022/6/geological_taxonomy#Saprists"/>
        </owl:members>
    </rdf:Description>
    <rdf:Description>
        <rdf:type rdf:resource="http://www.w3.org/2002/07/owl#AllDisjointClasses"/>
        <owl:members rdf:parseType="Collection">
            <rdf:Description rdf:about="http://www.semanticweb.org/ontologies/2022/6/geological_taxonomy#Geological_Object"/>
            <rdf:Description rdf:about="http://www.semanticweb.org/ontologies/2022/6/geological_taxonomy#Geological_phenomena"/>
            <rdf:Description rdf:about="http://www.semanticweb.org/ontologies/2022/6/geological_taxonomy#Units_of_Earth_structure"/>
        </owl:members>
    </rdf:Description>
    <rdf:Description>
        <rdf:type rdf:resource="http://www.w3.org/2002/07/owl#AllDisjointClasses"/>
        <owl:members rdf:parseType="Collection">
            <rdf:Description rdf:about="http://www.semanticweb.org/ontologies/2022/6/geological_taxonomy#Histels"/>
            <rdf:Description rdf:about="http://www.semanticweb.org/ontologies/2022/6/geological_taxonomy#Orthels"/>
            <rdf:Description rdf:about="http://www.semanticweb.org/ontologies/2022/6/geological_taxonomy#Turbels"/>
        </owl:members>
    </rdf:Description>
    <rdf:Description>
        <rdf:type rdf:resource="http://www.w3.org/2002/07/owl#AllDisjointClasses"/>
        <owl:members rdf:parseType="Collection">
            <rdf:Description rdf:about="http://www.semanticweb.org/ontologies/2022/6/geological_taxonomy#Hurricane"/>
            <rdf:Description rdf:about="http://www.semanticweb.org/ontologies/2022/6/geological_taxonomy#Major_Hurricane"/>
            <rdf:Description rdf:about="http://www.semanticweb.org/ontologies/2022/6/geological_taxonomy#Tropical_Depression"/>
            <rdf:Description rdf:about="http://www.semanticweb.org/ontologies/2022/6/geological_taxonomy#Tropical_Storm"/>
        </owl:members>
    </rdf:Description>
    <rdf:Description>
        <rdf:type rdf:resource="http://www.w3.org/2002/07/owl#AllDisjointClasses"/>
        <owl:members rdf:parseType="Collection">
            <rdf:Description rdf:about="http://www.semanticweb.org/ontologies/2022/6/geological_taxonomy#Igneous_rocks"/>
            <rdf:Description rdf:about="http://www.semanticweb.org/ontologies/2022/6/geological_taxonomy#Metamorphic_rocks"/>
            <rdf:Description rdf:about="http://www.semanticweb.org/ontologies/2022/6/geological_taxonomy#Sedimentary_rocks"/>
        </owl:members>
    </rdf:Description>
    <rdf:Description>
        <rdf:type rdf:resource="http://www.w3.org/2002/07/owl#AllDisjointClasses"/>
        <owl:members rdf:parseType="Collection">
            <rdf:Description rdf:about="http://www.semanticweb.org/ontologies/2022/6/geological_taxonomy#Lower_mantle"/>
            <rdf:Description rdf:about="http://www.semanticweb.org/ontologies/2022/6/geological_taxonomy#Upper_mantle"/>
            <rdf:Description rdf:about="http://www.semanticweb.org/ontologies/2022/6/geological_taxonomy#D_Double-Prime_(D’’)"/>
            <rdf:Description rdf:about="http://www.semanticweb.org/ontologies/2022/6/geological_taxonomy#Transition_zone_(Earth)"/>
        </owl:members>
    </rdf:Description>
    <rdf:Description>
        <rdf:type rdf:resource="http://www.w3.org/2002/07/owl#AllDisjointClasses"/>
        <owl:members rdf:parseType="Collection">
            <rdf:Description rdf:about="http://www.semanticweb.org/ontologies/2022/6/geological_taxonomy#Mineral"/>
            <rdf:Description rdf:about="http://www.semanticweb.org/ontologies/2022/6/geological_taxonomy#Rock"/>
            <rdf:Description rdf:about="http://www.semanticweb.org/ontologies/2022/6/geological_taxonomy#Soil"/>
        </owl:members>
    </rdf:Description>
</rdf:RDF>



<!-- Generated by the OWL API (version 4.5.29.2024-05-13T12:11:03Z) https://github.com/owlcs/owlapi -->

